#################### This file consists of 5 sections. You can find them by searching for '###'
## 1. Basic info about the ontology and GVP concept schemes
## 2. Hand-crafted properties
## 3. OWL Axioms (in addition to rdfs:subClassOf and rdfs:subPropertyOf
## 4. Classes, Properties and Values (individuals) defined from getty-codes.xls
## 5. Associative Relations: skos:related sub-properties defined from assoc-rels.xls
# We give section numbers/links to the documentation,
# and in some cases to https://share.getty.edu/confluence/, which is internal closed Confluence (wiki), sorry.

# http://vocab.getty.edu/doc/#GVP_URLs_and_Prefixes
@prefix aat:              <http://vocab.getty.edu/aat/>.
@prefix aat_contrib:      <http://vocab.getty.edu/aat/contrib/>.
@prefix aat_rel:          <http://vocab.getty.edu/aat/rel/>.
@prefix aat_rev:          <http://vocab.getty.edu/aat/rev/>.
@prefix aat_scopeNote:    <http://vocab.getty.edu/aat/scopeNote/>.
@prefix aat_source:       <http://vocab.getty.edu/aat/source/>.
@prefix aat_source_rev:   <http://vocab.getty.edu/aat/source/rev/>.
@prefix aat_term:         <http://vocab.getty.edu/aat/term/>.
@prefix tgn:              <http://vocab.getty.edu/tgn/>.
@prefix tgn_contrib:      <http://vocab.getty.edu/tgn/contrib/>.
@prefix tgn_rel:          <http://vocab.getty.edu/tgn/rel/>.
@prefix tgn_rev:          <http://vocab.getty.edu/tgn/rev/>.
@prefix tgn_scopeNote:    <http://vocab.getty.edu/tgn/scopeNote/>.
@prefix tgn_source:       <http://vocab.getty.edu/tgn/source/>.
@prefix tgn_source_rev:   <http://vocab.getty.edu/tgn/source/rev/>.
@prefix tgn_term:         <http://vocab.getty.edu/tgn/term/>.
@prefix ulan:             <http://vocab.getty.edu/ulan/>.
@prefix ulan_bio:         <http://vocab.getty.edu/ulan/bio/>.
@prefix ulan_contrib:     <http://vocab.getty.edu/ulan/contrib/>.
@prefix ulan_event:       <http://vocab.getty.edu/ulan/event/>.
@prefix ulan_rel:         <http://vocab.getty.edu/ulan/rel/>.
@prefix ulan_rev:         <http://vocab.getty.edu/ulan/rev/>.
@prefix ulan_scopeNote:   <http://vocab.getty.edu/ulan/scopeNote/>.
@prefix ulan_source:      <http://vocab.getty.edu/ulan/source/>.
@prefix ulan_source_rev:  <http://vocab.getty.edu/ulan/source/rev/>.
@prefix ulan_term:        <http://vocab.getty.edu/ulan/term/>.
@prefix gvp:              <http://vocab.getty.edu/ontology#>.
@prefix gvp_lang:         <http://vocab.getty.edu/language/>.

# http://vocab.getty.edu/doc/#External_Prefixes
@prefix bibo:          <http://purl.org/ontology/bibo/>.
@prefix bio:           <http://purl.org/vocab/bio/0.1/>.
@prefix dc:            <http://purl.org/dc/elements/1.1/>.
@prefix dct:           <http://purl.org/dc/terms/>.
@prefix foaf:          <http://xmlns.com/foaf/0.1/>.
@prefix iso:           <http://purl.org/iso25964/skos-thes#> .
@prefix luc:           <http://www.ontotext.com/owlim/lucene#>.
@prefix ontogeo:       <http://www.ontotext.com/owlim/geo#>.
@prefix owl:           <http://www.w3.org/2002/07/owl#>.
@prefix prov:          <http://www.w3.org/ns/prov#>.
@prefix ptop:          <http://www.ontotext.com/proton/protontop#>.
@prefix rdf:           <http://www.w3.org/1999/02/22-rdf-syntax-ns#>.
@prefix rdfs:          <http://www.w3.org/2000/01/rdf-schema#>.
@prefix rr:            <http://www.w3.org/ns/r2rml#>.
@prefix rrx:           <http://purl.org/r2rml-ext/>.
@prefix sesame:        <http://www.openrdf.org/schema/sesame#>.
@prefix schema:        <http://schema.org/>.
@prefix skos:          <http://www.w3.org/2004/02/skos/core#>.
@prefix skosxl:        <http://www.w3.org/2008/05/skos-xl#>.
@prefix wgs:           <http://www.w3.org/2003/01/geo/wgs84_pos#>.
@prefix xsd:           <http://www.w3.org/2001/XMLSchema#>.

# http://vocab.getty.edu/doc/#Descriptive_Prefixes
# (used only in http://vocab.getty.edu/.well-known/void = http://vocab.getty.edu/void.ttl)
@prefix adms:   <http://www.w3.org/ns/adms#> .                       # Asset Description Metadata Schema
@prefix cc:     <http://creativecommons.org/ns#> .                   # Creative Commons Rights Expression Language
@prefix dcat:   <http://www.w3.org/ns/dcat#> .                       # Data Catalog Vocabulary
@prefix dctype: <http://purl.org/dc/dcmitype/> .                     # DCMI Type Vocabulary
@prefix fmt:    <http://www.w3.org/ns/formats/> .                    # RDF formats used in datasets
@prefix sd:     <http://www.w3.org/ns/sparql-service-description#> . # SPARQL Service Description
@prefix vaem:   <http://www.linkedmodel.org/schema/vaem#> .          # Vocabulary for Attaching Essential Metadata
@prefix vann:   <http://purl.org/vocab/vann/> .                      # Vocabulary for annotating vocabulary descriptions
@prefix vcard:  <http://www.w3.org/2006/vcard/ns#> .                 # vCard (contact info)
@prefix vdpp:   <http://data.lirmm.fr/ontologies/vdpp#> .            # Vocabulary for Dataset Publication Projects
@prefix voaf:   <http://purl.org/vocommons/voaf#> .                  # Vocabulary of a Friend
@prefix voag:   <http://voag.linkedmodel.org/voag#> .                # Vocabulary Of Attribution and Governance
@prefix void:   <http://rdfs.org/ns/void#> .                         # Vocabulary of Interlinked Datasets
@prefix wdrs:   <http://www.w3.org/2007/05/powder-s#> .              # Protocol for Web Description Resources
@prefix wv:     <http://vocab.org/waiver/terms/> .                   # A vocabulary for waivers of rights

#################### Basic info about the ontology and GVP concept schemes ####################

# https://share.getty.edu/confluence/display/ITSLODV/Descriptive+Info
# lots more in http://vocab.getty.edu/.well-known/void

<http://vocab.getty.edu/ontology> a owl:Ontology, voaf:Vocabulary ;
  rdfs:label "Getty Vocabulary Program ontology" ;
  rdfs:comment """The GVP Ontology defines classes, properties and values (skos:Concepts) used in GVP LOD.
As of version 3.0, it is complete regarding AAT, TGN and ULAN, and will be extended in time with more elements needed for other GVP vocabularies (CONA).
It uses the SKOS, SKOS-XL, ISO 25964; DC, DCT, BIBO, FOAF, BIO, Schema, PROV, WGS84 ontologies, but we import only the first 3""";
  dct:created  "2014-02-15"^^xsd:date;
  dct:issued   "2014-02-20"^^xsd:date;
  dct:modified "2016-04-25"^^xsd:date;
  dct:creator <http://www.getty.edu/research/>, <http://www.ontotext.com>;
  dc:format "meta/rdf-schema";
  rdfs:seeAlso
    <http://vocab.getty.edu/doc>,
    <http://vocab.getty.edu/doc/queries>,
    <http://www.getty.edu/research/tools/vocabularies/lod/>,
    <http://vocab.getty.edu/.well-known/void>,
    <http://lov.okfn.org/dataset/lov/details/vocabulary_gvp.html>;
  vann:preferredNamespacePrefix "gvp";
  vann:preferredNamespaceUri "http://vocab.getty.edu/ontology#" ;
  owl:imports
    <http://www.w3.org/2004/02/skos/core>,
    <http://www.w3.org/2008/05/skos-xl>,
    <http://purl.org/iso25964/skos-thes>;
  owl:versionInfo "3.3";
  skos:changeNote
    """2.0 changes: replaced gvp:broaderTransitive with gvp:broaderExtended.
3.0 changes: replaced schema:startDate, endDate with gvp:estStart, estEnd; added ULAN). See details in referenced links.
3.1 & 3.2: no changes.
3.3: added 6 associative relations: gvp:aat2886_used-function_as - gvp:aat2887_exemplified_by, gvp:tgn3103_located_on - gvp:tgn3104_is_location_of, and gvp:ulan2583_chairman_of - gvp:ulan2584_chaired_by""",
    <http://vocab.getty.edu/doc#Version_2.0>,
    <http://vocab.getty.edu/doc#Version_3.0>,
    <http://vocab.getty.edu/doc#Version_3.3>.

aat: a skos:ConceptScheme;
  rdfs:label "Art and Architecture Thesaurus";
  rdfs:comment "The Art and Architecture Thesaurus concept scheme";
  dct:created "2014-02-20"^^xsd:date;
  dct:creator <http://www.getty.edu/research/>, <http://www.ontotext.com>;
  foaf:homepage <http://www.getty.edu/research/tools/vocabularies/aat/>;
  rdfs:seeAlso <http://vocab.getty.edu/>, <http://www.getty.edu/research/tools/vocabularies/lod/>,
    <http://vocab.getty.edu/.well-known/void>;
  vann:preferredNamespacePrefix "aat";
  vann:preferredNamespaceUri "http://vocab.getty.edu/aat/".

tgn: a skos:ConceptScheme;
  rdfs:label "Thesaurus of Geographic Names";
  rdfs:comment "The Thesaurus of Geographic Names concept scheme";
  dct:created "2014-06-15"^^xsd:date;
  dct:creator <http://www.getty.edu/research/>, <http://www.ontotext.com>;
  foaf:homepage <http://www.getty.edu/research/tools/vocabularies/tgn/>;
  rdfs:seeAlso <http://vocab.getty.edu/>, <http://www.getty.edu/research/tools/vocabularies/lod/>,
    <http://vocab.getty.edu/.well-known/void>;
  vann:preferredNamespacePrefix "tgn";
  vann:preferredNamespaceUri "http://vocab.getty.edu/tgn/".

ulan: a skos:ConceptScheme;
  rdfs:label "Union List of Artist Names";
  rdfs:comment "The Union List of Artist Names concept scheme";
  dct:created "2015-03-25"^^xsd:date;
  dct:creator <http://www.getty.edu/research/>, <http://www.ontotext.com>;
  foaf:homepage <http://www.getty.edu/research/tools/vocabularies/ulan/>;
  rdfs:seeAlso <http://vocab.getty.edu/>, <http://www.getty.edu/research/tools/vocabularies/lod/>,
    <http://vocab.getty.edu/.well-known/void>;
  vann:preferredNamespacePrefix "ulan";
  vann:preferredNamespaceUri "http://vocab.getty.edu/ulan/".

<http://www.getty.edu/research/> a foaf:Organization;
  rdfs:label "Getty Research Institute";
  foaf:name "Getty Research Institute".

<http://www.ontotext.com> a foaf:Organization;
  rdfs:label "Ontotext Corp";
  foaf:name "Ontotext Corp".

#################### Hand-crafted classes and properties ####################

# http://vocab.getty.edu/doc#Subject_Types

gvp:Subject a owl:Class ;
  rdfs:isDefinedBy <http://vocab.getty.edu/ontology> ;
  rdfs:label "Subject" ;
  rdfs:comment """Node in a GVP vocabulary hierarchy. 
May be Facet, GuideTerm, Hierarchy, Concept, AdminPlaceConcept, PhysPlaceConcept, PhysAdminPlaceConcept, or ObsoleteSubject.
Implemented as skos:Concept or iso:ThesaurusArray and skos:Collection""";
  dct:description """Node in a GVP vocabulary hierarchy. 
May be Facet, GuideTerm, Hierarchy, Concept, AdminPlaceConcept, PhysPlaceConcept, PhysAdminPlaceConcept, or ObsoleteSubject.
Implemented as skos:Concept or iso:ThesaurusArray and skos:Collection""".

# http://vocab.getty.edu/doc#GVP_Hierarchical_Relations
# https://share.getty.edu/confluence/display/ITSLODV/Hierarchical+Relations

gvp:broader a owl:ObjectProperty;
  rdfs:isDefinedBy <http://vocab.getty.edu/ontology> ;
  rdfs:label "broader";
  rdfs:domain gvp:Subject; rdfs:range gvp:Subject;
  rdfs:comment "Parents of a subject. Each broader is also Preferred|NonPreferred and Partitive|Instantial|Generic";
  dct:description "Parents of a subject. Each broader is also Preferred|NonPreferred and Partitive|Instantial|Generic".

gvp:broaderGenericExtended a owl:ObjectProperty;
  rdfs:isDefinedBy <http://vocab.getty.edu/ontology> ;
  rdfs:label "broaderGenericExtended";
  rdfs:domain gvp:Subject; rdfs:range gvp:Subject;
  rdfs:comment "Ancestors (Generic). Meaningful closure of gvp:broaderGeneric. Infers iso:broaderGeneric for pairs of directly related skos:Concepts";
  skos:example """<anvils and anvil accessories> BTG <forging and metal-shaping tools> BTG <forging and metal-shaping equipment>,
so <anvils and anvil accessories> BTGE <forging and metal-shaping equipment>""";
  dct:description """Ancestors (Generic). Meaningful closure of gvp:broaderGeneric. Infers iso:broaderGeneric for pairs of directly related skos:Concepts.
Example: <anvils and anvil accessories> BTG <forging and metal-shaping tools> BTG <forging and metal-shaping equipment>,
so <anvils and anvil accessories> BTGE <forging and metal-shaping equipment>""".

gvp:broaderPartitiveExtended a owl:ObjectProperty;
  rdfs:isDefinedBy <http://vocab.getty.edu/ontology> ;
  rdfs:label "broaderPartitiveExtended";
  rdfs:domain gvp:Subject; rdfs:range gvp:Subject;
  rdfs:comment "Ancestors (Partitive). Meaningful closure of gvp:broaderPartitive. Infers iso:broaderPartitive for pairs of directly related skos:Concepts";
  skos:example """anvil components BTP <anvils and anvil accessories> BTG <forging and metal-shaping tools>,
so anvil components BTPE <forging and metal-shaping tools>""";
  dct:description """Ancestors (Partitive). Meaningful closure of gvp:broaderPartitive. Infers iso:broaderPartitive for pairs of directly related skos:Concepts.
Example: anvil components BTP <anvils and anvil accessories> BTG <forging and metal-shaping tools>,
so anvil components BTPE <forging and metal-shaping tools>""".

gvp:broaderInstantialExtended a owl:ObjectProperty;
  rdfs:isDefinedBy <http://vocab.getty.edu/ontology> ;
  rdfs:label "broaderInstantialExtended";
  rdfs:domain gvp:Subject; rdfs:range gvp:Subject;
  #rdfs:comment "Ancestors (Instantial). Meaningful closure of gvp:broaderInstantial. Infers iso:broaderInstantial for pairs of directly related skos:Concepts";
  skos:example """Mt Athos (TGN) BTI orthodox religious center (AAT) BTG Christian religious center (AAT),
so Mt Athos (TGN) BTIE Christian religious center (AAT)""";
  dct:description """Ancestors (Instantial). Meaningful closure of gvp:broaderInstantial. Infers iso:broaderInstantial for pairs of directly related skos:Concepts.""".

gvp:broaderExtended a owl:ObjectProperty;
  rdfs:isDefinedBy <http://vocab.getty.edu/ontology> ;
  rdfs:label "broaderExtended";
  rdfs:domain gvp:Subject; rdfs:range gvp:Subject;
  rdfs:comment "Appropriate ancestors. Meaningful closure of gvp:broader for query expansion. Use this, not skos:broaderTransitive";
  skos:example """Mt Athos has ancestor places (BTPE) World, Europe, Greece, Macedonia, Pangaíon Óros regional division;
and place types (BTIE) inhabited place; and orthodox religious center, Christian religious center, religious center""";
  dct:description """Appropriate ancestors. Meaningful closure of gvp:broader for query expansion. Use this, not skos:broaderTransitive.
Example: Mt Athos has ancestor places (BTPE) World, Europe, Greece, Macedonia, Pangaíon Óros regional division;
and place types (BTIE) inhabited place; and orthodox religious center, Christian religious center, religious center""".

gvp:broaderPreferredExtended a owl:ObjectProperty;
  rdfs:isDefinedBy <http://vocab.getty.edu/ontology> ;
  rdfs:label "broaderPreferredExtended";
  rdfs:domain gvp:Subject; rdfs:range gvp:Subject;
  rdfs:comment "Preferred Ancestors. Meaningful closure of gvp:broaderPreferred. Needed to display the hierarchy";
  skos:example """Mt Athos has preferred ancestor places (BTPE) World, Europe, Greece, Macedonia, Pangaíon Óros regional division;
and prefererd place type (BTIE) inhabited place""";
  dct:description """Preferred Ancestors. Meaningful closure of gvp:broaderPreferred. Needed to display the hierarchy.
Example: Mt Athos has preferred ancestor places (BTPE) World, Europe, Greece, Macedonia, Pangaíon Óros regional division;
and prefererd place type (BTIE) inhabited place""".

## http://vocab.getty.edu/doc#Reduced_SKOS_Inference
#gvp:narrower a owl:ObjectProperty;
#  rdfs:isDefinedBy <http://vocab.getty.edu/ontology> ;
#  rdfs:label "narrower";
#  rdfs:domain gvp:Subject; rdfs:range gvp:Subject;
#  rdfs:comment "Children of a subject. Inverse of gvp:broader";
#  dct:description "Children of a subject. Inverse of gvp:broader";
#  owl:inverseOf gvp:broader.
#
#gvp:narrowerExtended a owl:ObjectProperty;
#  rdfs:isDefinedBy <http://vocab.getty.edu/ontology> ;
#  rdfs:label "narrowerExtended";
#  rdfs:domain gvp:Subject; rdfs:range gvp:Subject;
#  rdfs:comment "Appropriate descendants. Meaningful closure of gvp:narrower for query expansion. Use this, not skos:narrowerTransitive";
#  dct:description "Appropriate descendants. Meaningful closure of gvp:narrower for query expansion. Use this, not skos:narrowerTransitive".
#gvp:narrowerExtended owl:inverseOf gvp:broaderExtended.


# http://vocab.getty.edu/doc#Subject
# https://share.getty.edu/confluence/display/ITSLODV/Subjects

gvp:parentString a owl:DatatypeProperty;
  rdfs:isDefinedBy <http://vocab.getty.edu/ontology> ;
  rdfs:label "parentString";
  rdfs:domain gvp:Subject;
  rdfs:range rdfs:Literal;
  rdfs:comment "Preferred labels of *all* of the subject's preferred ancestors, listed bottom up. Useful to show the subject's full context";
  skos:note "Display version of gvp:broaderPreferredExtended";
  skos:example "For aat:300226882 baking dishes: bakeware, <vessels for cooking food>, <containers for cooking food>, <culinary containers>, <containers by function or context>, containers (receptacles), Containers (Hierarchy Name), Furnishings and Equipment (Hierarchy Name), Objects Facet";
  dct:description """Preferred labels of *all* of the subject's preferred ancestors, listed bottom up. Useful to show the subject's full context.
Display version of gvp:broaderPreferredExtended.
For aat:300226882 baking dishes: bakeware, <vessels for cooking food>, <containers for cooking food>, <culinary containers>, <containers by function or context>, containers (receptacles), Containers (Hierarchy Name), Furnishings and Equipment (Hierarchy Name), Objects Facet""".

gvp:parentStringAbbrev a owl:DatatypeProperty;
  rdfs:isDefinedBy <http://vocab.getty.edu/ontology> ;
  rdfs:label "parentStringAbbrev";
  rdfs:domain gvp:Subject;
  rdfs:range rdfs:Literal;
  rdfs:comment "Preferred labels of *some* of the subject's preferred ancestors, listed bottom up. Useful to show the subject's context";
  skos:note "Shortened display version of gvp:broaderPreferredExtended";
  skos:example "For aat:300226882 baking dishes: bakeware, <vessels for cooking food>, ... Furnishings and Equipment (Hierarchy Name)";
  dct:description """Preferred labels of *some* of the subject's preferred ancestors, listed bottom up. Useful to show the subject's context.
Shortened display version of gvp:broaderPreferredExtended.
Example for aat:300226882 baking dishes: bakeware, <vessels for cooking food>, ... Furnishings and Equipment (Hierarchy Name)""".

# https://jira.getty.edu/browse/ITSLOD-183 TGN flag Famous

gvp:isNoted a owl:DatatypeProperty;
  rdfs:isDefinedBy <http://vocab.getty.edu/ontology> ;
  rdfs:label "isNoted";
  rdfs:domain gvp:Subject;
  rdfs:range xsd:boolean;
  rdfs:comment "One amongst several homographic concepts may be especially noted so it's easier to find";
  skos:example "tgn:7008038 Paris, France is noted but tgn:2106600 Paris, Texas is not (except if you're Fassbinder)";
  dct:description """One amongst several homographic concepts may be especially noted so it's easier to find.
Example: tgn:7008038 Paris, France is noted but tgn:2106600 Paris, Texas is not (except if you're Fassbinder)""".

# http://vocab.getty.edu/doc#Term
# https://share.getty.edu/confluence/display/ITSLODV/Terms

gvp:term a owl:DatatypeProperty;
  rdfs:isDefinedBy <http://vocab.getty.edu/ontology> ;
  rdfs:domain skosxl:Label;
  rdfs:range rdfs:Literal;
  rdfs:label "term";
  rdfs:comment "Term (label), used as the basic (prefix) part of skosxsl:literalForm";
  dct:description "Term (label), used as the basic (prefix) part of skosxsl:literalForm".

gvp:qualifier a owl:DatatypeProperty;
  rdfs:isDefinedBy <http://vocab.getty.edu/ontology> ;
  rdfs:domain skosxl:Label;
  rdfs:range rdfs:Literal;
  rdfs:label "qualifier";
  rdfs:comment """Clarifies and disambiguates terms with the same spelling but different meaning.
Appended in parentheses to gvp:term, forming skosxsl:literalForm.
Every qualifier is in the same language as the term""";
  skos:example "Rhea (vessels)=rhyta (a kind of drinking vessel) vs rhea (species)=Boehmeria nivea (Chinese grass)";
  dct:description """Clarifies and disambiguates terms with the same spelling but different meaning.
Appended in parentheses to gvp:term, forming skosxsl:literalForm.
Every qualifier is in the same language as the term.
Example: "Rhea (vessels)"=rhyta (a kind of drinking vessel) vs "Rhea (species)"=Boehmeria nivea (Chinese grass)""".

# http://vocab.getty.edu/doc#Scope_Note
gvp:ScopeNote a owl:Class;
  rdfs:isDefinedBy <http://vocab.getty.edu/ontology> ;
  rdfs:comment """Defines a GVP subject or provides usage information. Has fields:
- dc:identifier: numeric ID, also used in the URL.
- rdf:value: the note itself (as per SKOS Primer: 4.2 Advanced Documentation Features) with language tag
- dct:language: matches the language tag
- gvp:displayOrder, order of this note amongst others
- gvp:historicFlag, gvp:estStart, gvp:estEnd, rdfs:comment: Historic Information about applicability
- dct:source or subproperties thereof 
- dct:contributor or subproperties thereof""";
  dct:description """Defines a GVP subject or provides usage information. Has fields:
- dc:identifier: numeric ID, also used in the URL.
- rdf:value: the note itself (as per SKOS Primer: 4.2 Advanced Documentation Features) with language tag
- dct:language: matches the language tag
- gvp:displayOrder, order of this note amongst others
- gvp:historicFlag, vp:estStart, gvp:estEnd, rdfs:comment: Historic Information about applicability
- dct:source or subproperties thereof 
- dct:contributor or subproperties thereof""".

# http://vocab.getty.edu/doc#Sort_Order
# https://share.getty.edu/confluence/display/ITSLODV/Sort+Order
gvp:displayOrder a owl:DatatypeProperty;
  rdfs:isDefinedBy <http://vocab.getty.edu/ontology> ;
  rdfs:label "displayOrder";
  rdfs:range xsd:positiveInteger;
  rdfs:comment """Display order of subject or term amongst its siblings.
If all are 1 then use alphabetical. Domain is gvp:Subject or skosxl:Label""";
  dct:description """Display order of subject or term amongst its siblings.
If all are 1 then use alphabetical. Domain is gvp:Subject or skosxl:Label""".

# http://vocab.getty.edu/doc#Estimated_Dates
# https://share.getty.edu/confluence/display/ITSLODV/Start+and+End+Dates
gvp:estStart a owl:DatatypeProperty;
  rdfs:isDefinedBy <http://vocab.getty.edu/ontology> ;
  rdfs:label "estStart";
  rdfs:comment "Estimated start date of term, relation, type assignment, event, biography";
  dct:description "Estimated start date of term, relation, type assignment, event, biography".

gvp:estEnd a owl:DatatypeProperty;
  rdfs:isDefinedBy <http://vocab.getty.edu/ontology> ;
  rdfs:label "estEnd";
  rdfs:comment "Estimated end date of term, relation, type assignment, event, biography";
  dct:description "Estimated end date of term, relation, type assignment, event, biography".
  
# http://vocab.getty.edu/doc#TGN_Place_Types
# https://share.getty.edu/confluence/display/ITSLODV/TGN+Place+Types
gvp:placeType a owl:ObjectProperty;
  rdfs:isDefinedBy <http://vocab.getty.edu/ontology> ;
  rdfs:label "placeType";
  rdfs:domain gvp:Subject; # TGN AdminPlaceConcept or PhysPlaceConcept
  rdfs:range gvp:Subject; # AAT Concept
  rdfs:comment "Type for a TGN place. Domain is TGN concept (AdminPlaceConcept or PhysPlaceConcept), range is AAT Concept";
  skos:example """Machupicchu, Peru has preferred type "deserted settlement" (current) and non-preferred type "Inca center" (historic)""";
  dct:description """Type for a TGN place. Domain is TGN concept (AdminPlaceConcept or PhysPlaceConcept), range is AAT Concept.
Example: Machupicchu, Peru has preferred type "deserted settlement" (current) and non-preferred type "Inca center" (historic)""".

#### ULAN Classes and Properties

gvp:agentType a owl:ObjectProperty ;
  rdfs:isDefinedBy <http://vocab.getty.edu/ontology> ;
  rdfs:label "agentType";
  rdfs:domain gvp:Subject; # ULAN
  rdfs:range gvp:Subject; # AAT
  rdfs:comment "Type of a ULAN PersonConcept or GroupConcept. Domain is ULAN concept, range is AAT concept";
  dct:description "Type of a ULAN PersonConcept or GroupConcept. Domain is ULAN concept, range is AAT concept".

gvp:Biography a owl:Class;
  rdfs:isDefinedBy <http://vocab.getty.edu/ontology> ;
  rdfs:comment """Biography of a ULAN agent (schema:Person|Organization). Depending on the agent, has these fields:
- schema:description: one-line-biography
- gvp:estStart
- schema:birthPlace | foundationLocation, pointing to TGN
- gvp:estEnd
- schema:deathPlace | dissolutionLocation, pointing to TGN
- schema:gender, pointing to AAT (male, female, other)
- dct:contributor
The fields of the preferred biogrpahy are also available in the agent.""".

gvp:biography a owl:ObjectProperty ;
  rdfs:isDefinedBy <http://vocab.getty.edu/ontology> ;
  rdfs:label "biography" ;
  rdfs:range gvp:Biography ;
  rdfs:subPropertyOf gvp:biography ;
  rdfs:comment "Biography of an ULAN agent. Domain is schema:Person/Organization, range is gvp:Biography. The preferred biography fields are also directly available in the Person/Organization";
  dct:description "Biography of an ULAN agent. Domain is schema:Person/Organization, range is gvp:Biography. The preferred biography fields are also directly available in the Person/Organization" .

# Hijacking a property in the schema.org namespace
schema:dissolutionLocation a owl:ObjectProperty;
  rdfs:isDefinedBy <http://vocab.getty.edu/ontology> ;
  rdfs:label "dissolutionLocation";
  rdfs:domain schema:Organization;
  rdfs:range schema:Place;
  rdfs:comment "The place where the Organization was dissolved";
  dct:description """The place where the Organization was dissolved.
Schema has properties foundationLocation and dissolutionDate but no dissolutionLocation. 
In contrast, for a person all 4 properties are present: birth/death place/date.
We posted issue https://github.com/schemaorg/schemaorg/issues/302, which looks like it will have a positive outcome in the far future.
And we define the property here""";
  rdfs:seeAlso <https://github.com/schemaorg/schemaorg/issues/302>.

## coreference of gender values
aat:300189559 skos:exactMatch <http://www.wikidata.org/entity/Q6581097>, <http://rdaregistry.info/termList/gender/1002>. # male
aat:300189557 skos:exactMatch <http://www.wikidata.org/entity/Q6581072>, <http://rdaregistry.info/termList/gender/1001>. # female

#################### OWL Axioms (in addition to rdfs:subClassOf and rdfs:subPropertyOf ####################

# http://vocab.getty.edu/doc#Obsolete_Subject
# https://share.getty.edu/confluence/display/ITSLODV/Obsolete+Subjects

dct:isReplacedBy owl:inverseOf dct:replaces.

# http://vocab.getty.edu/doc#SKOS-XL_Inference
# https://share.getty.edu/confluence/display/ITSLODV/Inference

skos:prefLabel   owl:propertyChainAxiom (skosxl:prefLabel   skosxl:literalForm).
skos:altLabel    owl:propertyChainAxiom (skosxl:altLabel    skosxl:literalForm).
skos:hiddenLabel owl:propertyChainAxiom (skosxl:hiddenLabel skosxl:literalForm).

# http://vocab.getty.edu/doc#BTG,_BTP,_BTI_Inference
# See V.Alexiev, J.Lindenthal, A.Isaac.
# Compositionality of ISO 25964 Hierarchical Relations, May 2014, submitted
# https://drive.google.com/file/d/0B7BFygWDV2_PNkQycHl0bWNLak0

# I1: BTG->BTGE, BTP->BTPE, BTI->BTIE: basic inferences
gvp:broaderGeneric    rdfs:subPropertyOf gvp:broaderGenericExtended.
gvp:broaderPartitive  rdfs:subPropertyOf gvp:broaderPartitiveExtended.
gvp:broaderInstantial rdfs:subPropertyOf gvp:broaderInstantialExtended.

# I2: BTGx/BTGx=>BTGE
gvp:broaderGenericExtended   owl:propertyChainAxiom  (gvp:broaderGenericExtended gvp:broaderGeneric).

# I3: BTGx/BTPx=>BTPE
gvp:broaderPartitiveExtended owl:propertyChainAxiom  (gvp:broaderGeneric gvp:broaderPartitiveExtended).
# I5: BTPx/BTGx=>BTPE
gvp:broaderPartitiveExtended owl:propertyChainAxiom  (gvp:broaderPartitiveExtended gvp:broaderGeneric).
# I6: BTPx/BTPx=>BTPE
gvp:broaderPartitiveExtended owl:propertyChainAxiom  (gvp:broaderPartitiveExtended gvp:broaderPartitive).

# I8: BTIx/BTGx=>BTIE
gvp:broaderInstantialExtended owl:propertyChainAxiom (gvp:broaderInstantialExtended gvp:broaderGeneric).

# I11: BTGE|BTPE|BTIE=>BTE
gvp:broaderGenericExtended    rdfs:subPropertyOf gvp:broaderExtended.
gvp:broaderPartitiveExtended  rdfs:subPropertyOf gvp:broaderExtended.
gvp:broaderInstantialExtended rdfs:subPropertyOf gvp:broaderExtended.

# http://vocab.getty.edu/doc#broaderPreferredExtended_Rules
gvp:broaderPreferred rdfs:subPropertyOf gvp:broaderPreferredExtended.

gvp:Infer_broaderPreferredExtended a ptop:PropChainRestr;
  ptop:premise1 gvp:broaderPreferredExtended;
  ptop:premise2 gvp:broaderPreferred;
  ptop:restriction gvp:broaderExtended;
  ptop:conclusion gvp:broaderPreferredExtended.

# http://vocab.getty.edu/doc#ISO_Rules
gvp:broaderNonConcept a owl:ObjectProperty;
  rdfs:isDefinedBy <http://vocab.getty.edu/ontology> ;
  rdfs:label "broaderNonConcept";
  rdfs:domain skos:Concept; rdfs:range gvp:GuideTerm;
  rdfs:comment "Chain of gvp:broader from Concept to GuideTerms, without intervening Concept";
  dct:description "Chain of gvp:broader from Concept to GuideTerms, without intervening Concept".

gvp:Infer_broaderNonConcept_TypeRestr a ptop:TypeRestr;
  ptop:premise gvp:broader;
  ptop:type1 skos:Concept;
  ptop:type2 gvp:GuideTerm;
  ptop:conclusion gvp:broaderNonConcept.
gvp:Infer_broaderNonConcept_PropChainType2 a ptop:PropChainType2;
  ptop:premise1 gvp:broaderNonConcept;
  ptop:premise2 gvp:broader;
  ptop:type2 gvp:GuideTerm;
  ptop:conclusion gvp:broaderNonConcept.

gvp:Infer_skosBroader_TypeRestr a ptop:TypeRestr;
  ptop:premise gvp:broader;
  ptop:type1 skos:Concept;
  ptop:type2 skos:Concept;
  ptop:conclusion skos:broader.
gvp:Infer_skosBroader_PropChainType2 a ptop:PropChainType2;
  ptop:premise1 gvp:broaderNonConcept;
  ptop:premise2 gvp:broader;
  ptop:type2 skos:Concept;
  ptop:conclusion skos:broader.

gvp:Infer_isoBroaderGeneric a ptop:PropRestr;
  ptop:premise gvp:broaderGenericExtended;
  ptop:restriction skos:broader;
  ptop:conclusion iso:broaderGeneric.
gvp:Infer_isoBroaderPartitive a ptop:PropRestr;
  ptop:premise gvp:broaderPartitiveExtended;
  ptop:restriction skos:broader;
  ptop:conclusion iso:broaderPartitive.
gvp:Infer_isoBroaderInstantial a ptop:PropRestr;
  ptop:premise gvp:broaderInstantialExtended;
  ptop:restriction skos:broader;
  ptop:conclusion iso:broaderInstantial.

#################### Classes, Properties and Values (individuals) defined from getty-codes.xls ####################

gvp:Facet a owl:Class ;
  rdfs:isDefinedBy <http://vocab.getty.edu/ontology> ;
  rdfs:subClassOf gvp:Subject, iso:ThesaurusArray ;
  rdfs:label "Facet" ;
  rdfs:comment "One of the major divisions of a vocabulary" ;
  skos:example "Objects Facet (AAT), World (TGN), Artists (ULAN)" ;
  dct:description "One of the major divisions of a vocabulary.\nExample: Objects Facet (AAT), World (TGN), Artists (ULAN)".

gvp:Hierarchy a owl:Class ;
  rdfs:isDefinedBy <http://vocab.getty.edu/ontology> ;
  rdfs:subClassOf gvp:Subject, iso:ThesaurusArray ;
  rdfs:label "Hierarchy" ;
  rdfs:comment "Top of a hierarchy. Used in AAT only. Not used for indexing or cataloguing" ;
  skos:example "Containers (Hierarchy Name) (AAT)" ;
  dct:description "Top of a hierarchy. Used in AAT only. Not used for indexing or cataloguing.\nExample: Containers (Hierarchy Name) (AAT)".

gvp:GuideTerm a owl:Class ;
  rdfs:isDefinedBy <http://vocab.getty.edu/ontology> ;
  rdfs:subClassOf gvp:Subject, iso:ThesaurusArray ;
  rdfs:label "GuideTerm" ;
  rdfs:comment "Guide Term: place holder to create a level in the hierarchy. Used in AAT and ULAN. Not used for indexing or cataloguing." ;
  skos:example "<vessels for serving and consuming food> (AAT), ulan:500353455 <named animals> under facet Non-Artists (ULAN)" ;
  dct:description "Guide Term: place holder to create a level in the hierarchy. Used in AAT and ULAN. Not used for indexing or cataloguing..\nExample: <vessels for serving and consuming food> (AAT), ulan:500353455 <named animals> under facet Non-Artists (ULAN)".

gvp:Concept a owl:Class ;
  rdfs:isDefinedBy <http://vocab.getty.edu/ontology> ;
  rdfs:subClassOf gvp:Subject, skos:Concept ;
  rdfs:label "Concept" ;
  rdfs:comment "Proper concept. Used in AAT only; TGN & ULAN have their own, e.g. gvp:PhysPlaceConcept & gvp:PersonConcept. Used for indexing and cataloguing" ;
  skos:example "rhyta (AAT)" ;
  dct:description "Proper concept. Used in AAT only; TGN & ULAN have their own, e.g. gvp:PhysPlaceConcept & gvp:PersonConcept. Used for indexing and cataloguing.\nExample: rhyta (AAT)".

gvp:ObsoleteSubject a owl:Class ;
  rdfs:isDefinedBy <http://vocab.getty.edu/ontology> ;
  rdfs:subClassOf gvp:Subject ;
  rdfs:label "ObsoleteSubject" ;
  rdfs:comment "Obsolete subject: moved out of the publishable hierarchy, or merged to another (pointed by dct:isReplacedBy)" ;
  skos:example "300375205 \"shranks\" (AAT) was merged to 300039264 \"schranks\" (AAT), so aat:300375205 dct:isReplacedBy aat:300039264" ;
  dct:description "Obsolete subject: moved out of the publishable hierarchy, or merged to another (pointed by dct:isReplacedBy).\nExample: 300375205 \"shranks\" (AAT) was merged to 300039264 \"schranks\" (AAT), so aat:300375205 dct:isReplacedBy aat:300039264".

gvp:PhysPlaceConcept a owl:Class ;
  rdfs:isDefinedBy <http://vocab.getty.edu/ontology> ;
  rdfs:subClassOf gvp:Subject, skos:Concept ;
  rdfs:label "PhysPlaceConcept" ;
  rdfs:comment "Physical feature, defined by its physical characteristics on planet Earth, including mountains, rivers, and oceans. Used in TGN only" ;
  skos:example "Amazon River (TGN)" ;
  dct:description "Physical feature, defined by its physical characteristics on planet Earth, including mountains, rivers, and oceans. Used in TGN only.\nExample: Amazon River (TGN)".

gvp:AdminPlaceConcept a owl:Class ;
  rdfs:isDefinedBy <http://vocab.getty.edu/ontology> ;
  rdfs:subClassOf gvp:Subject, skos:Concept ;
  rdfs:label "AdminPlaceConcept" ;
  rdfs:comment "Place defined by administrative boundaries and conditions, including inhabited places, nations, and empires. Used in TGN only" ;
  skos:example "Burgundy region in France (TGN)" ;
  dct:description "Place defined by administrative boundaries and conditions, including inhabited places, nations, and empires. Used in TGN only.\nExample: Burgundy region in France (TGN)".

gvp:PhysAdminPlaceConcept a owl:Class ;
  rdfs:isDefinedBy <http://vocab.getty.edu/ontology> ;
  rdfs:subClassOf gvp:Subject, skos:Concept ;
  rdfs:label "PhysAdminPlaceConcept" ;
  rdfs:comment "Place that is both administrative and physical. Rarely used. Used in TGN only" ;
  skos:example "6003090 Kiik-Koba (TGN)" ;
  dct:description "Place that is both administrative and physical. Rarely used. Used in TGN only.\nExample: 6003090 Kiik-Koba (TGN)".

gvp:PersonConcept a owl:Class ;
  rdfs:isDefinedBy <http://vocab.getty.edu/ontology> ;
  rdfs:subClassOf gvp:Subject, skos:Concept ;
  rdfs:label "PersonConcept" ;
  rdfs:comment "A single individual. Usually people engaged in the design or creation of art or architecture (\"Artists\"); but may also include donors, patrons, rulers, sitters, art historians, etc (\"Non-Artists\")" ;
  skos:example "500115493 Duerer, Albrecht (ULAN)" ;
  dct:description "A single individual. Usually people engaged in the design or creation of art or architecture (\"Artists\"); but may also include donors, patrons, rulers, sitters, art historians, etc (\"Non-Artists\").\nExample: 500115493 Duerer, Albrecht (ULAN)".

gvp:GroupConcept a owl:Class ;
  rdfs:isDefinedBy <http://vocab.getty.edu/ontology> ;
  rdfs:subClassOf gvp:Subject, skos:Concept ;
  rdfs:label "GroupConcept" ;
  rdfs:comment "Two or more people who generally worked together to collectively create art. Not necessarily legally incorporated. A family of artists may be considered a \"corporate body\". Corresponds to crm:E74_Group, not its subclass crm:E40_Legal_Body" ;
  skos:example "500356337 Albrecht Duerer Workshop (ULAN)" ;
  dct:description "Two or more people who generally worked together to collectively create art. Not necessarily legally incorporated. A family of artists may be considered a \"corporate body\". Corresponds to crm:E74_Group, not its subclass crm:E40_Legal_Body.\nExample: 500356337 Albrecht Duerer Workshop (ULAN)".

gvp:UnknownPersonConcept a owl:Class ;
  rdfs:isDefinedBy <http://vocab.getty.edu/ontology> ;
  rdfs:subClassOf gvp:Subject, skos:Concept ;
  rdfs:label "UnknownPersonConcept" ;
  rdfs:comment "Unknown person representing a nationality/culture (the Unknown People by Culture facet)" ;
  skos:example "500355202 Unknown Bulgarian (modern) (ULAN)" ;
  dct:description "Unknown person representing a nationality/culture (the Unknown People by Culture facet).\nExample: 500355202 Unknown Bulgarian (modern) (ULAN)".

gvp:broaderPreferred a owl:ObjectProperty ;
  rdfs:isDefinedBy <http://vocab.getty.edu/ontology> ;
  rdfs:label "broaderPreferred" ;
  rdfs:domain gvp:Subject ;
  rdfs:range gvp:Subject ;
  rdfs:subPropertyOf gvp:broader ;
  rdfs:comment "Main parent of a subject. Needed to display the hierarchy" ;
  skos:example "Preferred: \"baking dishes\" (AAT) BTG \"bakeware\" (AAT); Sofia (TGN) BTP Bulgaria (TGN)";
  dct:description "Main parent of a subject. Needed to display the hierarchy.\nExample: Preferred: \"baking dishes\" (AAT) BTG \"bakeware\" (AAT); Sofia (TGN) BTP Bulgaria (TGN)" .

gvp:broaderNonPreferred a owl:ObjectProperty ;
  rdfs:isDefinedBy <http://vocab.getty.edu/ontology> ;
  rdfs:label "broaderNonPreferred" ;
  rdfs:domain gvp:Subject ;
  rdfs:range gvp:Subject ;
  rdfs:subPropertyOf gvp:broader ;
  rdfs:comment "Auxiliary parents of a subject. Very often there are several non-preferred parents (poly-hierarchy). Can use to mark such parents with [N] in displays " ;
  skos:example "Non-preferred: \"baking dishes\" BTG \"dishes (vessels)\" (AAT)";
  dct:description "Auxiliary parents of a subject. Very often there are several non-preferred parents (poly-hierarchy). Can use to mark such parents with [N] in displays .\nExample: Non-preferred: \"baking dishes\" BTG \"dishes (vessels)\" (AAT)" .

gvp:broaderGeneric a owl:ObjectProperty ;
  rdfs:isDefinedBy <http://vocab.getty.edu/ontology> ;
  rdfs:label "broaderGeneric" ;
  rdfs:domain gvp:Subject ;
  rdfs:range gvp:Subject ;
  rdfs:subPropertyOf gvp:broader ;
  rdfs:comment "BTG (Genus/Species, \"is a\") relation. We also infer iso-thes:broaderGeneric, which goes only between Concepts" ;
  skos:example "calcite (AAT) BTG mineral (AAT)";
  dct:description "BTG (Genus/Species, \"is a\") relation. We also infer iso-thes:broaderGeneric, which goes only between Concepts.\nExample: calcite (AAT) BTG mineral (AAT)" .

gvp:broaderPartitive a owl:ObjectProperty ;
  rdfs:isDefinedBy <http://vocab.getty.edu/ontology> ;
  rdfs:label "broaderPartitive" ;
  rdfs:domain gvp:Subject ;
  rdfs:range gvp:Subject ;
  rdfs:subPropertyOf gvp:broader ;
  rdfs:comment "BTP (Part/Whole, \"part of\") relation. We also infer iso-thes:broaderPartitive, which goes only between Concepts" ;
  skos:example "Tuscany (TGN) BTP Italy (TGN)";
  dct:description "BTP (Part/Whole, \"part of\") relation. We also infer iso-thes:broaderPartitive, which goes only between Concepts.\nExample: Tuscany (TGN) BTP Italy (TGN)" .

gvp:broaderInstantial a owl:ObjectProperty ;
  rdfs:isDefinedBy <http://vocab.getty.edu/ontology> ;
  rdfs:label "broaderInstantial" ;
  rdfs:domain gvp:Subject ;
  rdfs:range gvp:Subject ;
  rdfs:subPropertyOf gvp:broader ;
  rdfs:comment "BTI (Kind/Instance, \"example of\") relation. We also infer iso-thes:broaderInstantial, which goes only between Concepts" ;
  skos:example "Rembrandt van Rijn BTI Persons/Artists (ULAN)";
  dct:description "BTI (Kind/Instance, \"example of\") relation. We also infer iso-thes:broaderInstantial, which goes only between Concepts.\nExample: Rembrandt van Rijn BTI Persons/Artists (ULAN)" .

gvp:prefLabelGVP a owl:ObjectProperty ;
  rdfs:isDefinedBy <http://vocab.getty.edu/ontology> ;
  rdfs:label "prefLabelGVP" ;
  rdfs:domain gvp:Subject ;
  rdfs:range skosxl:Label ;
  rdfs:comment "Term preferred by the Getty Vocabulary Program. The language is usually English. Applicable to AAT, ULAN, TGN. Used with skosxl:prefLabel";
  dct:description "Term preferred by the Getty Vocabulary Program. The language is usually English. Applicable to AAT, ULAN, TGN. Used with skosxl:prefLabel" .

gvp:prefLabelLoC a owl:ObjectProperty ;
  rdfs:isDefinedBy <http://vocab.getty.edu/ontology> ;
  rdfs:label "prefLabelLoC" ;
  rdfs:domain gvp:Subject ;
  rdfs:range skosxl:Label ;
  rdfs:comment "Term preferred by Library of Congress, thus used for cataloging according to AACR2. Applicable to AAT and ULAN. Used with skosxl:prefLabel";
  dct:description "Term preferred by Library of Congress, thus used for cataloging according to AACR2. Applicable to AAT and ULAN. Used with skosxl:prefLabel" .

gvp:termFlag a owl:ObjectProperty ;
  rdfs:isDefinedBy <http://vocab.getty.edu/ontology> ;
  rdfs:label "termFlag" ;
  rdfs:domain skosxl:Label ;
  rdfs:range skos:Concept;
  dct:description "Term Flag" .

<http://vocab.getty.edu/term/flag/> a skos:ConceptScheme ;
  rdfs:isDefinedBy <http://vocab.getty.edu/ontology> ;
  rdfs:label "Term Flag concept scheme";
  dct:description "Term Flag concept scheme".

<http://vocab.getty.edu/term/flag/Vernacular> a skos:Concept ;
  skos:inScheme <http://vocab.getty.edu/term/flag/> ;
  skos:notation "V" ;
  skos:prefLabel "Vernacular" ;
  skos:scopeNote "Term is the vernacular for a certain place" ;
  skos:example "\"kachoga\" is the Vernacular for 300266169 \"bird-and-flower paintings\" (AAT). \"Firenze\" is the vernacular in Italian (TGN)";
  dct:description "Term is the vernacular for a certain place.\nExample: \"kachoga\" is the Vernacular for 300266169 \"bird-and-flower paintings\" (AAT). \"Firenze\" is the vernacular in Italian (TGN)".

gvp:termKind a owl:ObjectProperty ;
  rdfs:isDefinedBy <http://vocab.getty.edu/ontology> ;
  rdfs:label "termKind" ;
  rdfs:domain skosxl:Label ;
  rdfs:range skos:Concept;
  dct:description "Term Kind" .

<http://vocab.getty.edu/term/kind/> a skos:ConceptScheme ;
  rdfs:isDefinedBy <http://vocab.getty.edu/ontology> ;
  rdfs:label "Term Kind concept scheme";
  dct:description "Term Kind concept scheme".

<http://vocab.getty.edu/term/kind/Abbreviation> a skos:Concept ;
  skos:inScheme <http://vocab.getty.edu/term/kind/> ;
  skos:notation "A" ;
  skos:prefLabel "Abbreviation" ;
  skos:scopeNote "Term is an abbreviation, initialism, or acronym" ;
  skos:example "\"FLIM\" is abbrevaition for \"fluorescence lifetime imaging microscopy\"";
  dct:description "Term is an abbreviation, initialism, or acronym.\nExample: \"FLIM\" is abbrevaition for \"fluorescence lifetime imaging microscopy\"".

<http://vocab.getty.edu/term/kind/CommonTerm> a skos:Concept ;
  skos:inScheme <http://vocab.getty.edu/term/kind/> ;
  skos:notation "C" ;
  skos:prefLabel "Common term" ;
  skos:scopeNote "Preferred common language term. Used for subjects that also include a Scientific term. Used in AAT only" ;
  skos:example "\"frankincense\" (species) is common term for \"Boswellia sacra\" (species)";
  dct:description "Preferred common language term. Used for subjects that also include a Scientific term. Used in AAT only.\nExample: \"frankincense\" (species) is common term for \"Boswellia sacra\" (species)".

<http://vocab.getty.edu/term/kind/ChemicalName> a skos:Concept ;
  skos:inScheme <http://vocab.getty.edu/term/kind/> ;
  skos:notation "CN" ;
  skos:prefLabel "Chemical Name" ;
  skos:scopeNote "Term is the chemical name for the descriptor. Used in AAT only" ;
  skos:example "\"sodium tetraborate decahydrate\" is chemical name for \"borax\"";
  dct:description "Term is the chemical name for the descriptor. Used in AAT only.\nExample: \"sodium tetraborate decahydrate\" is chemical name for \"borax\"".

<http://vocab.getty.edu/term/kind/FullTerm> a skos:Concept ;
  skos:inScheme <http://vocab.getty.edu/term/kind/> ;
  skos:notation "F" ;
  skos:prefLabel "Full term" ;
  skos:scopeNote "Full-form term. Used when the descriptor is a shorter form, or the subject also includes an Abbreviation. Used in AAT only" ;
  skos:example "\"Extensible Markup Language\" is the full term for \"XML\" (which is preferred)";
  dct:description "Full-form term. Used when the descriptor is a shorter form, or the subject also includes an Abbreviation. Used in AAT only.\nExample: \"Extensible Markup Language\" is the full term for \"XML\" (which is preferred)".

<http://vocab.getty.edu/term/kind/JargonOrSlang> a skos:Concept ;
  skos:inScheme <http://vocab.getty.edu/term/kind/> ;
  skos:notation "J" ;
  skos:prefLabel "Jargon or Slang" ;
  skos:scopeNote "Slang or jargon term. Used in AAT only" ;
  skos:example "\"fool's gold\" is slang for \"pyrite\"";
  dct:description "Slang or jargon term. Used in AAT only.\nExample: \"fool's gold\" is slang for \"pyrite\"".

<http://vocab.getty.edu/term/kind/Neologism> a skos:Concept ;
  skos:inScheme <http://vocab.getty.edu/term/kind/> ;
  skos:notation "N" ;
  skos:prefLabel "Neologism" ;
  skos:scopeNote "Term that is new to the language, generally having been coined due to new technology. Used in AAT only." ;
  skos:example "\"folksonomy\", \"podcasting\"";
  dct:description "Term that is new to the language, generally having been coined due to new technology. Used in AAT only..\nExample: \"folksonomy\", \"podcasting\"".

<http://vocab.getty.edu/term/kind/ScientificOrTechnical> a skos:Concept ;
  skos:inScheme <http://vocab.getty.edu/term/kind/> ;
  skos:notation "S" ;
  skos:prefLabel "Scientific or Technical term" ;
  skos:scopeNote "Scientific taxon name (genus, species, etc). Used in AAT only. All such are emitted marked with English language, and most have the same string marked with Latin" ;
  skos:example "\"Boswellia sacra\"@la, also emitted as \"Boswellia sacra\"@en, is scientific name of \"frankincense\"";
  dct:description "Scientific taxon name (genus, species, etc). Used in AAT only. All such are emitted marked with English language, and most have the same string marked with Latin.\nExample: \"Boswellia sacra\"@la, also emitted as \"Boswellia sacra\"@en, is scientific name of \"frankincense\"".

<http://vocab.getty.edu/term/kind/FIPSCode> a skos:Concept ;
  skos:inScheme <http://vocab.getty.edu/term/kind/> ;
  skos:notation "FIPS" ;
  skos:prefLabel "FIPS Code" ;
  skos:scopeNote "FIPS region code. Used in TGN" ;
  skos:example "\"MX21\" for Puebla, Mexico";
  dct:description "FIPS region code. Used in TGN.\nExample: \"MX21\" for Puebla, Mexico".

<http://vocab.getty.edu/term/kind/ISOalpha2> a skos:Concept ;
  skos:inScheme <http://vocab.getty.edu/term/kind/> ;
  skos:notation "ISO2L" ;
  skos:prefLabel "ISO alpha-2 code" ;
  skos:scopeNote "ISO 3166-1 alpha-2 country code. Used in TGN" ;
  skos:example "\"AQ\" for Antarctica";
  dct:description "ISO 3166-1 alpha-2 country code. Used in TGN.\nExample: \"AQ\" for Antarctica".

<http://vocab.getty.edu/term/kind/ISOnumeric2> a skos:Concept ;
  skos:inScheme <http://vocab.getty.edu/term/kind/> ;
  skos:notation "ISO2N" ;
  skos:prefLabel "ISO numeric-2 code" ;
  skos:scopeNote "May be used in TGN, but no code of this kind is present";
  dct:description "May be used in TGN, but no code of this kind is present".

<http://vocab.getty.edu/term/kind/ISOalpha3> a skos:Concept ;
  skos:inScheme <http://vocab.getty.edu/term/kind/> ;
  skos:notation "ISO3L" ;
  skos:prefLabel "ISO alpha-3 code" ;
  skos:scopeNote "ISO 3166-1 alpha-3 country code. Used in TGN" ;
  skos:example "\"ATA\" for Antarctica";
  dct:description "ISO 3166-1 alpha-3 country code. Used in TGN.\nExample: \"ATA\" for Antarctica".

<http://vocab.getty.edu/term/kind/ISOnumeric3> a skos:Concept ;
  skos:inScheme <http://vocab.getty.edu/term/kind/> ;
  skos:notation "ISO3N" ;
  skos:prefLabel "ISO numeric-3 code" ;
  skos:scopeNote "ISO 3166-1 numeric country code as \"ISOnnn\" (though ISO specifies only \"nnn\"). Used in TGN only" ;
  skos:example "\"ISO414\" for Kuwait";
  dct:description "ISO 3166-1 numeric country code as \"ISOnnn\" (though ISO specifies only \"nnn\"). Used in TGN only.\nExample: \"ISO414\" for Kuwait".

<http://vocab.getty.edu/term/kind/OfficialName> a skos:Concept ;
  skos:inScheme <http://vocab.getty.edu/term/kind/> ;
  skos:notation "O" ;
  skos:prefLabel "Official Name" ;
  skos:scopeNote "Used in TGN and ULAN" ;
  skos:example "\"Noyen-sur-Seine\" is official name of 7030197 \"Noyen\" (TGN)";
  dct:description "Used in TGN and ULAN.\nExample: \"Noyen-sur-Seine\" is official name of 7030197 \"Noyen\" (TGN)".

<http://vocab.getty.edu/term/kind/Pseudonym> a skos:Concept ;
  skos:inScheme <http://vocab.getty.edu/term/kind/> ;
  skos:notation "P" ;
  skos:prefLabel "Pseudonym" ;
  skos:scopeNote "Used in TGN and ULAN" ;
  skos:example "\"Frisco\" is nickname for San Francisco (TGN)";
  dct:description "Used in TGN and ULAN.\nExample: \"Frisco\" is nickname for San Francisco (TGN)".

<http://vocab.getty.edu/term/kind/ProvisionalName> a skos:Concept ;
  skos:inScheme <http://vocab.getty.edu/term/kind/> ;
  skos:notation "PN" ;
  skos:prefLabel "Provisional Name" ;
  skos:scopeNote "Used in TGN only" ;
  skos:example "\"Rockton\" was provisional name considered before adoption of \"Kent\" (Ohio)";
  dct:description "Used in TGN only.\nExample: \"Rockton\" was provisional name considered before adoption of \"Kent\" (Ohio)".

<http://vocab.getty.edu/term/kind/SiteName> a skos:Concept ;
  skos:inScheme <http://vocab.getty.edu/term/kind/> ;
  skos:notation "S" ;
  skos:prefLabel "Site Name" ;
  skos:scopeNote "Used in TGN only" ;
  skos:example "\"Flavia Solva\", a deserted settlement and archaeological site (TGN)";
  dct:description "Used in TGN only.\nExample: \"Flavia Solva\", a deserted settlement and archaeological site (TGN)".

<http://vocab.getty.edu/term/kind/USPSCode> a skos:Concept ;
  skos:inScheme <http://vocab.getty.edu/term/kind/> ;
  skos:notation "USPS" ;
  skos:prefLabel "US Postal Service Code" ;
  skos:scopeNote "Used in TGN only" ;
  skos:example "\"CA\" for California";
  dct:description "Used in TGN only.\nExample: \"CA\" for California".

<http://vocab.getty.edu/term/kind/BirthName> a skos:Concept ;
  skos:inScheme <http://vocab.getty.edu/term/kind/> ;
  skos:notation "BN" ;
  skos:prefLabel "Birth Name" ;
  skos:scopeNote "Birth Name of an ULAN agent" ;
  skos:example "TODO";
  dct:description "Birth Name of an ULAN agent.\nExample: TODO".

<http://vocab.getty.edu/term/kind/CommonName> a skos:Concept ;
  skos:inScheme <http://vocab.getty.edu/term/kind/> ;
  skos:notation "CN" ;
  skos:prefLabel "Common Name" ;
  skos:scopeNote "Common Name of an ULAN agent" ;
  skos:example "TODO";
  dct:description "Common Name of an ULAN agent.\nExample: TODO".

<http://vocab.getty.edu/term/kind/FullName> a skos:Concept ;
  skos:inScheme <http://vocab.getty.edu/term/kind/> ;
  skos:notation "FN" ;
  skos:prefLabel "Full Name" ;
  skos:scopeNote "Full Name of an ULAN agent" ;
  skos:example "TODO";
  dct:description "Full Name of an ULAN agent.\nExample: TODO".

gvp:termDisplay a owl:ObjectProperty ;
  rdfs:isDefinedBy <http://vocab.getty.edu/ontology> ;
  rdfs:label "termDisplay" ;
  rdfs:domain skosxl:Label ;
  rdfs:range skos:Concept;
  dct:description "Term Display" .

<http://vocab.getty.edu/term/display/> a skos:ConceptScheme ;
  rdfs:isDefinedBy <http://vocab.getty.edu/ontology> ;
  rdfs:label "Term Display concept scheme";
  dct:description "Term Display concept scheme".

<http://vocab.getty.edu/term/display/Display> a skos:Concept ;
  skos:inScheme <http://vocab.getty.edu/term/display/> ;
  skos:notation "D" ;
  skos:prefLabel "Use for Display" ;
  skos:scopeNote "Use in displays where natural order is appropriate";
  dct:description "Use in displays where natural order is appropriate".

<http://vocab.getty.edu/term/display/Display> a skos:Concept ;
  skos:inScheme <http://vocab.getty.edu/term/display/> ;
  skos:notation "Y" ;
  skos:prefLabel "Use for Display" ;
  skos:scopeNote "Use in displays where natural order is appropriate";
  dct:description "Use in displays where natural order is appropriate".

<http://vocab.getty.edu/term/display/Indexing> a skos:Concept ;
  skos:inScheme <http://vocab.getty.edu/term/display/> ;
  skos:notation "I" ;
  skos:prefLabel "Use in Indexes/lists" ;
  skos:scopeNote "Use in indexes or permuted lists where inverted order is appropriate";
  dct:description "Use in indexes or permuted lists where inverted order is appropriate".

gvp:historicFlag a owl:ObjectProperty ;
  rdfs:isDefinedBy <http://vocab.getty.edu/ontology> ;
  rdfs:label "historicFlag" ;
  rdfs:range skos:Concept;
  dct:description "Historic Flag" .

<http://vocab.getty.edu/historic/> a skos:ConceptScheme ;
  rdfs:isDefinedBy <http://vocab.getty.edu/ontology> ;
  rdfs:label "Historic Flag concept scheme";
  dct:description "Historic Flag concept scheme".

<http://vocab.getty.edu/historic/current> a skos:Concept ;
  skos:inScheme <http://vocab.getty.edu/historic/> ;
  skos:notation "C" ;
  skos:prefLabel "Current" ;
  skos:scopeNote "Valid/used currently";
  dct:description "Valid/used currently".

<http://vocab.getty.edu/historic/historic> a skos:Concept ;
  skos:inScheme <http://vocab.getty.edu/historic/> ;
  skos:notation "H" ;
  skos:prefLabel "Historic" ;
  skos:scopeNote "Valid/used in the past but not currently" ;
  skos:example "\"Lutetia\" is a historic name for \"Paris\" (TGN). \"weyneschot\" is a 16th-century spelling for \"wainscoting\" (AAT)";
  dct:description "Valid/used in the past but not currently.\nExample: \"Lutetia\" is a historic name for \"Paris\" (TGN). \"weyneschot\" is a 16th-century spelling for \"wainscoting\" (AAT)".

<http://vocab.getty.edu/historic/currentAndHistoric> a skos:Concept ;
  skos:inScheme <http://vocab.getty.edu/historic/> ;
  skos:notation "B" ;
  skos:prefLabel "Both Current and Historic" ;
  skos:scopeNote "Valid/used both in the past and currently" ;
  skos:example "Saint Petersburg (TGN)";
  dct:description "Valid/used both in the past and currently.\nExample: Saint Petersburg (TGN)".

<http://vocab.getty.edu/historic/localUse> a skos:Concept ;
  skos:inScheme <http://vocab.getty.edu/historic/> ;
  skos:notation "LU" ;
  skos:prefLabel "Local Use" ;
  skos:scopeNote "Used locally for Unidentified Named People mentioned in some document (ULAN only)" ;
  skos:example "500051176 Abinetti (ULAN) is an unknown artist mentioned in documentation of lot 209 of an auction held 29 Jan 1824 in London";
  dct:description "Used locally for Unidentified Named People mentioned in some document (ULAN only).\nExample: 500051176 Abinetti (ULAN) is an unknown artist mentioned in documentation of lot 209 of an auction held 29 Jan 1824 in London".

gvp:termType a owl:ObjectProperty ;
  rdfs:isDefinedBy <http://vocab.getty.edu/ontology> ;
  rdfs:label "termType" ;
  rdfs:domain skosxl:Label ;
  rdfs:range skos:Concept;
  dct:description "Term Type" .

<http://vocab.getty.edu/term/type/> a skos:ConceptScheme ;
  rdfs:isDefinedBy <http://vocab.getty.edu/ontology> ;
  rdfs:label "Term Type concept scheme";
  dct:description "Term Type concept scheme".

<http://vocab.getty.edu/term/type/Descriptor> a skos:Concept ;
  skos:inScheme <http://vocab.getty.edu/term/type/> ;
  skos:notation "D" ;
  skos:prefLabel "Descriptor" ;
  skos:scopeNote "Main term. Getty usually uses the plural" ;
  skos:example "\"manuscripts\" (English)";
  dct:description "Main term. Getty usually uses the plural.\nExample: \"manuscripts\" (English)".

<http://vocab.getty.edu/term/type/AlternateDescriptor> a skos:Concept ;
  skos:inScheme <http://vocab.getty.edu/term/type/> ;
  skos:notation "AD" ;
  skos:prefLabel "Alternate Descriptor" ;
  skos:scopeNote "A lexical variant, eg singular" ;
  skos:example "\"manuscript\" (English) instead of \"manuscripts\"";
  dct:description "A lexical variant, eg singular.\nExample: \"manuscript\" (English) instead of \"manuscripts\"".

<http://vocab.getty.edu/term/type/UsedForTerm> a skos:Concept ;
  skos:inScheme <http://vocab.getty.edu/term/type/> ;
  skos:notation "UF" ;
  skos:prefLabel "Used for Term" ;
  skos:scopeNote "A synonym" ;
  skos:example "\"handschriften\" (Dutch) instead of \"manuscripten\"";
  dct:description "A synonym.\nExample: \"handschriften\" (Dutch) instead of \"manuscripten\"".

gvp:termPOS a owl:ObjectProperty ;
  rdfs:isDefinedBy <http://vocab.getty.edu/ontology> ;
  rdfs:label "termPOS" ;
  rdfs:domain skosxl:Label ;
  rdfs:range skos:Concept;
  dct:description "Part of Speech" .

<http://vocab.getty.edu/term/POS/> a skos:ConceptScheme ;
  rdfs:isDefinedBy <http://vocab.getty.edu/ontology> ;
  rdfs:label "Part of Speech concept scheme";
  dct:description "Part of Speech concept scheme".

<http://vocab.getty.edu/term/POS/PluralNoun> a skos:Concept ;
  skos:inScheme <http://vocab.getty.edu/term/POS/> ;
  skos:notation "PN" ;
  skos:prefLabel "Plural Noun" ;
  skos:scopeNote "A term that is plural (the same word may be singular in another language)" ;
  skos:example "\"filigrane\" is the Italian plural for \"watermarks\"";
  dct:description "A term that is plural (the same word may be singular in another language).\nExample: \"filigrane\" is the Italian plural for \"watermarks\"".

<http://vocab.getty.edu/term/POS/SingularNoun> a skos:Concept ;
  skos:inScheme <http://vocab.getty.edu/term/POS/> ;
  skos:notation "SN" ;
  skos:prefLabel "Singular Noun" ;
  skos:scopeNote "A term that is singular (the same word may be plural in another language)" ;
  skos:example "\"filigrane\" is the French singular for \"watermark\"";
  dct:description "A term that is singular (the same word may be plural in another language).\nExample: \"filigrane\" is the French singular for \"watermark\"".

<http://vocab.getty.edu/term/POS/BothSingularAndPlural> a skos:Concept ;
  skos:inScheme <http://vocab.getty.edu/term/POS/> ;
  skos:notation "B" ;
  skos:prefLabel "Both Singular and Plural" ;
  skos:scopeNote "A term that is used for both the singular and plural in the same language" ;
  skos:example "\"chassis\" is both singular and plural in French";
  dct:description "A term that is used for both the singular and plural in the same language.\nExample: \"chassis\" is both singular and plural in French".

<http://vocab.getty.edu/term/POS/PastParticiple> a skos:Concept ;
  skos:inScheme <http://vocab.getty.edu/term/POS/> ;
  skos:notation "PP" ;
  skos:prefLabel "Past Participle" ;
  skos:scopeNote "Rarely used but if at all, is most likely to apply in Attributes and Properties" ;
  skos:example "hand-painted";
  dct:description "Rarely used but if at all, is most likely to apply in Attributes and Properties.\nExample: hand-painted".

<http://vocab.getty.edu/term/POS/VerbalNounGerund> a skos:Concept ;
  skos:inScheme <http://vocab.getty.edu/term/POS/> ;
  skos:notation "VN" ;
  skos:prefLabel "Verbal Noun/Gerund" ;
  skos:scopeNote "Term is a verbal noun or gerund" ;
  skos:example "polishing";
  dct:description "Term is a verbal noun or gerund.\nExample: polishing".

<http://vocab.getty.edu/term/POS/Adjectival> a skos:Concept ;
  skos:inScheme <http://vocab.getty.edu/term/POS/> ;
  skos:notation "A" ;
  skos:prefLabel "Adjectival" ;
  skos:scopeNote "This term may be combined with others in post-coordinated compound terms" ;
  skos:example "\"Renaissance\" (as in \"Renaissance cathedral\"), \"painter's\" (as in \"painter's smock\")";
  dct:description "This term may be combined with others in post-coordinated compound terms.\nExample: \"Renaissance\" (as in \"Renaissance cathedral\"), \"painter's\" (as in \"painter's smock\")".

<http://vocab.getty.edu/term/POS/Noun> a skos:Concept ;
  skos:inScheme <http://vocab.getty.edu/term/POS/> ;
  skos:notation "N" ;
  skos:prefLabel "Noun" ;
  skos:scopeNote "Term is a noun but we are uncertain if it is plural or singular" ;
  skos:example "Panthera leo";
  dct:description "Term is a noun but we are uncertain if it is plural or singular.\nExample: Panthera leo".

<http://vocab.getty.edu/term/flag/LoanTerm> a skos:Concept ;
  skos:inScheme <http://vocab.getty.edu/term/flag/> ;
  skos:notation "L" ;
  skos:prefLabel "Loan Term" ;
  skos:scopeNote "Term borrowed from another language that has become naturalized in American English" ;
  skos:example "papier mache";
  dct:description "Term borrowed from another language that has become naturalized in American English.\nExample: papier mache".

<http://vocab.getty.edu/term/flag/LiteralTranslation> a skos:Concept ;
  skos:inScheme <http://vocab.getty.edu/term/flag/> ;
  skos:notation "T" ;
  skos:prefLabel "Literal Translation" ;
  skos:scopeNote "Literal translation of a name.  Defined for ULAN, but currently there are no examples of this";
  dct:description "Literal translation of a name.  Defined for ULAN, but currently there are no examples of this".

<http://vocab.getty.edu/term/kind/Code> a skos:Concept ;
  skos:inScheme <http://vocab.getty.edu/term/kind/> ;
  skos:notation "79000" ;
  skos:prefLabel "Code" ;
  skos:scopeNote "Code, similar to Abbreviation" ;
  skos:example "\"sq yds\", \"m2\"";
  dct:description "Code, similar to Abbreviation.\nExample: \"sq yds\", \"m2\"".

gvp:contributorPreferred a owl:ObjectProperty ;
  rdfs:isDefinedBy <http://vocab.getty.edu/ontology> ;
  rdfs:label "contributorPreferred" ;
  rdfs:domain skosxl:Label ;
  rdfs:range foaf:Agent ;
  rdfs:subPropertyOf dct:contributor ;
  rdfs:comment "Contributor for which the term is Preferred. Range is foaf:Agent" ;
  skos:example "\"organza\" is preferred term for WHS";
  dct:description "Contributor for which the term is Preferred. Range is foaf:Agent.\nExample: \"organza\" is preferred term for WHS" .

gvp:contributorNonPreferred a owl:ObjectProperty ;
  rdfs:isDefinedBy <http://vocab.getty.edu/ontology> ;
  rdfs:label "contributorNonPreferred" ;
  rdfs:domain skosxl:Label ;
  rdfs:range foaf:Agent ;
  rdfs:subPropertyOf dct:contributor ;
  rdfs:comment "Contributor for which the term is Non-preferred. Range is foaf:Agent" ;
  skos:example "\"Lycra\" is non-preferred term for WHS";
  dct:description "Contributor for which the term is Non-preferred. Range is foaf:Agent.\nExample: \"Lycra\" is non-preferred term for WHS" .

gvp:contributorAlternatePreferred a owl:ObjectProperty ;
  rdfs:isDefinedBy <http://vocab.getty.edu/ontology> ;
  rdfs:label "contributorAlternatePreferred" ;
  rdfs:domain skosxl:Label ;
  rdfs:range foaf:Agent ;
  rdfs:subPropertyOf dct:contributor ;
  rdfs:comment "Contributor for which the term is Alternate Preferred. Range is foaf:Agent";
  dct:description "Contributor for which the term is Alternate Preferred. Range is foaf:Agent" .

gvp:sourcePreferred a owl:ObjectProperty ;
  rdfs:isDefinedBy <http://vocab.getty.edu/ontology> ;
  rdfs:label "sourcePreferred" ;
  rdfs:domain skosxl:Label ;
  rdfs:range bibo:Document ;
  rdfs:subPropertyOf dct:source ;
  rdfs:comment "Source for which the term is Preferred. Range is bibo:Document or bibo:DocumentPart" ;
  skos:example "\"Isfahan\" is preferred in Webster's New Geographical Dictionary (1988)";
  dct:description "Source for which the term is Preferred. Range is bibo:Document or bibo:DocumentPart.\nExample: \"Isfahan\" is preferred in Webster's New Geographical Dictionary (1988)" .

gvp:sourceNonPreferred a owl:ObjectProperty ;
  rdfs:isDefinedBy <http://vocab.getty.edu/ontology> ;
  rdfs:label "sourceNonPreferred" ;
  rdfs:domain skosxl:Label ;
  rdfs:range bibo:Document ;
  rdfs:subPropertyOf dct:source ;
  rdfs:comment "Source for which the term is Non-preferred. Range is bibo:Document or bibo:DocumentPart" ;
  skos:example "\"Panderma\" is non-preferred in Webster's New Geographical Dictionary (1988)";
  dct:description "Source for which the term is Non-preferred. Range is bibo:Document or bibo:DocumentPart.\nExample: \"Panderma\" is non-preferred in Webster's New Geographical Dictionary (1988)" .

gvp:sourceAlternatePreferred a owl:ObjectProperty ;
  rdfs:isDefinedBy <http://vocab.getty.edu/ontology> ;
  rdfs:label "sourceAlternatePreferred" ;
  rdfs:domain skosxl:Label ;
  rdfs:range bibo:Document ;
  rdfs:subPropertyOf dct:source ;
  rdfs:comment "Source for which the term is Alternate Preferred. Range is bibo:Document or bibo:DocumentPart" ;
  skos:example "\"Kayseri\" is alternate preferred in Webster's New Geographical Dictionary (1988)";
  dct:description "Source for which the term is Alternate Preferred. Range is bibo:Document or bibo:DocumentPart.\nExample: \"Kayseri\" is alternate preferred in Webster's New Geographical Dictionary (1988)" .

gvp:placeTypePreferred a owl:ObjectProperty ;
  rdfs:isDefinedBy <http://vocab.getty.edu/ontology> ;
  rdfs:label "placeTypePreferred" ;
  rdfs:domain gvp:Subject ;
  rdfs:range gvp:Subject ;
  rdfs:subPropertyOf gvp:placeType ;
  rdfs:comment "The primary type of a TGN Place. Domain is TGN concept, range is AAT concept" ;
  skos:example "The preferred place type of Machupicchu, Peru is \"deserted settlement\" (current)";
  dct:description "The primary type of a TGN Place. Domain is TGN concept, range is AAT concept.\nExample: The preferred place type of Machupicchu, Peru is \"deserted settlement\" (current)" .

gvp:placeTypeNonPreferred a owl:ObjectProperty ;
  rdfs:isDefinedBy <http://vocab.getty.edu/ontology> ;
  rdfs:label "placeTypeNonPreferred" ;
  rdfs:domain gvp:Subject ;
  rdfs:range gvp:Subject ;
  rdfs:subPropertyOf gvp:placeType ;
  rdfs:comment "A secondary type for a TGN Place. Domain is TGN concept, range is AAT concept" ;
  skos:example "A non-preferred type of Machupicchu, Peru is \"Inca center\" (historical)";
  dct:description "A secondary type for a TGN Place. Domain is TGN concept, range is AAT concept.\nExample: A non-preferred type of Machupicchu, Peru is \"Inca center\" (historical)" .

gvp:agentTypePreferred a owl:ObjectProperty ;
  rdfs:isDefinedBy <http://vocab.getty.edu/ontology> ;
  rdfs:label "agentTypePreferred" ;
  rdfs:domain gvp:Subject ;
  rdfs:range gvp:Subject ;
  rdfs:subPropertyOf gvp:agentType ;
  rdfs:comment "The primary type of a ULAN Person or Corporate body. Domain is ULAN concept, range is AAT concept" ;
  skos:example "The preferred type of \"Albrecht Duerer Workshop\" (ULAN) is \"workshop\" (AAT)";
  dct:description "The primary type of a ULAN Person or Corporate body. Domain is ULAN concept, range is AAT concept.\nExample: The preferred type of \"Albrecht Duerer Workshop\" (ULAN) is \"workshop\" (AAT)" .

gvp:agentTypeNonPreferred a owl:ObjectProperty ;
  rdfs:isDefinedBy <http://vocab.getty.edu/ontology> ;
  rdfs:label "agentTypeNonPreferred" ;
  rdfs:domain gvp:Subject ;
  rdfs:range gvp:Subject ;
  rdfs:subPropertyOf gvp:agentType ;
  rdfs:comment "A secondary type of a ULAN Person or Corporate body. Domain is ULAN concept, range is AAT concept" ;
  skos:example "Non-preferred types of \"Albrecht Duerer Workshop\" (ULAN) include \"printmakers\" and painters\" (AAT)";
  dct:description "A secondary type of a ULAN Person or Corporate body. Domain is ULAN concept, range is AAT concept.\nExample: Non-preferred types of \"Albrecht Duerer Workshop\" (ULAN) include \"printmakers\" and painters\" (AAT)" .

gvp:biographyPreferred a owl:ObjectProperty ;
  rdfs:isDefinedBy <http://vocab.getty.edu/ontology> ;
  rdfs:label "biographyPreferred" ;
  rdfs:range gvp:Biography ;
  rdfs:subPropertyOf gvp:biography ;
  rdfs:comment "Preferred biography of an ULAN agent. Domain is schema:Person/Organization, range is gvp:Biography. The biography fields are also directly available in the Person/Organization";
  dct:description "Preferred biography of an ULAN agent. Domain is schema:Person/Organization, range is gvp:Biography. The biography fields are also directly available in the Person/Organization" .

gvp:biographyNonPreferred a owl:ObjectProperty ;
  rdfs:isDefinedBy <http://vocab.getty.edu/ontology> ;
  rdfs:label "biographyNonPreferred" ;
  rdfs:range gvp:Biography ;
  rdfs:subPropertyOf gvp:biography ;
  rdfs:comment "Non-preferred biography of an ULAN agent. Domain is schema:Person/Organization, range is gvp:Biography";
  dct:description "Non-preferred biography of an ULAN agent. Domain is schema:Person/Organization, range is gvp:Biography" .

gvp:eventPreferred a owl:ObjectProperty ;
  rdfs:isDefinedBy <http://vocab.getty.edu/ontology> ;
  rdfs:label "eventPreferred" ;
  rdfs:range bio:Event ;
  rdfs:subPropertyOf bio:event ;
  rdfs:comment "Preferred life event of an ULAN agent. Domain is schema:Person/Organization, range is bio:Event";
  dct:description "Preferred life event of an ULAN agent. Domain is schema:Person/Organization, range is bio:Event" .

gvp:eventNonPreferred a owl:ObjectProperty ;
  rdfs:isDefinedBy <http://vocab.getty.edu/ontology> ;
  rdfs:label "eventNonPreferred" ;
  rdfs:range bio:Event ;
  rdfs:subPropertyOf bio:event ;
  rdfs:comment "Non-preferred life event of an ULAN agent. Domain is schema:Person/Organization, range is bio:Event";
  dct:description "Non-preferred life event of an ULAN agent. Domain is schema:Person/Organization, range is bio:Event" .

gvp:nationalityPreferred a owl:ObjectProperty ;
  rdfs:isDefinedBy <http://vocab.getty.edu/ontology> ;
  rdfs:label "nationalityPreferred" ;
  rdfs:range gvp:Subject ;
  rdfs:subPropertyOf schema:nationality ;
  rdfs:comment "Preferred nationality/culture/race/ethnicity/religion/sexual orientation of an ULAN agent. Domain is schema:Person/Organization, range is AAT concept";
  dct:description "Preferred nationality/culture/race/ethnicity/religion/sexual orientation of an ULAN agent. Domain is schema:Person/Organization, range is AAT concept" .

gvp:nationalityNonPreferred a owl:ObjectProperty ;
  rdfs:isDefinedBy <http://vocab.getty.edu/ontology> ;
  rdfs:label "nationalityNonPreferred" ;
  rdfs:range gvp:Subject ;
  rdfs:subPropertyOf schema:nationality ;
  rdfs:comment "Non-preferred nationality/culture/race/ethnicity/religion/sexual orientation of an ULAN agent. Domain is schema:Person/Organization, range is AAT concept";
  dct:description "Non-preferred nationality/culture/race/ethnicity/religion/sexual orientation of an ULAN agent. Domain is schema:Person/Organization, range is AAT concept" .

#################### Associative Relations: skos:related sub-properties defined from assoc-rels.xls ####################


gvp:aat2000_related_to a owl:ObjectProperty;
  rdfs:isDefinedBy <http://vocab.getty.edu/ontology>, aat: ;
  rdfs:subPropertyOf skos:related;
  rdfs:domain skos:Concept; rdfs:range skos:Concept;
  # domain "any"; range "any";
  dc:identifier "2000";
  skos:prefLabel "aat2000_related_to";
  dc:title "related to - any";
  skos:example "gulf red is related to light red (pigment)";
  skos:scopeNote "generic relationship, not explained" ;
  dct:description """any - related to - any; generic relationship, not explained.
Example: gulf red is related to light red (pigment)""" .
gvp:aat2000_related_to a owl:SymmetricProperty.


gvp:aat2001_formerly_referred_to a owl:ObjectProperty;
  rdfs:isDefinedBy <http://vocab.getty.edu/ontology>, aat: ;
  rdfs:subPropertyOf skos:related;
  rdfs:domain skos:Concept; rdfs:range skos:Concept;
  # domain "any"; range "any";
  dc:identifier "2001";
  skos:prefLabel "aat2001_formerly_referred_to";
  dc:title "formerly referred to - any";
  skos:example "gigues formerly referred to fiddles" ;
  dct:description """any - formerly referred - any.
Example: gigues formerly referred to fiddles""" .
gvp:aat2001_formerly_referred_to a owl:SymmetricProperty.


gvp:aat2100_distinguished_from a owl:ObjectProperty;
  rdfs:isDefinedBy <http://vocab.getty.edu/ontology>, aat: ;
  rdfs:subPropertyOf skos:related;
  rdfs:domain skos:Concept; rdfs:range skos:Concept;
  # domain "any"; range "any";
  dc:identifier "2100";
  skos:prefLabel "aat2100_distinguished_from";
  dc:title "distinguished from - any";
  skos:example "historic farms are distinguished from abandoned farms",
    "naive art is distinguished from outsider art" ;
  dct:description """any - distinguished from - any.
Example: historic farms are distinguished from abandoned farms; naive art is distinguished from outsider art""" .
gvp:aat2100_distinguished_from a owl:SymmetricProperty.


gvp:aat2110_meaning-usage_overlaps_with a owl:ObjectProperty;
  rdfs:isDefinedBy <http://vocab.getty.edu/ontology>, aat: ;
  rdfs:subPropertyOf skos:related;
  rdfs:domain skos:Concept; rdfs:range skos:Concept;
  # domain "any"; range "any";
  dc:identifier "2110";
  skos:prefLabel "aat2110_meaning-usage_overlaps_with";
  dc:title "meaning/usage overlaps with - any";
  skos:example "chimney hoods has meaning/usage that overlaps with chimney caps",
    "scribes has meaning/usage that overlaps with copyists" ;
  dct:description """any - meaning/usage overlaps with - any.
Example: chimney hoods has meaning/usage that overlaps with chimney caps; scribes has meaning/usage that overlaps with copyists""" .
gvp:aat2110_meaning-usage_overlaps_with a owl:SymmetricProperty.


gvp:aat2203_associated_with a owl:ObjectProperty;
  rdfs:isDefinedBy <http://vocab.getty.edu/ontology>, aat: ;
  rdfs:subPropertyOf skos:related;
  rdfs:domain skos:Concept; rdfs:range skos:Concept;
  # domain "activity/event"; range "activity/event";
  dc:identifier "2203";
  skos:prefLabel "aat2203_associated_with";
  dc:title "associated with - activity/event";
  skos:example "Easter is associated with Lent",
    "cavalry exercises are associated with dressage" ;
  dct:description """activity/event/[process/function] - [is] associated with - activity/event/[process/function].
Example: Easter is associated with Lent; cavalry exercises are associated with dressage""" .
gvp:aat2203_associated_with a owl:SymmetricProperty.


gvp:aat2205_causes-is_required a owl:ObjectProperty;
  rdfs:isDefinedBy <http://vocab.getty.edu/ontology>, aat: ;
  rdfs:subPropertyOf skos:related;
  rdfs:domain skos:Concept; rdfs:range skos:Concept;
  # domain "activity/event"; range "activity/event";
  dc:identifier "2205";
  skos:prefLabel "aat2205_causes-is_required";
  dc:title "causes/is required - activity/event";
  skos:example "on-demand printing causes/is required for on-demand publishing",
    "preserving causes/is required for preservation" ;
  dct:description """activity/event/[process/function] - causes/is required for - activity/event/[process/function].
Example: on-demand printing causes/is required for on-demand publishing;  preserving causes/is required for preservation""" .


gvp:aat2206_caused_by-requires a owl:ObjectProperty;
  rdfs:isDefinedBy <http://vocab.getty.edu/ontology>, aat: ;
  rdfs:subPropertyOf skos:related;
  rdfs:domain skos:Concept; rdfs:range skos:Concept;
  # domain "activity/event"; range "activity/event";
  dc:identifier "2206";
  skos:prefLabel "aat2206_caused_by-requires";
  dc:title "caused by/requires - activity/event";
  skos:example "on-demand publishing is caused by/requires on-demand printing",
    "preservation is caused by/requires preserving" ;
  dct:description """activity/event/[process/function] - [is] caused by/dependent upon - activity/event/[process/function].
Example: on-demand publishing is caused by/requires on-demand printing; preservation is caused by/requires preserving""" .
gvp:aat2205_causes-is_required owl:inverseOf gvp:aat2206_caused_by-requires.


gvp:aat2208_locus-setting_for a owl:ObjectProperty;
  rdfs:isDefinedBy <http://vocab.getty.edu/ontology>, aat: ;
  rdfs:subPropertyOf skos:related;
  rdfs:domain skos:Concept; rdfs:range skos:Concept;
  # domain "locus/setting"; range "things";
  dc:identifier "2208";
  skos:prefLabel "aat2208_locus-setting_for";
  dc:title "locus/setting for - things";
  skos:example "glassworks (buildings) are the locus/setting for glassware",
    "caves are the locus/setting for cave paintings" ;
  dct:description """locus/setting - [is] locus/setting for - things.
Example: glassworks (buildings) are the locus/setting for glassware; caves are the locus/setting for cave paintings""" .


gvp:aat2209_used-located_in a owl:ObjectProperty;
  rdfs:isDefinedBy <http://vocab.getty.edu/ontology>, aat: ;
  rdfs:subPropertyOf skos:related;
  rdfs:domain skos:Concept; rdfs:range skos:Concept;
  # domain "things"; range "locus/setting";
  dc:identifier "2209";
  skos:prefLabel "aat2209_used-located_in";
  dc:title "used/located in - locus/setting";
  skos:example "glassware is used/located in glassworks (buildings)",
    "cave paintings are located in caves" ;
  dct:description """things -used/located in -  locus/setting.
Example: glassware is used/located in glassworks (buildings); cave paintings are located in caves""" .
gvp:aat2208_locus-setting_for owl:inverseOf gvp:aat2209_used-located_in.


gvp:aat2211_produce a owl:ObjectProperty;
  rdfs:isDefinedBy <http://vocab.getty.edu/ontology>, aat: ;
  rdfs:subPropertyOf skos:related;
  rdfs:domain skos:Concept; rdfs:range skos:Concept;
  # domain "things"; range "things";
  dc:identifier "2211";
  skos:prefLabel "aat2211_produce";
  dc:title "produce - things";
  skos:example "stereoscopic cameras produce stereoscopic photographs",
    "punches (marking tools) produce punchwork" ;
  dct:description """things/[equipment] - produce - things.
Example: stereoscopic cameras produce stereoscopic photographs; punches (marking tools) produce punchwork""" .


gvp:aat2212_produced_by a owl:ObjectProperty;
  rdfs:isDefinedBy <http://vocab.getty.edu/ontology>, aat: ;
  rdfs:subPropertyOf skos:related;
  rdfs:domain skos:Concept; rdfs:range skos:Concept;
  # domain "things"; range "things";
  dc:identifier "2212";
  skos:prefLabel "aat2212_produced_by";
  dc:title "produced by - things";
  skos:example "stereoscopic photographs are produced by stereoscopic cameras",
    "punchwork is produced by punches (marking tools)" ;
  dct:description """things - [are] produced by - things/[equipment].
Example: stereoscopic photographs are produced by stereoscopic cameras; punchwork is produced by punches (marking tools)""" .
gvp:aat2211_produce owl:inverseOf gvp:aat2212_produced_by.


gvp:aat2215_required_for a owl:ObjectProperty;
  rdfs:isDefinedBy <http://vocab.getty.edu/ontology>, aat: ;
  rdfs:subPropertyOf skos:related;
  rdfs:domain skos:Concept; rdfs:range skos:Concept;
  # domain "things"; range "things";
  dc:identifier "2215";
  skos:prefLabel "aat2215_required_for";
  dc:title "required for - things";
  skos:example "eyelets are required for broderie anglaise",
    "compact discs are required for compact disc players" ;
  dct:description """things - [are] required for -  things.
Example: eyelets are required for broderie anglaise; compact discs are required for compact disc players""" .


gvp:aat2216_require a owl:ObjectProperty;
  rdfs:isDefinedBy <http://vocab.getty.edu/ontology>, aat: ;
  rdfs:subPropertyOf skos:related;
  rdfs:domain skos:Concept; rdfs:range skos:Concept;
  # domain "things"; range "things";
  dc:identifier "2216";
  skos:prefLabel "aat2216_require";
  dc:title "require - things";
  skos:example "broderie anglaise requires eyelets",
    "compact disc players require compact discs" ;
  dct:description """things - require - things [in order to exist or work].
Example: broderie anglaise requires eyelets; compact disc players require compact discs""" .
gvp:aat2215_required_for owl:inverseOf gvp:aat2216_require.


gvp:aat2218_used-function_as a owl:ObjectProperty;
  rdfs:isDefinedBy <http://vocab.getty.edu/ontology>, aat: ;
  rdfs:subPropertyOf skos:related;
  rdfs:domain skos:Concept; rdfs:range skos:Concept;
  # domain "things"; range "things";
  dc:identifier "2218";
  skos:prefLabel "aat2218_used-function_as";
  dc:title "used/function as - things";
  skos:example "arc lamps are used/function as lighthouse lamps",
    "toile peinte is used/function as cartoons (working drawings)" ;
  dct:description """things - [are] used/function as - things.
Example: arc lamps are used/function as lighthouse lamps;  toile peinte is used/function as cartoons (working drawings)""" .


gvp:aat2219_have_form a owl:ObjectProperty;
  rdfs:isDefinedBy <http://vocab.getty.edu/ontology>, aat: ;
  rdfs:subPropertyOf skos:related;
  rdfs:domain skos:Concept; rdfs:range skos:Concept;
  # domain "things"; range "things";
  dc:identifier "2219";
  skos:prefLabel "aat2219_have_form";
  dc:title "have form - things";
  skos:example "lighthouse lamps have the form of arc lamps",
    "cartoons (working drawings) have the form of toile peinte" ;
  dct:description """things - have form [of] - things.
Example: lighthouse lamps have the form of arc lamps; cartoons (working drawings) have the form of toile peinte""" .
gvp:aat2218_used-function_as owl:inverseOf gvp:aat2219_have_form.


gvp:aat2221_act_upon a owl:ObjectProperty;
  rdfs:isDefinedBy <http://vocab.getty.edu/ontology>, aat: ;
  rdfs:subPropertyOf skos:related;
  rdfs:domain skos:Concept; rdfs:range skos:Concept;
  # domain "role"; range "genus/species";
  dc:identifier "2221";
  skos:prefLabel "aat2221_act_upon";
  dc:title "act upon - genus/species";
  skos:example "jockeys act upon Equus caballus(species)",
    "tappers act upon Acer saccharum(species)" ;
  dct:description """[actors having] role - act upon - genus/species.
Example: jockeys act upon Equus caballus(species); tappers act upon Acer saccharum(species)""" .


gvp:aat2222_are_acted_upon a owl:ObjectProperty;
  rdfs:isDefinedBy <http://vocab.getty.edu/ontology>, aat: ;
  rdfs:subPropertyOf skos:related;
  rdfs:domain skos:Concept; rdfs:range skos:Concept;
  # domain "genus/species"; range "role";
  dc:identifier "2222";
  skos:prefLabel "aat2222_are_acted_upon";
  dc:title "are acted upon - role";
  skos:example "Equus caballus(species) is acted upon by jockeys",
    "Acer saccharum(species) is acted upon by tappers" ;
  dct:description """genus/species - is acted upon [by] - [actors having] role.
Example: Equus caballus(species) is acted upon by jockeys; Acer saccharum(species) is acted upon by tappers""" .
gvp:aat2221_act_upon owl:inverseOf gvp:aat2222_are_acted_upon.


gvp:aat2281_have_counterpart a owl:ObjectProperty;
  rdfs:isDefinedBy <http://vocab.getty.edu/ontology>, aat: ;
  rdfs:subPropertyOf skos:related;
  rdfs:domain skos:Concept; rdfs:range skos:Concept;
  # domain "role"; range "role";
  dc:identifier "2281";
  skos:prefLabel "aat2281_have_counterpart";
  dc:title "have counterpart - role";
  skos:example "duchesses have counterpart dukes",
    "godesses have counterpart gods" ;
  dct:description """role -[is] counterpart to - role.
Example: duchesses have counterpart dukes; godesses have counterpart gods""" .
gvp:aat2281_have_counterpart a owl:SymmetricProperty.


gvp:aat2285_practiced-studied_by a owl:ObjectProperty;
  rdfs:isDefinedBy <http://vocab.getty.edu/ontology>, aat: ;
  rdfs:subPropertyOf skos:related;
  rdfs:domain skos:Concept; rdfs:range skos:Concept;
  # domain "field/discipline"; range "role";
  dc:identifier "2285";
  skos:prefLabel "aat2285_practiced-studied_by";
  dc:title "practiced/studied by - role";
  skos:example "Egyptology is practiced/studied by Egyptologists",
    "architectural history is practiced/studied by architectural historians" ;
  dct:description """field [of study, genre]/discipline - [is] practiced/studied by - a role.
Example: Egyptology is practiced/studied by Egyptologists; architectural history is practiced/studied by architectural historians""" .


gvp:aat2286_practice-study a owl:ObjectProperty;
  rdfs:isDefinedBy <http://vocab.getty.edu/ontology>, aat: ;
  rdfs:subPropertyOf skos:related;
  rdfs:domain skos:Concept; rdfs:range skos:Concept;
  # domain "role"; range "field/discipline";
  dc:identifier "2286";
  skos:prefLabel "aat2286_practice-study";
  dc:title "practice/study - field/discipline";
  skos:example "Egyptologists practice/study Egyptology",
    "architectural historians practice/study architectural history" ;
  dct:description """[actor having] role - practice/study - field [of study, genre]/discipline.
Example: Egyptologists practice/study Egyptology; architectural historians practice/study architectural history""" .
gvp:aat2285_practiced-studied_by owl:inverseOf gvp:aat2286_practice-study.


gvp:aat2291_locus-setting_for a owl:ObjectProperty;
  rdfs:isDefinedBy <http://vocab.getty.edu/ontology>, aat: ;
  rdfs:subPropertyOf skos:related;
  rdfs:domain skos:Concept; rdfs:range skos:Concept;
  # domain "locus/setting"; range "role";
  dc:identifier "2291";
  skos:prefLabel "aat2291_locus-setting_for";
  dc:title "locus/setting for - role";
  skos:example "roperies are the locus/setting of rope-makers",
    "convents (built complexes) are the locus/setting of nuns",
    "libraries (buildings) are the locus/setting of libraries (institutions)" ;
  dct:description """locus/setting - [is] locus setting for - [actor or institution having] role.
Example: roperies are the locus/setting of rope-makers; convents (built complexes) are the locus/setting of nuns; libraries (buildings) are the locus/setting of libraries (institutions)""" .


gvp:aat2292_work-live_in a owl:ObjectProperty;
  rdfs:isDefinedBy <http://vocab.getty.edu/ontology>, aat: ;
  rdfs:subPropertyOf skos:related;
  rdfs:domain skos:Concept; rdfs:range skos:Concept;
  # domain "role"; range "locus/setting";
  dc:identifier "2292";
  skos:prefLabel "aat2292_work-live_in";
  dc:title "work/live in - locus/setting";
  skos:example "rope-makers live/work in roperies",
    "nuns live/work in convents (nunneries)",
    "libraries (institutions) live/work in libraries (buildings)" ;
  dct:description """[actor or institution having] role - work/live/[exist] in - locus/setting.
Example: rope-makers live/work in roperies; nuns live/work in convents (nunneries); libraries (institutions) live/work in libraries (buildings)""" .
gvp:aat2291_locus-setting_for owl:inverseOf gvp:aat2292_work-live_in.


gvp:aat2294_locus-setting_for a owl:ObjectProperty;
  rdfs:isDefinedBy <http://vocab.getty.edu/ontology>, aat: ;
  rdfs:subPropertyOf skos:related;
  rdfs:domain skos:Concept; rdfs:range skos:Concept;
  # domain "locus/setting"; range "locus/setting";
  dc:identifier "2294";
  skos:prefLabel "aat2294_locus-setting_for";
  dc:title "locus/setting for - locus/setting";
  skos:example "nations are the locus/setting for national capitals",
    "mountain ranges are the locus/setting for mountains" ;
  dct:description """locus/setting - [is] locus setting for - locus/setting.
Example: nations are the locus/setting for national capitals; mountain ranges are the locus/setting for mountains""" .


gvp:aat2295_located_in a owl:ObjectProperty;
  rdfs:isDefinedBy <http://vocab.getty.edu/ontology>, aat: ;
  rdfs:subPropertyOf skos:related;
  rdfs:domain skos:Concept; rdfs:range skos:Concept;
  # domain "locus/setting"; range "locus/setting";
  dc:identifier "2295";
  skos:prefLabel "aat2295_located_in";
  dc:title "located in - locus/setting";
  skos:example "national capitals are located in nations",
    "mountains are located in mountain ranges" ;
  dct:description """locus/setting - [is] located in - locus/setting.
Example: national capitals are located in nations; mountains are located in mountain ranges""" .
gvp:aat2294_locus-setting_for owl:inverseOf gvp:aat2295_located_in.


gvp:aat2311_performed_by a owl:ObjectProperty;
  rdfs:isDefinedBy <http://vocab.getty.edu/ontology>, aat: ;
  rdfs:subPropertyOf skos:related;
  rdfs:domain skos:Concept; rdfs:range skos:Concept;
  # domain "activity/event"; range "role";
  dc:identifier "2311";
  skos:prefLabel "aat2311_performed_by";
  dc:title "performed by - role";
  skos:example "clockmaking is performed by clockmakers",
    "curating is performed by curators" ;
  dct:description """activity/event/[process/function] - [is] performed by - [actors having] a role.
Example: clockmaking is performed by clockmakers; curating is performed by curators""" .


gvp:aat2312_perform a owl:ObjectProperty;
  rdfs:isDefinedBy <http://vocab.getty.edu/ontology>, aat: ;
  rdfs:subPropertyOf skos:related;
  rdfs:domain skos:Concept; rdfs:range skos:Concept;
  # domain "role"; range "activity/event";
  dc:identifier "2312";
  skos:prefLabel "aat2312_perform";
  dc:title "perform - activity/event";
  skos:example "clockmakers perform clockmaking",
    "curators perform curating" ;
  dct:description """[actors having] a role - perform - activity/event/process.
Example: clockmakers perform clockmaking; curators perform curating""" .
gvp:aat2311_performed_by owl:inverseOf gvp:aat2312_perform.


gvp:aat2315_used_by a owl:ObjectProperty;
  rdfs:isDefinedBy <http://vocab.getty.edu/ontology>, aat: ;
  rdfs:subPropertyOf skos:related;
  rdfs:domain skos:Concept; rdfs:range skos:Concept;
  # domain "material"; range "role";
  dc:identifier "2315";
  skos:prefLabel "aat2315_used_by";
  dc:title "used by - role";
  skos:example "precious stone is used by lapidiaries",
    "brass (alloy) is used by braziers (metalworkers)" ;
  dct:description """material - [is] used by - [actor having] role.
Example: precious stone is used by lapidiaries; brass (alloy) is used by braziers (metalworkers)""" .


gvp:aat2316_use a owl:ObjectProperty;
  rdfs:isDefinedBy <http://vocab.getty.edu/ontology>, aat: ;
  rdfs:subPropertyOf skos:related;
  rdfs:domain skos:Concept; rdfs:range skos:Concept;
  # domain "role"; range "material";
  dc:identifier "2316";
  skos:prefLabel "aat2316_use";
  dc:title "use - material";
  skos:example "lapidaries use precious stone",
    "braziers (metalworkers) use brass (alloy)" ;
  dct:description """[actors having] role - use - material.
Example: lapidaries use precious stone; braziers (metalworkers) use brass (alloy)""" .
gvp:aat2315_used_by owl:inverseOf gvp:aat2316_use.


gvp:aat2318_involved_in a owl:ObjectProperty;
  rdfs:isDefinedBy <http://vocab.getty.edu/ontology>, aat: ;
  rdfs:subPropertyOf skos:related;
  rdfs:domain skos:Concept; rdfs:range skos:Concept;
  # domain "role"; range "activity/event";
  dc:identifier "2318";
  skos:prefLabel "aat2318_involved_in";
  dc:title "involved in - activity/event";
  skos:example "bridegrooms are involved in weddings",
    "martyrs are involved in martyrdoms" ;
  dct:description """[actors having] role -[are] involved - activity/event.
Example: bridegrooms are involved in weddings; martyrs are involved in martyrdoms""" .


gvp:aat2319_involves a owl:ObjectProperty;
  rdfs:isDefinedBy <http://vocab.getty.edu/ontology>, aat: ;
  rdfs:subPropertyOf skos:related;
  rdfs:domain skos:Concept; rdfs:range skos:Concept;
  # domain "activity/event"; range "role";
  dc:identifier "2319";
  skos:prefLabel "aat2319_involves";
  dc:title "involves - role";
  skos:example "weddings involve bridegrooms",
    "martyrdoms involve martyrs" ;
  dct:description """activity/event - involves - [actors having] role.
Example: weddings involve bridegrooms; martyrdoms involve martyrs""" .
gvp:aat2318_involved_in owl:inverseOf gvp:aat2319_involves.


gvp:aat2321_used_by a owl:ObjectProperty;
  rdfs:isDefinedBy <http://vocab.getty.edu/ontology>, aat: ;
  rdfs:subPropertyOf skos:related;
  rdfs:domain skos:Concept; rdfs:range skos:Concept;
  # domain "things"; range "role";
  dc:identifier "2321";
  skos:prefLabel "aat2321_used_by";
  dc:title "used by - role";
  skos:example "violoncellos are used by violoncellists",
    "surveying instruments are used by surveyors" ;
  dct:description """things/equipment - [are] used by - [actors having] role.
Example: violoncellos are used by violoncellists; surveying instruments are used by surveyors""" .


gvp:aat2322_use a owl:ObjectProperty;
  rdfs:isDefinedBy <http://vocab.getty.edu/ontology>, aat: ;
  rdfs:subPropertyOf skos:related;
  rdfs:domain skos:Concept; rdfs:range skos:Concept;
  # domain "role"; range "things";
  dc:identifier "2322";
  skos:prefLabel "aat2322_use";
  dc:title "use - things";
  skos:example "violoncellists use violoncellos",
    "surveyors use surveying instruments" ;
  dct:description """[actors having] role - use - things/equipment.
Example: violoncellists use violoncellos; surveyors use surveying instruments""" .
gvp:aat2321_used_by owl:inverseOf gvp:aat2322_use.


gvp:aat2325_created_by a owl:ObjectProperty;
  rdfs:isDefinedBy <http://vocab.getty.edu/ontology>, aat: ;
  rdfs:subPropertyOf skos:related;
  rdfs:domain skos:Concept; rdfs:range skos:Concept;
  # domain "things"; range "role";
  dc:identifier "2325";
  skos:prefLabel "aat2325_created_by";
  dc:title "created by - role";
  skos:example "drawings are created by draftsmen",
    "poems are created by poets" ;
  dct:description """things - [are] created by - [actors having] role.
Example: drawings are created by draftsmen; poems are created by poets""" .


gvp:aat2326_create a owl:ObjectProperty;
  rdfs:isDefinedBy <http://vocab.getty.edu/ontology>, aat: ;
  rdfs:subPropertyOf skos:related;
  rdfs:domain skos:Concept; rdfs:range skos:Concept;
  # domain "role"; range "things";
  dc:identifier "2326";
  skos:prefLabel "aat2326_create";
  dc:title "create - things";
  skos:example "draftsmen create drawings",
    "poets create poems" ;
  dct:description """[actors having] role - create - things.
Example: draftsmen create drawings; poets create poems""" .
gvp:aat2325_created_by owl:inverseOf gvp:aat2326_create.


gvp:aat2328_involved_with a owl:ObjectProperty;
  rdfs:isDefinedBy <http://vocab.getty.edu/ontology>, aat: ;
  rdfs:subPropertyOf skos:related;
  rdfs:domain skos:Concept; rdfs:range skos:Concept;
  # domain "role"; range "things";
  dc:identifier "2328";
  skos:prefLabel "aat2328_involved_with";
  dc:title "involved with - things";
  skos:example "sitters are involved with portraits",
    "actors (performing artists) are involved with motion pictures (visual works)" ;
  dct:description """[actors having] role - [are] involved in- things.
Example: sitters are involved with portraits; actors (performing artists) are involved with motion pictures (visual works)""" .


gvp:aat2329_involves a owl:ObjectProperty;
  rdfs:isDefinedBy <http://vocab.getty.edu/ontology>, aat: ;
  rdfs:subPropertyOf skos:related;
  rdfs:domain skos:Concept; rdfs:range skos:Concept;
  # domain "things"; range "role";
  dc:identifier "2329";
  skos:prefLabel "aat2329_involves";
  dc:title "involves - role";
  skos:example "portraits involve sitters",
    "motion pictures (visual works) involve actors (performing artists)" ;
  dct:description """things - involve - [actors having] role.
Example: portraits involve sitters; motion pictures (visual works) involve actors (performing artists)""" .
gvp:aat2328_involved_with owl:inverseOf gvp:aat2329_involves.


gvp:aat2332_affiliated_with a owl:ObjectProperty;
  rdfs:isDefinedBy <http://vocab.getty.edu/ontology>, aat: ;
  rdfs:subPropertyOf skos:related;
  rdfs:domain skos:Concept; rdfs:range skos:Concept;
  # domain "role"; range "role";
  dc:identifier "2332";
  skos:prefLabel "aat2332_affiliated_with";
  dc:title "affiliated with - role";
  skos:example "students are affiliated with schools (organizations)",
    "dukes are affiliated with duchies" ;
  dct:description """[actors having] role - [are] affiliated with - role [organization].
Example: students are affiliated with schools (organizations); dukes are affiliated with duchies""" .


gvp:aat2333_have_affiliates a owl:ObjectProperty;
  rdfs:isDefinedBy <http://vocab.getty.edu/ontology>, aat: ;
  rdfs:subPropertyOf skos:related;
  rdfs:domain skos:Concept; rdfs:range skos:Concept;
  # domain "role"; range "role";
  dc:identifier "2333";
  skos:prefLabel "aat2333_have_affiliates";
  dc:title "have affiliates - role";
  skos:example "schools (organizations) have as affiliates students",
    "duchies have as affiliates dukes" ;
  dct:description """role [organizations] - have affiliates - [actors having] role.
Example: schools (organizations) have as affiliates students; duchies have as affiliates dukes""" .
gvp:aat2332_affiliated_with owl:inverseOf gvp:aat2333_have_affiliates.


gvp:aat2335_associated_with a owl:ObjectProperty;
  rdfs:isDefinedBy <http://vocab.getty.edu/ontology>, aat: ;
  rdfs:subPropertyOf skos:related;
  rdfs:domain skos:Concept; rdfs:range skos:Concept;
  # domain "role"; range "style/period/culture";
  dc:identifier "2335";
  skos:prefLabel "aat2335_associated_with";
  dc:title "associated with - style/period/culture";
  skos:example "abstract artists are associated with Abstract (fine arts style)",
    "popes are associated with Roman Catholicism" ;
  dct:description """[actors having] role - [are] associated with - style/period/culture/[religion/ideology].
Example: abstract artists are associated with Abstract (fine arts style); popes are associated with Roman Catholicism""" .


gvp:aat2336_has_associates a owl:ObjectProperty;
  rdfs:isDefinedBy <http://vocab.getty.edu/ontology>, aat: ;
  rdfs:subPropertyOf skos:related;
  rdfs:domain skos:Concept; rdfs:range skos:Concept;
  # domain "style/period/culture"; range "role";
  dc:identifier "2336";
  skos:prefLabel "aat2336_has_associates";
  dc:title "has associates - role";
  skos:example "Abstract (fine arts style) has associates abstract artists",
    "Roman Catholicism has associates popes" ;
  dct:description """style/period/culture/[relgion] - has associates - [actors having] role.
Example: Abstract (fine arts style) has associates abstract artists; Roman Catholicism has associates popes""" .
gvp:aat2335_associated_with owl:inverseOf gvp:aat2336_has_associates.


gvp:aat2397_focus_of a owl:ObjectProperty;
  rdfs:isDefinedBy <http://vocab.getty.edu/ontology>, aat: ;
  rdfs:subPropertyOf skos:related;
  rdfs:domain skos:Concept; rdfs:range skos:Concept;
  # domain "any"; range "field/discipline";
  dc:identifier "2397";
  skos:prefLabel "aat2397_focus_of";
  dc:title "focus of - field/discipline";
  skos:example "manuscripts are the focus of codicology",
    "music is the focus of musicology",
    "Plantae (kingdom) is the focus of botany" ;
  dct:description """any - [is] focus of - field [of study]/discipline.
Example: manuscripts are the focus of codicology; music is the focus of musicology; Plantae (kingdom) is the focus of botany""" .


gvp:aat2398_focuses_on a owl:ObjectProperty;
  rdfs:isDefinedBy <http://vocab.getty.edu/ontology>, aat: ;
  rdfs:subPropertyOf skos:related;
  rdfs:domain skos:Concept; rdfs:range skos:Concept;
  # domain "field/discipline"; range "any";
  dc:identifier "2398";
  skos:prefLabel "aat2398_focuses_on";
  dc:title "focuses on - any";
  skos:example "codicology focuses on manuscripts",
    "musicology focuses on music",
    "bontany focuses on Plantae (kingdom)" ;
  dct:description """field [of study]/discipline - focuses on - any.
Example: codicology focuses on manuscripts; musicology focuses on music; bontany focuses on Plantae (kingdom)""" .
gvp:aat2397_focus_of owl:inverseOf gvp:aat2398_focuses_on.


gvp:aat2408_locus-setting_for a owl:ObjectProperty;
  rdfs:isDefinedBy <http://vocab.getty.edu/ontology>, aat: ;
  rdfs:subPropertyOf skos:related;
  rdfs:domain skos:Concept; rdfs:range skos:Concept;
  # domain "locus/setting"; range "field/discipline";
  dc:identifier "2408";
  skos:prefLabel "aat2408_locus-setting_for";
  dc:title "locus/setting for - field/discipline";
  skos:example "schools (buildings) are the locus/setting for education",
    "hospitals (buildings) are the locus/setting for medicine (discipline)" ;
  dct:description """locus/setting - [is] locus/setting for - field of study/discipline.
Example: schools (buildings) are the locus/setting for education; hospitals (buildings) are the locus/setting for medicine (discipline)""" .


gvp:aat2409_takes_place_in a owl:ObjectProperty;
  rdfs:isDefinedBy <http://vocab.getty.edu/ontology>, aat: ;
  rdfs:subPropertyOf skos:related;
  rdfs:domain skos:Concept; rdfs:range skos:Concept;
  # domain "field/discipline"; range "locus/setting";
  dc:identifier "2409";
  skos:prefLabel "aat2409_takes_place_in";
  dc:title "takes place in - locus/setting";
  skos:example "education takes place in schools (buildings)",
    "medicine (discipline) takes place in hospitals (buildings)" ;
  dct:description """field of study/discipline - takes place in - locus/setting.
Example: education takes place in schools (buildings); medicine (discipline) takes place in hospitals (buildings)""" .
gvp:aat2408_locus-setting_for owl:inverseOf gvp:aat2409_takes_place_in.


gvp:aat2411_involved_in a owl:ObjectProperty;
  rdfs:isDefinedBy <http://vocab.getty.edu/ontology>, aat: ;
  rdfs:subPropertyOf skos:related;
  rdfs:domain skos:Concept; rdfs:range skos:Concept;
  # domain "activity/event"; range "field/discipline";
  dc:identifier "2411";
  skos:prefLabel "aat2411_involved_in";
  dc:title "involved in - field/discipline";
  skos:example "journalistic photography is involved in photojournalism (discipline)",
    "gardening is involved in horticulture" ;
  dct:description """activity/event/[process/function] - [is] involved in - field/discipline.
Example: journalistic photography is involved in photojournalism (discipline); gardening is involved in horticulture""" .


gvp:aat2412_involves a owl:ObjectProperty;
  rdfs:isDefinedBy <http://vocab.getty.edu/ontology>, aat: ;
  rdfs:subPropertyOf skos:related;
  rdfs:domain skos:Concept; rdfs:range skos:Concept;
  # domain "field/discipline"; range "activity/event";
  dc:identifier "2412";
  skos:prefLabel "aat2412_involves";
  dc:title "involves - activity/event";
  skos:example "photojournalism (discipline) involves journalistic photography",
    "horticulture involves gardening" ;
  dct:description """field/discipline - involves - activity/event/[process/function].
Example: photojournalism (discipline) involves journalistic photography; horticulture involves gardening""" .
gvp:aat2411_involved_in owl:inverseOf gvp:aat2412_involves.


gvp:aat2415_required_for a owl:ObjectProperty;
  rdfs:isDefinedBy <http://vocab.getty.edu/ontology>, aat: ;
  rdfs:subPropertyOf skos:related;
  rdfs:domain skos:Concept; rdfs:range skos:Concept;
  # domain "material"; range "activity/event";
  dc:identifier "2415";
  skos:prefLabel "aat2415_required_for";
  dc:title "required for - activity/event";
  skos:example "dye is required for dying",
    "pewter is required for pewtersmithing" ;
  dct:description """material - [is] required for - activity/event/[process/function].
Example: dye is required for dying; pewter is required for pewtersmithing""" .


gvp:aat2416_requires a owl:ObjectProperty;
  rdfs:isDefinedBy <http://vocab.getty.edu/ontology>, aat: ;
  rdfs:subPropertyOf skos:related;
  rdfs:domain skos:Concept; rdfs:range skos:Concept;
  # domain "activity/event"; range "material";
  dc:identifier "2416";
  skos:prefLabel "aat2416_requires";
  dc:title "requires - material";
  skos:example "dying requires dye",
    "pewtersmithing requires pewter" ;
  dct:description """activity/event/[process/function] - requires - material.
Example: dying requires dye; pewtersmithing requires pewter""" .
gvp:aat2415_required_for owl:inverseOf gvp:aat2416_requires.


gvp:aat2418_uses a owl:ObjectProperty;
  rdfs:isDefinedBy <http://vocab.getty.edu/ontology>, aat: ;
  rdfs:subPropertyOf skos:related;
  rdfs:domain skos:Concept; rdfs:range skos:Concept;
  # domain "field/discipline"; range "things";
  dc:identifier "2418";
  skos:prefLabel "aat2418_uses";
  dc:title "uses - things";
  skos:example "astronomy uses astronomical instruments",
    "divination [discipline] uses divination objects" ;
  dct:description """field [of study]/discipline - uses - things/[equipment].
Example: astronomy uses astronomical instruments; divination [discipline] uses divination objects""" .


gvp:aat2419_used_for a owl:ObjectProperty;
  rdfs:isDefinedBy <http://vocab.getty.edu/ontology>, aat: ;
  rdfs:subPropertyOf skos:related;
  rdfs:domain skos:Concept; rdfs:range skos:Concept;
  # domain "things"; range "field/discipline";
  dc:identifier "2419";
  skos:prefLabel "aat2419_used_for";
  dc:title "used for - field/discipline";
  skos:example "astronomical instruments are used for astronomy",
    "divination objects are used for divination [discipline]" ;
  dct:description """things/[equipment] - [are] used for - field [of study]/discipline.
Example: astronomical instruments are used for astronomy; divination objects are used for divination [discipline]""" .
gvp:aat2418_uses owl:inverseOf gvp:aat2419_used_for.


gvp:aat2421_locus-setting_for a owl:ObjectProperty;
  rdfs:isDefinedBy <http://vocab.getty.edu/ontology>, aat: ;
  rdfs:subPropertyOf skos:related;
  rdfs:domain skos:Concept; rdfs:range skos:Concept;
  # domain "locus/setting"; range "activity/event";
  dc:identifier "2421";
  skos:prefLabel "aat2421_locus-setting_for";
  dc:title "locus/setting for - activity/event";
  skos:example "smelters (metalworking plants) are the locus/setting for smelting",
    "pilgrimage centers are the locus/setting for pilgrimages" ;
  dct:description """locus/setting - [is] locus/setting for - activity/event/[process/function].
Example: smelters (metalworking plants) are the locus/setting for smelting; pilgrimage centers are the locus/setting for pilgrimages""" .


gvp:aat2422_takes_place_in a owl:ObjectProperty;
  rdfs:isDefinedBy <http://vocab.getty.edu/ontology>, aat: ;
  rdfs:subPropertyOf skos:related;
  rdfs:domain skos:Concept; rdfs:range skos:Concept;
  # domain "activity/event"; range "locus/setting";
  dc:identifier "2422";
  skos:prefLabel "aat2422_takes_place_in";
  dc:title "takes place in - locus/setting";
  skos:example "smelting takes place in smelters (metalworking plants)",
    "pilgrimages take place in pilgrimage centers" ;
  dct:description """activity/event/[process/function] - takes place in - locus/setting.
Example: smelting takes place in smelters (metalworking plants); pilgrimages take place in pilgrimage centers""" .
gvp:aat2421_locus-setting_for owl:inverseOf gvp:aat2422_takes_place_in.


gvp:aat2424_produced_by a owl:ObjectProperty;
  rdfs:isDefinedBy <http://vocab.getty.edu/ontology>, aat: ;
  rdfs:subPropertyOf skos:related;
  rdfs:domain skos:Concept; rdfs:range skos:Concept;
  # domain "material"; range "activity/event/process";
  dc:identifier "2424";
  skos:prefLabel "aat2424_produced_by";
  dc:title "produced by - activity/event/process";
  skos:example "wire is produced by wiredrawing",
    "paper is produced by papermaking" ;
  dct:description """material - [is] produced by - activity/event/process.
Example: wire is produced by wiredrawing; paper is produced by papermaking""" .


gvp:aat2425_produces a owl:ObjectProperty;
  rdfs:isDefinedBy <http://vocab.getty.edu/ontology>, aat: ;
  rdfs:subPropertyOf skos:related;
  rdfs:domain skos:Concept; rdfs:range skos:Concept;
  # domain "activity/event/process"; range "material";
  dc:identifier "2425";
  skos:prefLabel "aat2425_produces";
  dc:title "produces - material";
  skos:example "wiredrawing produces wire",
    "papermaking produces paper" ;
  dct:description """activity/event/process - produces - material.
Example: wiredrawing produces wire; papermaking produces paper""" .
gvp:aat2424_produced_by owl:inverseOf gvp:aat2425_produces.


gvp:aat2427_produced_by a owl:ObjectProperty;
  rdfs:isDefinedBy <http://vocab.getty.edu/ontology>, aat: ;
  rdfs:subPropertyOf skos:related;
  rdfs:domain skos:Concept; rdfs:range skos:Concept;
  # domain "things"; range "activity/event/process";
  dc:identifier "2427";
  skos:prefLabel "aat2427_produced_by";
  dc:title "produced by - activity/event/process";
  skos:example "vase paintings (visual works) are produced by vase painting (image making)",
    "forgeries are produced by forging (copying)" ;
  dct:description """things - [are] produced by - activity/event/process.
Example: vase paintings (visual works) are produced by vase painting (image making); forgeries are produced by forging (copying)""" .


gvp:aat2428_produces a owl:ObjectProperty;
  rdfs:isDefinedBy <http://vocab.getty.edu/ontology>, aat: ;
  rdfs:subPropertyOf skos:related;
  rdfs:domain skos:Concept; rdfs:range skos:Concept;
  # domain "activity/event/process"; range "things";
  dc:identifier "2428";
  skos:prefLabel "aat2428_produces";
  dc:title "produces - things";
  skos:example "vase painting (image making) produces vase paintings (visual works)",
    "forging (copying) produces forgeries" ;
  dct:description """activity/event/process - produces - things.
Example: vase painting (image making) produces vase paintings (visual works); forging (copying) produces forgeries""" .
gvp:aat2427_produced_by owl:inverseOf gvp:aat2428_produces.


gvp:aat2431_required_for a owl:ObjectProperty;
  rdfs:isDefinedBy <http://vocab.getty.edu/ontology>, aat: ;
  rdfs:subPropertyOf skos:related;
  rdfs:domain skos:Concept; rdfs:range skos:Concept;
  # domain "things"; range "activity/event/process";
  dc:identifier "2431";
  skos:prefLabel "aat2431_required_for";
  dc:title "required for - activity/event/process";
  skos:example "painting equipment is required for painting (image making)",
    "dowels are required for doweling" ;
  dct:description """things/equipment - [are] required for - activity/event/process.
Example: painting equipment is required for painting (image making); dowels are required for doweling""" .


gvp:aat2432_requires a owl:ObjectProperty;
  rdfs:isDefinedBy <http://vocab.getty.edu/ontology>, aat: ;
  rdfs:subPropertyOf skos:related;
  rdfs:domain skos:Concept; rdfs:range skos:Concept;
  # domain "activity/event/process"; range "things";
  dc:identifier "2432";
  skos:prefLabel "aat2432_requires";
  dc:title "requires - things";
  skos:example "painting (image making) requires painting equipment",
    "doweling requires dowels" ;
  dct:description """activity/event/process - requires - things/equipment.
Example: painting (image making) requires painting equipment; doweling requires dowels""" .
gvp:aat2431_required_for owl:inverseOf gvp:aat2432_requires.


gvp:aat2434_contextualized_in a owl:ObjectProperty;
  rdfs:isDefinedBy <http://vocab.getty.edu/ontology>, aat: ;
  rdfs:subPropertyOf skos:related;
  rdfs:domain skos:Concept; rdfs:range skos:Concept;
  # domain "things"; range "activity/event/process";
  dc:identifier "2434";
  skos:prefLabel "aat2434_contextualized_in";
  dc:title "contextualized in - activity/event/process";
  skos:example "funeral books are contextualized in funerals",
    "Christmas trees are contextualized in Christmas" ;
  dct:description """things - [are] context for - activity/event/process.
Example: funeral books are contextualized in funerals; Christmas trees are contextualized in Christmas""" .


gvp:aat2435_context_for a owl:ObjectProperty;
  rdfs:isDefinedBy <http://vocab.getty.edu/ontology>, aat: ;
  rdfs:subPropertyOf skos:related;
  rdfs:domain skos:Concept; rdfs:range skos:Concept;
  # domain "activity/event/process"; range "things";
  dc:identifier "2435";
  skos:prefLabel "aat2435_context_for";
  dc:title "context for - things";
  skos:example "funerals are the context for funeral books",
    "Christmas is the context for Christmas trees" ;
  dct:description """activity/event/process - [is] contextualized in - thing.
Example: funerals are the context for funeral books; Christmas is the context for Christmas trees""" .
gvp:aat2434_contextualized_in owl:inverseOf gvp:aat2435_context_for.


gvp:aat2501_made_of-require a owl:ObjectProperty;
  rdfs:isDefinedBy <http://vocab.getty.edu/ontology>, aat: ;
  rdfs:subPropertyOf skos:related;
  rdfs:domain skos:Concept; rdfs:range skos:Concept;
  # domain "things"; range "material";
  dc:identifier "2501";
  skos:prefLabel "aat2501_made_of-require";
  dc:title "made of/require - material";
  skos:example "obsidian mirrors are made of/require obsidian",
    "ivories (sculptures) are made of/require ivory" ;
  dct:description """things - [are] made of/require - material.
Example: obsidian mirrors are made of/require obsidian; ivories (sculptures) are made of/require ivory""" .


gvp:aat2502_material_for a owl:ObjectProperty;
  rdfs:isDefinedBy <http://vocab.getty.edu/ontology>, aat: ;
  rdfs:subPropertyOf skos:related;
  rdfs:domain skos:Concept; rdfs:range skos:Concept;
  # domain "material"; range "things";
  dc:identifier "2502";
  skos:prefLabel "aat2502_material_for";
  dc:title "material for - things";
  skos:example "obsidian is material for obsidian mirrors",
    "ivory is material for ivories (sculptures)" ;
  dct:description """material - [is] material for - things.
Example: obsidian is material for obsidian mirrors; ivory is material for ivories (sculptures)""" .
gvp:aat2501_made_of-require owl:inverseOf gvp:aat2502_material_for.


gvp:aat2504_used-located_in a owl:ObjectProperty;
  rdfs:isDefinedBy <http://vocab.getty.edu/ontology>, aat: ;
  rdfs:subPropertyOf skos:related;
  rdfs:domain skos:Concept; rdfs:range skos:Concept;
  # domain "material"; range "locus/setting";
  dc:identifier "2504";
  skos:prefLabel "aat2504_used-located_in";
  dc:title "used/located in - locus/setting";
  skos:example "tephra is used/located in [at] volcanoes",
    "brick (clay product) is used/located in brickworks (factories)" ;
  dct:description """material - [is] used/located in - locus/setting.
Example: tephra is used/located in [at] volcanoes; brick (clay product) is used/located in brickworks (factories)""" .


gvp:aat2505_locus-setting_for a owl:ObjectProperty;
  rdfs:isDefinedBy <http://vocab.getty.edu/ontology>, aat: ;
  rdfs:subPropertyOf skos:related;
  rdfs:domain skos:Concept; rdfs:range skos:Concept;
  # domain "locus/setting"; range "material";
  dc:identifier "2505";
  skos:prefLabel "aat2505_locus-setting_for";
  dc:title "locus/setting for - material";
  skos:example "volcanoes are locus/setting for  tephra",
    "brickworks (factories) are locus/setting for brick (clay product)" ;
  dct:description """locus/setting - [is] locus/setting for - material.
Example: volcanoes are locus/setting for  tephra; brickworks (factories) are locus/setting for brick (clay product)""" .
gvp:aat2504_used-located_in owl:inverseOf gvp:aat2505_locus-setting_for.


gvp:aat2507_produce-process a owl:ObjectProperty;
  rdfs:isDefinedBy <http://vocab.getty.edu/ontology>, aat: ;
  rdfs:subPropertyOf skos:related;
  rdfs:domain skos:Concept; rdfs:range skos:Concept;
  # domain "things"; range "material";
  dc:identifier "2507";
  skos:prefLabel "aat2507_produce-process";
  dc:title "produce/process - material";
  skos:example "cotton (fiber) is produced/processed by cotton gins",
    "groundwater is produced/processed by water wells" ;
  dct:description """things/[equipment] - produce/process - material.
Example: cotton (fiber) is produced/processed by cotton gins; groundwater is produced/processed by water wells""" .


gvp:aat2508_produced-processed_by a owl:ObjectProperty;
  rdfs:isDefinedBy <http://vocab.getty.edu/ontology>, aat: ;
  rdfs:subPropertyOf skos:related;
  rdfs:domain skos:Concept; rdfs:range skos:Concept;
  # domain "material"; range "things";
  dc:identifier "2508";
  skos:prefLabel "aat2508_produced-processed_by";
  dc:title "produced/processed by - things";
  skos:example "cotton gins produce/process cotton (fiber)",
    "waterwells produce/process groundwater" ;
  dct:description """material - [is] produced/processed by - things/[equipment].
Example: cotton gins produce/process cotton (fiber); waterwells produce/process groundwater""" .
gvp:aat2507_produce-process owl:inverseOf gvp:aat2508_produced-processed_by.


gvp:aat2551_reflect-produced_by a owl:ObjectProperty;
  rdfs:isDefinedBy <http://vocab.getty.edu/ontology>, aat: ;
  rdfs:subPropertyOf skos:related;
  rdfs:domain skos:Concept; rdfs:range skos:Concept;
  # domain "things"; range "style/period/culture";
  dc:identifier "2551";
  skos:prefLabel "aat2551_reflect-produced_by";
  dc:title "reflect/produced by - style/period/culture";
  skos:example "Nasca lines reflect/are produced by Nasca [culture]",
    "Judaica reflects/is produced by Judaism" ;
  dct:description """things - reflect/[are] produced by - style/period/culture/[religion/ideology].
Example: Nasca lines reflect/are produced by Nasca [culture]; Judaica reflects/is produced by Judaism""" .


gvp:aat2552_reflected_in-produces a owl:ObjectProperty;
  rdfs:isDefinedBy <http://vocab.getty.edu/ontology>, aat: ;
  rdfs:subPropertyOf skos:related;
  rdfs:domain skos:Concept; rdfs:range skos:Concept;
  # domain "style/period/culture"; range "things";
  dc:identifier "2552";
  skos:prefLabel "aat2552_reflected_in-produces";
  dc:title "reflected in/produces - things";
  skos:example "Nasca [culture] produces/is reflected in Nasca lines",
    "Judaism produces/is reflected in Judaica" ;
  dct:description """style/period/culture/[religion/ideology] - [is] reflected in/produces - things.
Example: Nasca [culture] produces/is reflected in Nasca lines; Judaism produces/is reflected in Judaica""" .
gvp:aat2551_reflect-produced_by owl:inverseOf gvp:aat2552_reflected_in-produces.


gvp:aat2554_reflects a owl:ObjectProperty;
  rdfs:isDefinedBy <http://vocab.getty.edu/ontology>, aat: ;
  rdfs:subPropertyOf skos:related;
  rdfs:domain skos:Concept; rdfs:range skos:Concept;
  # domain "activity/event"; range "style/period/culture";
  dc:identifier "2554";
  skos:prefLabel "aat2554_reflects";
  dc:title "reflects - style/period/culture";
  skos:example "dhokra (casting technique) reflects Dhokra (culture)",
    "red-figure vase painting reflects Red-figure [style]" ;
  dct:description """activity/event - reflects - style/period/culture /[religion/ideology].
Example: dhokra (casting technique) reflects Dhokra (culture); red-figure vase painting reflects Red-figure [style]""" .


gvp:aat2555_reflected_in a owl:ObjectProperty;
  rdfs:isDefinedBy <http://vocab.getty.edu/ontology>, aat: ;
  rdfs:subPropertyOf skos:related;
  rdfs:domain skos:Concept; rdfs:range skos:Concept;
  # domain "style/period/culture"; range "activity/event";
  dc:identifier "2555";
  skos:prefLabel "aat2555_reflected_in";
  dc:title "reflected in - activity/event";
  skos:example "Dhokra (culture) is reflected in dhokra (casting technique)",
    "Red-figure [style] is reflected in red-figure vase painting" ;
  dct:description """style/period/culture /[religion/ideology] - [is] reflected in activity/event.
Example: Dhokra (culture) is reflected in dhokra (casting technique); Red-figure [style] is reflected in red-figure vase painting""" .
gvp:aat2554_reflects owl:inverseOf gvp:aat2555_reflected_in.


gvp:aat2557_reflects a owl:ObjectProperty;
  rdfs:isDefinedBy <http://vocab.getty.edu/ontology>, aat: ;
  rdfs:subPropertyOf skos:related;
  rdfs:domain skos:Concept; rdfs:range skos:Concept;
  # domain "field/discipline"; range "style/period/culture";
  dc:identifier "2557";
  skos:prefLabel "aat2557_reflects";
  dc:title "reflects - style/period/culture";
  skos:example "bugatu [dance discipline] reflects Buddhism",
    "church history reflects Christianity",
    "classics (discipline) reflects Ancient Greek [culture]" ;
  dct:description """field/discipline - reflects - style/period/culture /[religion/ideology].
Example: bugatu [dance discipline] reflects Buddhism; church history reflects Christianity; classics (discipline) reflects Ancient Greek [culture]""" .


gvp:aat2558_reflected_in a owl:ObjectProperty;
  rdfs:isDefinedBy <http://vocab.getty.edu/ontology>, aat: ;
  rdfs:subPropertyOf skos:related;
  rdfs:domain skos:Concept; rdfs:range skos:Concept;
  # domain "style/period/culture"; range "field/discipline";
  dc:identifier "2558";
  skos:prefLabel "aat2558_reflected_in";
  dc:title "reflected in - field/discipline";
  skos:example "Buddhism is reflected in bugatu [dance discipline]",
    "Christianity is reflected in church history",
    "Ancient Greek [culture] is reflected in classics (discipline)" ;
  dct:description """style/period/culture /[religion/ideology] - [is] reflected in field/discipline.
Example: Buddhism is reflected in bugatu [dance discipline]; Christianity is reflected in church history; Ancient Greek [culture] is reflected in classics (discipline)""" .
gvp:aat2557_reflects owl:inverseOf gvp:aat2558_reflected_in.


gvp:aat2562_locus-setting_for a owl:ObjectProperty;
  rdfs:isDefinedBy <http://vocab.getty.edu/ontology>, aat: ;
  rdfs:subPropertyOf skos:related;
  rdfs:domain skos:Concept; rdfs:range skos:Concept;
  # domain "locus/setting"; range "style/period/culture";
  dc:identifier "2562";
  skos:prefLabel "aat2562_locus-setting_for";
  dc:title "locus/setting for - style/period/culture";
  skos:example "First Nations reserves are the locus/setting for First Nations (culture)",
    "agraharas are the locus/setting for Brahmanism" ;
  dct:description """locus/setting - [is] locus/setting for - style/period/culture/[religion/ideology].
Example: First Nations reserves are the locus/setting for First Nations (culture); agraharas are the locus/setting for Brahmanism""" .


gvp:aat2563_located_in a owl:ObjectProperty;
  rdfs:isDefinedBy <http://vocab.getty.edu/ontology>, aat: ;
  rdfs:subPropertyOf skos:related;
  rdfs:domain skos:Concept; rdfs:range skos:Concept;
  # domain "style/period/culture"; range "locus/setting";
  dc:identifier "2563";
  skos:prefLabel "aat2563_located_in";
  dc:title "located in - locus/setting";
  skos:example "First Nations (culture) is located/reflected in First Nations reserves",
    "Brahmanism is located/reflected in agraharas" ;
  dct:description """style/period/culture/[religion/ideology] - is located/[reflected] in - locus/setting.
Example: First Nations (culture) is located/reflected in First Nations reserves; Brahmanism is located/reflected in agraharas""" .
gvp:aat2562_locus-setting_for owl:inverseOf gvp:aat2563_located_in.


gvp:aat2601_possessed_by-existing_in a owl:ObjectProperty;
  rdfs:isDefinedBy <http://vocab.getty.edu/ontology>, aat: ;
  rdfs:subPropertyOf skos:related;
  rdfs:domain skos:Concept; rdfs:range skos:Concept;
  # domain "attributes /associated concepts"; range "role";
  dc:identifier "2601";
  skos:prefLabel "aat2601_possessed_by-existing_in";
  dc:title "possessed by/existing in - role";
  skos:example "adulthood is possessed by/existing in adults",
    "nomadism is possessed by/existing in nomads" ;
  dct:description """attributes /associated concepts - [is] possessed by/existing in - role [of actors].
Example: adulthood is possessed by/existing in adults; nomadism is possessed by/existing in nomads""" .


gvp:aat2602_possess-exist_in a owl:ObjectProperty;
  rdfs:isDefinedBy <http://vocab.getty.edu/ontology>, aat: ;
  rdfs:subPropertyOf skos:related;
  rdfs:domain skos:Concept; rdfs:range skos:Concept;
  # domain "role"; range "attributes /associated concepts";
  dc:identifier "2602";
  skos:prefLabel "aat2602_possess-exist_in";
  dc:title "possess/exist in - attributes /associated concepts";
  skos:example "adults possess/exist in adulthood",
    "nomads possess/exist in [state of] nomadism" ;
  dct:description """role [of actors] - possess/exist in - attributes /associated concepts.
Example: adults possess/exist in adulthood; nomads possess/exist in [state of] nomadism""" .
gvp:aat2601_possessed_by-existing_in owl:inverseOf gvp:aat2602_possess-exist_in.


gvp:aat2604_possessed_by-existing_in a owl:ObjectProperty;
  rdfs:isDefinedBy <http://vocab.getty.edu/ontology>, aat: ;
  rdfs:subPropertyOf skos:related;
  rdfs:domain skos:Concept; rdfs:range skos:Concept;
  # domain "attributes /associated concepts"; range "things";
  dc:identifier "2604";
  skos:prefLabel "aat2604_possessed_by-existing_in";
  dc:title "possessed by/existing in - things";
  skos:example "boudoir (photograph size) is possessed by/existing in boudoir photographs",
    "ruined [condition] is possessed by/existing in ruins" ;
  dct:description """attributes /associated concepts - [is] possessed by/existing in - things.
Example: boudoir (photograph size) is possessed by/existing in boudoir photographs; ruined [condition] is possessed by/existing in ruins""" .


gvp:aat2605_possess-exist_in a owl:ObjectProperty;
  rdfs:isDefinedBy <http://vocab.getty.edu/ontology>, aat: ;
  rdfs:subPropertyOf skos:related;
  rdfs:domain skos:Concept; rdfs:range skos:Concept;
  # domain "things"; range "attributes /associated concepts";
  dc:identifier "2605";
  skos:prefLabel "aat2605_possess-exist_in";
  dc:title "possess/exist in - attributes /associated concepts";
  skos:example "boudoir photographs possess/exist in boudoir (photograph size)",
    "ruins possess/exist in ruined [contition]" ;
  dct:description """things - possess/exist in - attributes /associated concepts.
Example: boudoir photographs possess/exist in boudoir (photograph size); ruins possess/exist in ruined [contition]""" .
gvp:aat2604_possessed_by-existing_in owl:inverseOf gvp:aat2605_possess-exist_in.


gvp:aat2607_caused_by-requires a owl:ObjectProperty;
  rdfs:isDefinedBy <http://vocab.getty.edu/ontology>, aat: ;
  rdfs:subPropertyOf skos:related;
  rdfs:domain skos:Concept; rdfs:range skos:Concept;
  # domain "attributes /associated concepts"; range "activity/event";
  dc:identifier "2607";
  skos:prefLabel "aat2607_caused_by-requires";
  dc:title "caused by/requires - activity/event";
  skos:example "watertightness is caused by/requires waterproofing",
    "creases (condition) is caused by/requires creasing (process)" ;
  dct:description """attributes /associated concepts - [is] caused by/requires - an activity/event/[process/function].
Example: watertightness is caused by/requires waterproofing; creases (condition) is caused by/requires creasing (process)""" .


gvp:aat2608_causes-required_for a owl:ObjectProperty;
  rdfs:isDefinedBy <http://vocab.getty.edu/ontology>, aat: ;
  rdfs:subPropertyOf skos:related;
  rdfs:domain skos:Concept; rdfs:range skos:Concept;
  # domain "activity/event"; range "attributes /associated concepts";
  dc:identifier "2608";
  skos:prefLabel "aat2608_causes-required_for";
  dc:title "causes/required for - attributes /associated concepts";
  skos:example "waterproofing causes/is required for watertighness",
    "creasing (process) causes/is required for creases (condition)" ;
  dct:description """activity/event/[process/function] - causes/[is] required for - [a] state/condition/attributes.
Example: waterproofing causes/is required for watertighness; creasing (process) causes/is required for creases (condition)""" .
gvp:aat2607_caused_by-requires owl:inverseOf gvp:aat2608_causes-required_for.


gvp:aat2612_possessed_by-existing_in a owl:ObjectProperty;
  rdfs:isDefinedBy <http://vocab.getty.edu/ontology>, aat: ;
  rdfs:subPropertyOf skos:related;
  rdfs:domain skos:Concept; rdfs:range skos:Concept;
  # domain "attributes /associated concepts"; range "material";
  dc:identifier "2612";
  skos:prefLabel "aat2612_possessed_by-existing_in";
  dc:title "possessed by/existing in - material";
  skos:example "dry rot is possessed by/existing in wood(plant material)",
    "dielectric properties are possessed by/existing in dielectric (material)" ;
  dct:description """attributes /associated concepts - is possessed by/existing in - material.
Example: dry rot is possessed by/existing in wood(plant material); dielectric properties are possessed by/existing in dielectric (material)""" .


gvp:aat2613_possess-exist_in a owl:ObjectProperty;
  rdfs:isDefinedBy <http://vocab.getty.edu/ontology>, aat: ;
  rdfs:subPropertyOf skos:related;
  rdfs:domain skos:Concept; rdfs:range skos:Concept;
  # domain "material"; range "attributes /associated concepts";
  dc:identifier "2613";
  skos:prefLabel "aat2613_possess-exist_in";
  dc:title "possess/exist in - attributes /associated concepts";
  skos:example "wood(plant material) possesses/exists in [condition of] dry rot",
    "dielectric (material) possesses/exists in dielectric properties" ;
  dct:description """material - possesses/exists in - condition/state/[property].
Example: wood(plant material) possesses/exists in [condition of] dry rot; dielectric (material) possesses/exists in dielectric properties""" .
gvp:aat2612_possessed_by-existing_in owl:inverseOf gvp:aat2613_possess-exist_in.


gvp:aat2801_conjuncted_with a owl:ObjectProperty;
  rdfs:isDefinedBy <http://vocab.getty.edu/ontology>, aat: ;
  rdfs:subPropertyOf skos:related;
  rdfs:domain skos:Concept; rdfs:range skos:Concept;
  # domain "things"; range "things";
  dc:identifier "2801";
  skos:prefLabel "aat2801_conjuncted_with";
  dc:title "conjuncted with - things";
  skos:example "cups are conjuncted with saucers",
    "dining tables are conjuncted with dining chairs" ;
  dct:description """things - [are] conjuncted with - things.
Example: cups are conjuncted with saucers; dining tables are conjuncted with dining chairs""" .
gvp:aat2801_conjuncted_with a owl:SymmetricProperty.


gvp:aat2802_exemplified_by a owl:ObjectProperty;
  rdfs:isDefinedBy <http://vocab.getty.edu/ontology>, aat: ;
  rdfs:subPropertyOf skos:related;
  rdfs:domain skos:Concept; rdfs:range skos:Concept;
  # domain "material"; range "brand name";
  dc:identifier "2802";
  skos:prefLabel "aat2802_exemplified_by";
  dc:title "exemplified by - brand name";
  skos:example "petrolium jelly is exemplified by Vaseline (TM)",
    "polytetrafluoroethyelene is exemplified by Teflon (TM)" ;
  dct:description """material - [is] exemplified by - brand name.
Example: petrolium jelly is exemplified by Vaseline (TM); polytetrafluoroethyelene is exemplified by Teflon (TM)""" .


gvp:aat2803_example_of a owl:ObjectProperty;
  rdfs:isDefinedBy <http://vocab.getty.edu/ontology>, aat: ;
  rdfs:subPropertyOf skos:related;
  rdfs:domain skos:Concept; rdfs:range skos:Concept;
  # domain "brand name"; range "material";
  dc:identifier "2803";
  skos:prefLabel "aat2803_example_of";
  dc:title "example of - material";
  skos:example "Vaseline (TM) is an example of petrolium jelly",
    "Teflon (TM) is an example of polytetrafluoroethyelene" ;
  dct:description """brand name - [is] example of - material.
Example: Vaseline (TM) is an example of petrolium jelly; Teflon (TM) is an example of polytetrafluoroethyelene""" .
gvp:aat2802_exemplified_by owl:inverseOf gvp:aat2803_example_of.


gvp:aat2805_contextualized_in a owl:ObjectProperty;
  rdfs:isDefinedBy <http://vocab.getty.edu/ontology>, aat: ;
  rdfs:subPropertyOf skos:related;
  rdfs:domain skos:Concept; rdfs:range skos:Concept;
  # domain "things"; range "things";
  dc:identifier "2805";
  skos:prefLabel "aat2805_contextualized_in";
  dc:title "contextualized in - things";
  skos:example "predellas are contextualized in altarpieces",
    "chapters are contextualized in books" ;
  dct:description """[smaller] things - [are] contextualized in - [larger] things.
Example: predellas are contextualized in altarpieces; chapters are contextualized in books""" .


gvp:aat2806_provide_context a owl:ObjectProperty;
  rdfs:isDefinedBy <http://vocab.getty.edu/ontology>, aat: ;
  rdfs:subPropertyOf skos:related;
  rdfs:domain skos:Concept; rdfs:range skos:Concept;
  # domain "things"; range "things";
  dc:identifier "2806";
  skos:prefLabel "aat2806_provide_context";
  dc:title "provide context - things";
  skos:example "altarpieces provide context for predellas",
    "books provide context for chapters" ;
  dct:description """[larger] things - provide context [for] - [smaller] things.
Example: altarpieces provide context for predellas; books provide context for chapters""" .
gvp:aat2805_contextualized_in owl:inverseOf gvp:aat2806_provide_context.


gvp:aat2807_derived_from_common_source a owl:ObjectProperty;
  rdfs:isDefinedBy <http://vocab.getty.edu/ontology>, aat: ;
  rdfs:subPropertyOf skos:related;
  rdfs:domain skos:Concept; rdfs:range skos:Concept;
  # domain "material"; range "material";
  dc:identifier "2807";
  skos:prefLabel "aat2807_derived_from_common_source";
  dc:title "derived from common source - material";
  skos:example "malachite (mineral) is derived from common source with azurite (mineral)",
    "mustard(material) is derived from common source with mustard oil" ;
  dct:description """material - [is] derived from common source [as] - material.
Example: malachite (mineral) is derived from common source with azurite (mineral); mustard(material) is derived from common source with mustard oil""" .
gvp:aat2807_derived_from_common_source a owl:SymmetricProperty.


gvp:aat2809_coexisted_with a owl:ObjectProperty;
  rdfs:isDefinedBy <http://vocab.getty.edu/ontology>, aat: ;
  rdfs:subPropertyOf skos:related;
  rdfs:domain skos:Concept; rdfs:range skos:Concept;
  # domain "style/period/culture"; range "style/period/culture";
  dc:identifier "2809";
  skos:prefLabel "aat2809_coexisted_with";
  dc:title "coexisted with - style/period/culture";
  skos:example "Sangoan coexisted with Fauresmith",
    "Early Minoan coexisted with Prepalatial" ;
  dct:description """style/period/culture/[religion/ideology] - coexisted with -  style/period/culture/[religion/ideology].
Example: Sangoan coexisted with Fauresmith; Early Minoan coexisted with Prepalatial""" .
gvp:aat2809_coexisted_with a owl:SymmetricProperty.


gvp:aat2811_preceded a owl:ObjectProperty;
  rdfs:isDefinedBy <http://vocab.getty.edu/ontology>, aat: ;
  rdfs:subPropertyOf skos:related;
  rdfs:domain skos:Concept; rdfs:range skos:Concept;
  # domain "style/period/culture"; range "style/period/culture";
  dc:identifier "2811";
  skos:prefLabel "aat2811_preceded";
  dc:title "preceded - style/period/culture";
  skos:example "Impressionist preceded Abstract Impressionist",
    "Acheulian preceded Micoquian" ;
  dct:description """style/period/culture/[religion/ideology] - preceded  - style/period/culture/[religion/ideology].
Example: Impressionist preceded Abstract Impressionist; Acheulian preceded Micoquian""" .


gvp:aat2812_followed a owl:ObjectProperty;
  rdfs:isDefinedBy <http://vocab.getty.edu/ontology>, aat: ;
  rdfs:subPropertyOf skos:related;
  rdfs:domain skos:Concept; rdfs:range skos:Concept;
  # domain "style/period/culture"; range "style/period/culture";
  dc:identifier "2812";
  skos:prefLabel "aat2812_followed";
  dc:title "followed - style/period/culture";
  skos:example "Abstract Impressionism followed Impressionist",
    "Micoquian followed Acheulian" ;
  dct:description """style/period/culture/[religion/ideology] - followed  - style/period/culture/[religion/ideology].
Example: Abstract Impressionism followed Impressionist; Micoquian followed Acheulian""" .
gvp:aat2811_preceded owl:inverseOf gvp:aat2812_followed.


gvp:aat2814_constituent_of a owl:ObjectProperty;
  rdfs:isDefinedBy <http://vocab.getty.edu/ontology>, aat: ;
  rdfs:subPropertyOf skos:related;
  rdfs:domain skos:Concept; rdfs:range skos:Concept;
  # domain "material"; range "material";
  dc:identifier "2814";
  skos:prefLabel "aat2814_constituent_of";
  dc:title "constituent of - material";
  skos:example "titanium white is a constituent of composite white",
    "iron oxide is a constituent of desert varnish" ;
  dct:description """material - [is] constituent of - material.
Example: titanium white is a constituent of composite white; iron oxide is a constituent of desert varnish""" .


gvp:aat2815_composed_of a owl:ObjectProperty;
  rdfs:isDefinedBy <http://vocab.getty.edu/ontology>, aat: ;
  rdfs:subPropertyOf skos:related;
  rdfs:domain skos:Concept; rdfs:range skos:Concept;
  # domain "material"; range "material";
  dc:identifier "2815";
  skos:prefLabel "aat2815_composed_of";
  dc:title "composed of - material";
  skos:example "composite white is composed of titanium white",
    "desert varnish is composed of iron oxide" ;
  dct:description """material - [is] composed of - material.
Example: composite white is composed of titanium white; desert varnish is composed of iron oxide""" .
gvp:aat2814_constituent_of owl:inverseOf gvp:aat2815_composed_of.


gvp:aat2817_derived-made_from a owl:ObjectProperty;
  rdfs:isDefinedBy <http://vocab.getty.edu/ontology>, aat: ;
  rdfs:subPropertyOf skos:related;
  rdfs:domain skos:Concept; rdfs:range skos:Concept;
  # domain "material"; range "material";
  dc:identifier "2817";
  skos:prefLabel "aat2817_derived-made_from";
  dc:title "derived/made from - material";
  skos:example "gypsum is derived/made from from anhydrite",
    "wood board is derived/made from timber (lumber)" ;
  dct:description """material - [is] derived/made from - material.
Example: gypsum is derived/made from from anhydrite; wood board is derived/made from timber (lumber)""" .


gvp:aat2818_source_for a owl:ObjectProperty;
  rdfs:isDefinedBy <http://vocab.getty.edu/ontology>, aat: ;
  rdfs:subPropertyOf skos:related;
  rdfs:domain skos:Concept; rdfs:range skos:Concept;
  # domain "material"; range "material";
  dc:identifier "2818";
  skos:prefLabel "aat2818_source_for";
  dc:title "source for - material";
  skos:example "anhydrite is the source for gypsum",
    "timber (lumber) is the source for wood board" ;
  dct:description """material - [is] source for - material.
Example: anhydrite is the source for gypsum; timber (lumber) is the source for wood board""" .
gvp:aat2817_derived-made_from owl:inverseOf gvp:aat2818_source_for.


gvp:aat2821_based_on a owl:ObjectProperty;
  rdfs:isDefinedBy <http://vocab.getty.edu/ontology>, aat: ;
  rdfs:subPropertyOf skos:related;
  rdfs:domain skos:Concept; rdfs:range skos:Concept;
  # domain "any"; range "any";
  dc:identifier "2821";
  skos:prefLabel "aat2821_based_on";
  dc:title "based on - any";
  skos:example "Neo-Gothic is based on Gothic (Medieval)",
    "curved [form attribute] is based on curves (geometric figures)",
    "pencils are based on plummets" ;
  dct:description """any - [is] based on - any.
Example: Neo-Gothic is based on Gothic (Medieval); curved [form attribute] is based on curves (geometric figures); pencils are based on plummets""" .


gvp:aat2822_basis_of a owl:ObjectProperty;
  rdfs:isDefinedBy <http://vocab.getty.edu/ontology>, aat: ;
  rdfs:subPropertyOf skos:related;
  rdfs:domain skos:Concept; rdfs:range skos:Concept;
  # domain "any"; range "any";
  dc:identifier "2822";
  skos:prefLabel "aat2822_basis_of";
  dc:title "basis of - any";
  skos:example "Gothic (Medieval) is the basis of Neo-Gothic",
    "curves (geometric figures) are the basis of curved [form attribute]",
    "plummets are the basis of pencils" ;
  dct:description """any - [is] basis of - any.
Example: Gothic (Medieval) is the basis of Neo-Gothic; curves (geometric figures) are the basis of curved [form attribute]; plummets are the basis of pencils""" .
gvp:aat2821_based_on owl:inverseOf gvp:aat2822_basis_of.


gvp:aat2824_has_parallels_with a owl:ObjectProperty;
  rdfs:isDefinedBy <http://vocab.getty.edu/ontology>, aat: ;
  rdfs:subPropertyOf skos:related;
  rdfs:domain skos:Concept; rdfs:range skos:Concept;
  # domain "style/period/culture"; range "style/period/culture";
  dc:identifier "2824";
  skos:prefLabel "aat2824_has_parallels_with";
  dc:title "has parallels with - style/period/culture";
  skos:example "Lagozza [culture] has parallels with Chasseen [culture]",
    "Gnathian (pottery style) has parallels with West Slope (pottery style)" ;
  dct:description """style/period/culture/[religion/ideology] - has parallels with - style/period/culture/[religion/ideology].
Example: Lagozza [culture] has parallels with Chasseen [culture];  Gnathian (pottery style) has parallels with West Slope (pottery style)""" .
gvp:aat2824_has_parallels_with a owl:SymmetricProperty.


gvp:aat2826_used_with a owl:ObjectProperty;
  rdfs:isDefinedBy <http://vocab.getty.edu/ontology>, aat: ;
  rdfs:subPropertyOf skos:related;
  rdfs:domain skos:Concept; rdfs:range skos:Concept;
  # domain "material"; range "material";
  dc:identifier "2826";
  skos:prefLabel "aat2826_used_with";
  dc:title "used with - material";
  skos:example "watercolor paper is used with watercolor (paint)",
    "arriccio is used with intonaco" ;
  dct:description """material - [is] used with - material.
Example: watercolor paper is used with watercolor (paint); arriccio is used with intonaco""" .
gvp:aat2826_used_with a owl:SymmetricProperty.


gvp:aat2828_use-require a owl:ObjectProperty;
  rdfs:isDefinedBy <http://vocab.getty.edu/ontology>, aat: ;
  rdfs:subPropertyOf skos:related;
  rdfs:domain skos:Concept; rdfs:range skos:Concept;
  # domain "things"; range "material";
  dc:identifier "2828";
  skos:prefLabel "aat2828_use-require";
  dc:title "use/require - material";
  skos:example "oil paintings use/require varnish",
    "wine glasses use/require wine" ;
  dct:description """things - use/require - material.
Example: oil paintings use/require varnish; wine glasses use/require wine""" .


gvp:aat2829_used-required_for a owl:ObjectProperty;
  rdfs:isDefinedBy <http://vocab.getty.edu/ontology>, aat: ;
  rdfs:subPropertyOf skos:related;
  rdfs:domain skos:Concept; rdfs:range skos:Concept;
  # domain "material"; range "things";
  dc:identifier "2829";
  skos:prefLabel "aat2829_used-required_for";
  dc:title "used/required for - things";
  skos:example "varnish is used/required for oil paintings",
    "wine is required/used for wine glasses" ;
  dct:description """material - [is] required/used for - things.
Example: varnish is used/required for oil paintings; wine is required/used for wine glasses""" .
gvp:aat2828_use-require owl:inverseOf gvp:aat2829_used-required_for.


gvp:aat2831_associated_with a owl:ObjectProperty;
  rdfs:isDefinedBy <http://vocab.getty.edu/ontology>, aat: ;
  rdfs:subPropertyOf skos:related;
  rdfs:domain skos:Concept; rdfs:range skos:Concept;
  # domain "genus/species"; range "genus/species";
  dc:identifier "2831";
  skos:prefLabel "aat2831_associated_with";
  dc:title "associated with - genus/species";
  skos:example "Anthonomus grandis (species) [boll weevil] is associated with Gossypium (genus) [cotton]",
    "Amphiprioninae (subfamily) [clown fish] is associated with Actiniaria (order) [sea anemone]" ;
  dct:description """genus/species/[other living organism term] - [is] associated with - genus/species.
Example: Anthonomus grandis (species) [boll weevil] is associated with Gossypium (genus) [cotton]; Amphiprioninae (subfamily) [clown fish] is associated with Actiniaria (order) [sea anemone]""" .
gvp:aat2831_associated_with a owl:SymmetricProperty.


gvp:aat2833_ancestor_of a owl:ObjectProperty;
  rdfs:isDefinedBy <http://vocab.getty.edu/ontology>, aat: ;
  rdfs:subPropertyOf skos:related;
  rdfs:domain skos:Concept; rdfs:range skos:Concept;
  # domain "genus/species"; range "genus/species";
  dc:identifier "2833";
  skos:prefLabel "aat2833_ancestor_of";
  dc:title "ancestor of - genus/species";
  skos:example "Canis lupus is the ancestor of Canis familiaris",
    "Equus asinus is the ancestor of donkeys" ;
  dct:description """genus/species - is ancestor of -  another genus/species.
Example: Canis lupus is the ancestor of Canis familiaris; Equus asinus is the ancestor of donkeys""" .


gvp:aat2834_decendant_of a owl:ObjectProperty;
  rdfs:isDefinedBy <http://vocab.getty.edu/ontology>, aat: ;
  rdfs:subPropertyOf skos:related;
  rdfs:domain skos:Concept; rdfs:range skos:Concept;
  # domain "genus/species"; range "genus/species";
  dc:identifier "2834";
  skos:prefLabel "aat2834_decendant_of";
  dc:title "decendant of - genus/species";
  skos:example "Canis familiaris is the descendant of Canis lupus",
    "donkeys are the descendents of Equus asinus" ;
  dct:description """genus/species - is decendant of -  genus/species.
Example: Canis familiaris is the descendant of Canis lupus; donkeys are the descendents of Equus asinus""" .
gvp:aat2833_ancestor_of owl:inverseOf gvp:aat2834_decendant_of.


gvp:aat2836_derived-made_from a owl:ObjectProperty;
  rdfs:isDefinedBy <http://vocab.getty.edu/ontology>, aat: ;
  rdfs:subPropertyOf skos:related;
  rdfs:domain skos:Concept; rdfs:range skos:Concept;
  # domain "things"; range "genus/species";
  dc:identifier "2836";
  skos:prefLabel "aat2836_derived-made_from";
  dc:title "derived/made from - genus/species";
  skos:example "k?kaku are derived/made from Phormium tenax (species)",
    "ostrich-egg cups are derived/made from Struthio camelus (species)" ;
  dct:description """things - [are] derived/made from - genus/species [or its parts].
Example: k?kaku are derived/made from Phormium tenax (species); ostrich-egg cups are derived/made from Struthio camelus (species)""" .


gvp:aat2837_source_for a owl:ObjectProperty;
  rdfs:isDefinedBy <http://vocab.getty.edu/ontology>, aat: ;
  rdfs:subPropertyOf skos:related;
  rdfs:domain skos:Concept; rdfs:range skos:Concept;
  # domain "genus/species"; range "things";
  dc:identifier "2837";
  skos:prefLabel "aat2837_source_for";
  dc:title "source for - things";
  skos:example "Phormium tenax (species) is the source for k?kaku",
    "Struthio camelus(species) is the source for ostrich-egg cups" ;
  dct:description """genus/species [or its parts] - [is] source for - things.
Example: Phormium tenax (species) is the source for k?kaku; Struthio camelus(species) is the source for ostrich-egg cups""" .
gvp:aat2836_derived-made_from owl:inverseOf gvp:aat2837_source_for.


gvp:aat2841_derived-made_from a owl:ObjectProperty;
  rdfs:isDefinedBy <http://vocab.getty.edu/ontology>, aat: ;
  rdfs:subPropertyOf skos:related;
  rdfs:domain skos:Concept; rdfs:range skos:Concept;
  # domain "material"; range "genus/species";
  dc:identifier "2841";
  skos:prefLabel "aat2841_derived-made_from";
  dc:title "derived/made from - genus/species";
  skos:example "alpaca (wool) is derived from Vicugna pacos (species)",
    "maple (wood) is derived from Acer (genus)" ;
  dct:description """material - [is] derived/made from - genus/species.
Example: alpaca (wool) is derived from Vicugna pacos (species); maple (wood) is derived from Acer (genus)""" .


gvp:aat2842_source_for a owl:ObjectProperty;
  rdfs:isDefinedBy <http://vocab.getty.edu/ontology>, aat: ;
  rdfs:subPropertyOf skos:related;
  rdfs:domain skos:Concept; rdfs:range skos:Concept;
  # domain "genus/species"; range "material";
  dc:identifier "2842";
  skos:prefLabel "aat2842_source_for";
  dc:title "source for - material";
  skos:example "Vicugna pacos (species) is the source for alpaca (wool)",
    "Acer (genus) is the source for maple (wood)" ;
  dct:description """genus/species - [is] source for - material.
Example: Vicugna pacos (species) is the source for alpaca (wool); Acer (genus) is the source for maple (wood)""" .
gvp:aat2841_derived-made_from owl:inverseOf gvp:aat2842_source_for.


gvp:aat2845_used-located_in a owl:ObjectProperty;
  rdfs:isDefinedBy <http://vocab.getty.edu/ontology>, aat: ;
  rdfs:subPropertyOf skos:related;
  rdfs:domain skos:Concept; rdfs:range skos:Concept;
  # domain "genus/species"; range "locus/setting";
  dc:identifier "2845";
  skos:prefLabel "aat2845_used-located_in";
  dc:title "used/located in - locus/setting";
  skos:example "Elephantidae(family) are used/located in elephant houses",
    "Vitaceae (family) is used/located in vineyards" ;
  dct:description """genus/species - [is] used/located in -  locus/setting.
Example: Elephantidae(family) are used/located in elephant houses; Vitaceae (family) is used/located in vineyards""" .


gvp:aat2846_locus-setting_for a owl:ObjectProperty;
  rdfs:isDefinedBy <http://vocab.getty.edu/ontology>, aat: ;
  rdfs:subPropertyOf skos:related;
  rdfs:domain skos:Concept; rdfs:range skos:Concept;
  # domain "locus/setting"; range "genus/species";
  dc:identifier "2846";
  skos:prefLabel "aat2846_locus-setting_for";
  dc:title "locus/setting for - genus/species";
  skos:example "elephant houses are the locus/setting for Elephantidae(family)",
    "vineyards are the locus/setting of Vitaceae (family)" ;
  dct:description """locus/setting - [is] locus/setting for - genus/species.
Example: elephant houses are the locus/setting for Elephantidae(family); vineyards are the locus/setting of Vitaceae (family)""" .
gvp:aat2845_used-located_in owl:inverseOf gvp:aat2846_locus-setting_for.


gvp:aat2848_involved_in a owl:ObjectProperty;
  rdfs:isDefinedBy <http://vocab.getty.edu/ontology>, aat: ;
  rdfs:subPropertyOf skos:related;
  rdfs:domain skos:Concept; rdfs:range skos:Concept;
  # domain "genus/species"; range "activity/event";
  dc:identifier "2848";
  skos:prefLabel "aat2848_involved_in";
  dc:title "involved in - activity/event";
  skos:example "bulls (animals) are involved in bullfighting",
    "Equus caballus (species) is involved in polo(field sport)" ;
  dct:description """genus/species - is involved in - activity/event.
Example: bulls (animals) are involved in bullfighting; Equus caballus (species) is involved in polo(field sport)""" .


gvp:aat2849_involves a owl:ObjectProperty;
  rdfs:isDefinedBy <http://vocab.getty.edu/ontology>, aat: ;
  rdfs:subPropertyOf skos:related;
  rdfs:domain skos:Concept; rdfs:range skos:Concept;
  # domain "activity/event"; range "genus/species";
  dc:identifier "2849";
  skos:prefLabel "aat2849_involves";
  dc:title "involves - genus/species";
  skos:example "bullfighting involves bulls (animals)",
    "polo (field sport) involves Equus caballus (species)" ;
  dct:description """activity/event - involves - genus/species.
Example: bullfighting involves bulls (animals); polo (field sport) involves Equus caballus (species)""" .
gvp:aat2848_involved_in owl:inverseOf gvp:aat2849_involves.


gvp:aat2852_involved_with a owl:ObjectProperty;
  rdfs:isDefinedBy <http://vocab.getty.edu/ontology>, aat: ;
  rdfs:subPropertyOf skos:related;
  rdfs:domain skos:Concept; rdfs:range skos:Concept;
  # domain "genus/species"; range "things";
  dc:identifier "2852";
  skos:prefLabel "aat2852_involved_with";
  dc:title "involved with - things";
  skos:example "Rosa (genus) is involved with rose bowls",
    "Camelus (genus) is involved with camel saddles" ;
  dct:description """genus/species - [is] involved with - things/[equipment].
Example: Rosa (genus) is involved with rose bowls; Camelus (genus) is involved with camel saddles""" .


gvp:aat2853_involve a owl:ObjectProperty;
  rdfs:isDefinedBy <http://vocab.getty.edu/ontology>, aat: ;
  rdfs:subPropertyOf skos:related;
  rdfs:domain skos:Concept; rdfs:range skos:Concept;
  # domain "things"; range "genus/species";
  dc:identifier "2853";
  skos:prefLabel "aat2853_involve";
  dc:title "involve - genus/species";
  skos:example "rose bowls involve Rosa (genus)",
    "camel saddles involve Camelus (genus)" ;
  dct:description """things/[equipment] - involve - genus/species.
Example: rose bowls involve Rosa (genus); camel saddles involve Camelus (genus)""" .
gvp:aat2852_involved_with owl:inverseOf gvp:aat2853_involve.


gvp:aat2875_characteristic_of a owl:ObjectProperty;
  rdfs:isDefinedBy <http://vocab.getty.edu/ontology>, aat: ;
  rdfs:subPropertyOf skos:related;
  rdfs:domain skos:Concept; rdfs:range skos:Concept;
  # domain "language"; range "style/period/culture";
  dc:identifier "2875";
  skos:prefLabel "aat2875_characteristic_of";
  dc:title "characteristic of - style/period/culture";
  skos:example "Afar (language) is characteristic of Afar (culture)",
    "Celtic (language) was characteristic of Celtic (culture)" ;
  dct:description """language - [is] characteristic of - style/period/culture.
Example: Afar (language) is characteristic of Afar (culture); Celtic (language) was characteristic of Celtic (culture)""" .


gvp:aat2876_characterized_by a owl:ObjectProperty;
  rdfs:isDefinedBy <http://vocab.getty.edu/ontology>, aat: ;
  rdfs:subPropertyOf skos:related;
  rdfs:domain skos:Concept; rdfs:range skos:Concept;
  # domain "style/period/culture"; range "language";
  dc:identifier "2876";
  skos:prefLabel "aat2876_characterized_by";
  dc:title "characterized by - language";
  skos:example "Afar (culture) is characterized by Afar (language)",
    "Celtic (culture) is characterized by Celtic (language)" ;
  dct:description """style/period/culture - [is] characterized by - language.
Example: Afar (culture) is characterized by Afar (language); Celtic (culture) is characterized by Celtic (language)""" .
gvp:aat2875_characteristic_of owl:inverseOf gvp:aat2876_characterized_by.


gvp:aat2878_preceded-source_for a owl:ObjectProperty;
  rdfs:isDefinedBy <http://vocab.getty.edu/ontology>, aat: ;
  rdfs:subPropertyOf skos:related;
  rdfs:domain skos:Concept; rdfs:range skos:Concept;
  # domain "language"; range "language";
  dc:identifier "2878";
  skos:prefLabel "aat2878_preceded-source_for";
  dc:title "preceded/source for - language";
  skos:example "Ancient Greek (language) preceded/is source for Greek (modern language)",
    "Ancient Egyptian (language) preceded/is source for Egyptian, Coptic (language)" ;
  dct:description """language - preceded/[is] source for - language.
Example: Ancient Greek (language) preceded/is source for Greek (modern language); Ancient Egyptian (language) preceded/is source for Egyptian, Coptic (language)""" .


gvp:aat2879_followed-developed_from a owl:ObjectProperty;
  rdfs:isDefinedBy <http://vocab.getty.edu/ontology>, aat: ;
  rdfs:subPropertyOf skos:related;
  rdfs:domain skos:Concept; rdfs:range skos:Concept;
  # domain "language"; range "language";
  dc:identifier "2879";
  skos:prefLabel "aat2879_followed-developed_from";
  dc:title "followed/developed from - language";
  skos:example "Greek (modern language) followed/developed from Ancient Greek (language)",
    "Egyptian, Coptic (language) followed/developed from Ancient Egyptian (language)" ;
  dct:description """language - followed/developed from - language.
Example: Greek (modern language) followed/developed from Ancient Greek (language); Egyptian, Coptic (language) followed/developed from Ancient Egyptian (language)""" .
gvp:aat2878_preceded-source_for owl:inverseOf gvp:aat2879_followed-developed_from.


gvp:aat2881_reflected_in a owl:ObjectProperty;
  rdfs:isDefinedBy <http://vocab.getty.edu/ontology>, aat: ;
  rdfs:subPropertyOf skos:related;
  rdfs:domain skos:Concept; rdfs:range skos:Concept;
  # domain "language"; range "things";
  dc:identifier "2881";
  skos:prefLabel "aat2881_reflected_in";
  dc:title "reflected in - things";
  skos:example "Greek (language) is reflected in Greek alphabet",
    "Sanskrit is reflected in Vedas" ;
  dct:description """language - [is] reflected in - things.
Example: Greek (language) is reflected in Greek alphabet; Sanskrit is reflected in Vedas""" .


gvp:aat2882_reflect a owl:ObjectProperty;
  rdfs:isDefinedBy <http://vocab.getty.edu/ontology>, aat: ;
  rdfs:subPropertyOf skos:related;
  rdfs:domain skos:Concept; rdfs:range skos:Concept;
  # domain "things"; range "language";
  dc:identifier "2882";
  skos:prefLabel "aat2882_reflect";
  dc:title "reflect - language";
  skos:example "Greek alphabet reflects Greek (language)",
    "Vedas reflect Sanskrit" ;
  dct:description """things - reflect - language.
Example: Greek alphabet reflects Greek (language); Vedas reflect Sanskrit""" .
gvp:aat2881_reflected_in owl:inverseOf gvp:aat2882_reflect.


gvp:aat2884_involved_with a owl:ObjectProperty;
  rdfs:isDefinedBy <http://vocab.getty.edu/ontology>, aat: ;
  rdfs:subPropertyOf skos:related;
  rdfs:domain skos:Concept; rdfs:range skos:Concept;
  # domain "attributes /associated concepts"; range "any";
  dc:identifier "2884";
  skos:prefLabel "aat2884_involved_with";
  dc:title "involved with - any";
  skos:example "climate is involved with climate change",
    "insect damage is involved with infestation",
    "Celtic crosses (design motif) are involved with Celtic culture" ;
  dct:description """attributes /associated concepts - [are] involved with - any.
Example: climate is involved with climate change; insect damage is involved with infestation; Celtic crosses (design motif) are involved with Celtic culture""" .


gvp:aat2885_involves a owl:ObjectProperty;
  rdfs:isDefinedBy <http://vocab.getty.edu/ontology>, aat: ;
  rdfs:subPropertyOf skos:related;
  rdfs:domain skos:Concept; rdfs:range skos:Concept;
  # domain "any"; range "attributes /associated concepts";
  dc:identifier "2885";
  skos:prefLabel "aat2885_involves";
  dc:title "involves - attributes /associated concepts";
  skos:example "climate change involves climate",
    "infestation involves insect damage",
    "Celtic culture involves Celtic crosses (design motif)" ;
  dct:description """any - involves - attributes /associated concepts.
Example: climate change involves climate;  infestation involves insect damage; Celtic culture involves Celtic crosses (design motif)""" .
gvp:aat2884_involved_with owl:inverseOf gvp:aat2885_involves.


gvp:aat2886_used-function_as a owl:ObjectProperty;
  rdfs:isDefinedBy <http://vocab.getty.edu/ontology>, aat: ;
  rdfs:subPropertyOf skos:related;
  rdfs:domain skos:Concept; rdfs:range skos:Concept;
  # domain "material"; range "material";
  dc:identifier "2886";
  skos:prefLabel "aat2886_used-function_as";
  dc:title "used/function as - material";
  skos:example "carbon disulfide - is used/functions as - solvent" ;
  dct:description """material - used/function as - material.
Example: carbon disulfide - is used/functions as - solvent""" .


gvp:aat2887_exemplified_by a owl:ObjectProperty;
  rdfs:isDefinedBy <http://vocab.getty.edu/ontology>, aat: ;
  rdfs:subPropertyOf skos:related;
  rdfs:domain skos:Concept; rdfs:range skos:Concept;
  # domain "material"; range "material";
  dc:identifier "2887";
  skos:prefLabel "aat2887_exemplified_by";
  dc:title "exemplified by - material";
  skos:example "solvent - exemplified by - carbon disulfide" ;
  dct:description """material - exemplified by - material.
Example: solvent - exemplified by - carbon disulfide""" .
gvp:aat2886_used-function_as owl:inverseOf gvp:aat2887_exemplified_by.


gvp:aat2891_exemplified_by a owl:ObjectProperty;
  rdfs:isDefinedBy <http://vocab.getty.edu/ontology>, aat: ;
  rdfs:subPropertyOf skos:related;
  rdfs:domain skos:Concept; rdfs:range skos:Concept;
  # domain "things"; range "brand name";
  dc:identifier "2891";
  skos:prefLabel "aat2891_exemplified_by";
  dc:title "exemplified by - brand name";
  skos:example "photothermographic transfer prints are exemplified by Pictrography (TM) prints" ;
  dct:description """things - [are] exemplied by - brand name.
Example: photothermographic transfer prints are exemplified by Pictrography (TM) prints""" .


gvp:aat2892_example_of a owl:ObjectProperty;
  rdfs:isDefinedBy <http://vocab.getty.edu/ontology>, aat: ;
  rdfs:subPropertyOf skos:related;
  rdfs:domain skos:Concept; rdfs:range skos:Concept;
  # domain "brand name"; range "things";
  dc:identifier "2892";
  skos:prefLabel "aat2892_example_of";
  dc:title "example of - things";
  skos:example "Pictrography (TM) prints are examples of photothermographic transfer prints" ;
  dct:description """brand name - [is] example of - things.
Example: Pictrography (TM) prints are examples of photothermographic transfer prints""" .
gvp:aat2891_exemplified_by owl:inverseOf gvp:aat2892_example_of.


gvp:aat2894_exemplified_by a owl:ObjectProperty;
  rdfs:isDefinedBy <http://vocab.getty.edu/ontology>, aat: ;
  rdfs:subPropertyOf skos:related;
  rdfs:domain skos:Concept; rdfs:range skos:Concept;
  # domain "activity/event"; range "brand name";
  dc:identifier "2894";
  skos:prefLabel "aat2894_exemplified_by";
  dc:title "exemplified by - brand name";
  skos:example "deacidification [process/function] is exemplified by Papersave Process (TM)" ;
  dct:description """activity/event/[process/function] - [is] exemplified by - brand name.
Example: deacidification [process/function] is exemplified by Papersave Process (TM)""" .


gvp:aat2895_example_of a owl:ObjectProperty;
  rdfs:isDefinedBy <http://vocab.getty.edu/ontology>, aat: ;
  rdfs:subPropertyOf skos:related;
  rdfs:domain skos:Concept; rdfs:range skos:Concept;
  # domain "brand name"; range "activity/event";
  dc:identifier "2895";
  skos:prefLabel "aat2895_example_of";
  dc:title "example of - activity/event";
  skos:example "Papersave Process (TM) is example of deacidification [process/function]" ;
  dct:description """brand name - [is] example of - activity/event/[process/function].
Example: Papersave Process (TM) is example of deacidification [process/function]""" .
gvp:aat2894_exemplified_by owl:inverseOf gvp:aat2895_example_of.


gvp:aat2900_miscellaneous_relationship a owl:ObjectProperty;
  rdfs:isDefinedBy <http://vocab.getty.edu/ontology>, aat: ;
  rdfs:subPropertyOf skos:related;
  rdfs:domain skos:Concept; rdfs:range skos:Concept;
  # domain "any"; range "any";
  dc:identifier "2900";
  skos:prefLabel "aat2900_miscellaneous_relationship";
  dc:title "miscellaneous relationship - any";
  skos:example "Conditions and Effects has miscellaneous relationship with Processes and Techniques" ;
  dct:description """any - [has] miscellaneous relationship [to] - any.
Example: Conditions and Effects has miscellaneous relationship with Processes and Techniques""" .
gvp:aat2900_miscellaneous_relationship a owl:SymmetricProperty.


gvp:tgn3000_related_to a owl:ObjectProperty;
  rdfs:isDefinedBy <http://vocab.getty.edu/ontology>, tgn: ;
  rdfs:subPropertyOf skos:related;
  rdfs:domain skos:Concept; rdfs:range skos:Concept;
  # domain "any"; range "any";
  dc:identifier "3000";
  skos:prefLabel "tgn3000_related_to";
  dc:title "related to - any";
  skos:example "Fountains Abbey is related to Studley Royal",
    "Austria-Hungary is related to Magyarorszag" ;
  dct:description """any - related to - any.
Example: Fountains Abbey is related to Studley Royal; Austria-Hungary is related to Magyarorszag""" .
gvp:tgn3000_related_to a owl:SymmetricProperty.


gvp:tgn3001_distinguished_from a owl:ObjectProperty;
  rdfs:isDefinedBy <http://vocab.getty.edu/ontology>, tgn: ;
  rdfs:subPropertyOf skos:related;
  rdfs:domain skos:Concept; rdfs:range skos:Concept;
  # domain "any"; range "any";
  dc:identifier "3001";
  skos:prefLabel "tgn3001_distinguished_from";
  dc:title "distinguished from - any";
  skos:example "The Ancient Mesopotamian Kingdom 'Assyria' is distinguished from the Roman Province of the same name" ;
  dct:description """any - distinguished from - any.
Example: The Ancient Mesopotamian Kingdom 'Assyria' is distinguished from the Roman Province of the same name""" .
gvp:tgn3001_distinguished_from a owl:SymmetricProperty.


gvp:tgn3005_possibly_identified_as a owl:ObjectProperty;
  rdfs:isDefinedBy <http://vocab.getty.edu/ontology>, tgn: ;
  rdfs:subPropertyOf skos:related;
  rdfs:domain skos:Concept; rdfs:range skos:Concept;
  # domain "place"; range "place";
  dc:identifier "3005";
  skos:prefLabel "tgn3005_possibly_identified_as";
  dc:title "possibly identified as - place";
  skos:example "The lost settlement of Sharuhen is possibly identified as Tel el-Far'ah (As Suwayda', Syria) (deserted settlement)" ;
  dct:description """place - possibly identified as - place.
Example: The lost settlement of Sharuhen is possibly identified as Tel el-Far'ah (As Suwayda', Syria) (deserted settlement)""" .
gvp:tgn3005_possibly_identified_as a owl:SymmetricProperty.


gvp:tgn3006_formerly_identified_as a owl:ObjectProperty;
  rdfs:isDefinedBy <http://vocab.getty.edu/ontology>, tgn: ;
  rdfs:subPropertyOf skos:related;
  rdfs:domain skos:Concept; rdfs:range skos:Concept;
  # domain "place"; range "place";
  dc:identifier "3006";
  skos:prefLabel "tgn3006_formerly_identified_as";
  dc:title "formerly identified as - place";
  skos:example "The deserted settlement of Machupicchu was formerly identified as Tampu Tocco";
  skos:scopeNote "New" ;
  dct:description """place - formerly identified as - place; New.
Example: The deserted settlement of Machupicchu was formerly identified as Tampu Tocco""" .
gvp:tgn3006_formerly_identified_as a owl:SymmetricProperty.


gvp:tgn3101_near-adjacent_to a owl:ObjectProperty;
  rdfs:isDefinedBy <http://vocab.getty.edu/ontology>, tgn: ;
  rdfs:subPropertyOf skos:related;
  rdfs:domain skos:Concept; rdfs:range skos:Concept;
  # domain "any"; range "any";
  dc:identifier "3101";
  skos:prefLabel "tgn3101_near-adjacent_to";
  dc:title "near/adjacent to - any";
  skos:example "Saint Paul (Minnesota, USA), is linked to its 'Twin City' Minneapolis (Hennepin county, Minnesota, USA)" ;
  dct:description """any - near/adjacent to - any.
Example: Saint Paul (Minnesota, USA), is linked to its 'Twin City' Minneapolis (Hennepin county, Minnesota, USA)""" .
gvp:tgn3101_near-adjacent_to a owl:SymmetricProperty.


gvp:tgn3102_coextensive_with a owl:ObjectProperty;
  rdfs:isDefinedBy <http://vocab.getty.edu/ontology>, tgn: ;
  rdfs:subPropertyOf skos:related;
  rdfs:domain skos:Concept; rdfs:range skos:Concept;
  # domain "place"; range "place";
  dc:identifier "3102";
  skos:prefLabel "tgn3102_coextensive_with";
  dc:title "coextensive with - place";
  skos:example "Kings county (New York, USA) is coextensive with Brooklyn (New York, USA)" ;
  dct:description """place - coextensive with - place.
Example: Kings county (New York, USA) is coextensive with Brooklyn (New York, USA)""" .
gvp:tgn3102_coextensive_with a owl:SymmetricProperty.


gvp:tgn3103_located_on a owl:ObjectProperty;
  rdfs:isDefinedBy <http://vocab.getty.edu/ontology>, tgn: ;
  rdfs:subPropertyOf skos:related;
  rdfs:domain skos:Concept; rdfs:range skos:Concept;
  # domain "place"; range "place";
  dc:identifier "3103";
  skos:prefLabel "tgn3103_located_on";
  dc:title "located on - place";
  skos:example "tgn:7018835 Palmyra is located on tgn:7031416 Silk Road" ;
  dct:description """place - located on - place.
Example: tgn:7018835 Palmyra is located on tgn:7031416 Silk Road""" .


gvp:tgn3104_is_location_of a owl:ObjectProperty;
  rdfs:isDefinedBy <http://vocab.getty.edu/ontology>, tgn: ;
  rdfs:subPropertyOf skos:related;
  rdfs:domain skos:Concept; rdfs:range skos:Concept;
  # domain "place"; range "place";
  dc:identifier "3104";
  skos:prefLabel "tgn3104_is_location_of";
  dc:title "is location of - place";
  skos:example "tgn:7031416 Silk Road is location of tgn:7018835 Palmyra" ;
  dct:description """place - is location of - place.
Example: tgn:7031416 Silk Road is location of tgn:7018835 Palmyra""" .
gvp:tgn3103_located_on owl:inverseOf gvp:tgn3104_is_location_of.


gvp:tgn3110_meaning-usage_overlaps_with a owl:ObjectProperty;
  rdfs:isDefinedBy <http://vocab.getty.edu/ontology>, tgn: ;
  rdfs:subPropertyOf skos:related;
  rdfs:domain skos:Concept; rdfs:range skos:Concept;
  # domain "any"; range "any";
  dc:identifier "3110";
  skos:prefLabel "tgn3110_meaning-usage_overlaps_with";
  dc:title "meaning/usage overlaps with - any";
  skos:example "Judaea (Israel) (historical region) meaning/usage overlaps with Holy Land (Asia) (historical region)" ;
  dct:description """any - meaning/usage overlaps with - any.
Example: Judaea (Israel) (historical region) meaning/usage overlaps with Holy Land (Asia) (historical region)""" .
gvp:tgn3110_meaning-usage_overlaps_with a owl:SymmetricProperty.


gvp:tgn3201_capital_of a owl:ObjectProperty;
  rdfs:isDefinedBy <http://vocab.getty.edu/ontology>, tgn: ;
  rdfs:subPropertyOf skos:related;
  rdfs:domain skos:Concept; rdfs:range skos:Concept;
  # domain "city"; range "nation";
  dc:identifier "3201";
  skos:prefLabel "tgn3201_capital_of";
  dc:title "capital of - nation";
  skos:example "Thecapital of Maxima Caesariensis from 296 to 800 CE was London" ;
  dct:description """city - capital of - nation.
Example: Thecapital of Maxima Caesariensis from 296 to 800 CE was London""" .


gvp:tgn3202_capital_is a owl:ObjectProperty;
  rdfs:isDefinedBy <http://vocab.getty.edu/ontology>, tgn: ;
  rdfs:subPropertyOf skos:related;
  rdfs:domain skos:Concept; rdfs:range skos:Concept;
  # domain "nation"; range "city";
  dc:identifier "3202";
  skos:prefLabel "tgn3202_capital_is";
  dc:title "capital is - city";
  skos:example "London was the capital of Maxima Caesariensis from 296 to 800 CE" ;
  dct:description """nation - capital is - city.
Example: London was the capital of Maxima Caesariensis from 296 to 800 CE""" .
gvp:tgn3201_capital_of owl:inverseOf gvp:tgn3202_capital_is.


gvp:tgn3301_ally_of a owl:ObjectProperty;
  rdfs:isDefinedBy <http://vocab.getty.edu/ontology>, tgn: ;
  rdfs:subPropertyOf skos:related;
  rdfs:domain skos:Concept; rdfs:range skos:Concept;
  # domain "nation"; range "nation";
  dc:identifier "3301";
  skos:prefLabel "tgn3301_ally_of";
  dc:title "ally of - nation";
  skos:example "Siena, Arezzo, Pisa, and Pistoia were Ghibeline allies during the 13th and 14th centuries." ;
  dct:description """nation - ally of - nation.
Example: Siena, Arezzo, Pisa, and Pistoia were Ghibeline allies during the 13th and 14th centuries.""" .
gvp:tgn3301_ally_of a owl:SymmetricProperty.


gvp:tgn3317_member_of a owl:ObjectProperty;
  rdfs:isDefinedBy <http://vocab.getty.edu/ontology>, tgn: ;
  rdfs:subPropertyOf skos:related;
  rdfs:domain skos:Concept; rdfs:range skos:Concept;
  # domain "nation"; range "union";
  dc:identifier "3317";
  skos:prefLabel "tgn3317_member_of";
  dc:title "member of - union";
  skos:example "Austria is a member of the European Union since 1915",
    "Belgium is a member of the European Union since 1958" ;
  dct:description """nation - member of - union.
Example: Austria is a member of the European Union since 1915; Belgium is a member of the European Union since 1958""" .


gvp:tgn3318_member_is a owl:ObjectProperty;
  rdfs:isDefinedBy <http://vocab.getty.edu/ontology>, tgn: ;
  rdfs:subPropertyOf skos:related;
  rdfs:domain skos:Concept; rdfs:range skos:Concept;
  # domain "union"; range "nation";
  dc:identifier "3318";
  skos:prefLabel "tgn3318_member_is";
  dc:title "member is - nation";
  skos:example "Austria is a member of the European Union since 1915",
    "Belgium is a member of the European Union since 1958" ;
  dct:description """union - member is - nation.
Example: Austria is a member of the European Union since 1915; Belgium is a member of the European Union since 1958""" .
gvp:tgn3317_member_of owl:inverseOf gvp:tgn3318_member_is.


gvp:tgn3401_moved_from a owl:ObjectProperty;
  rdfs:isDefinedBy <http://vocab.getty.edu/ontology>, tgn: ;
  rdfs:subPropertyOf skos:related;
  rdfs:domain skos:Concept; rdfs:range skos:Concept;
  # domain "place"; range "place";
  dc:identifier "3401";
  skos:prefLabel "tgn3401_moved_from";
  dc:title "moved from - place";
  skos:example "Troupville, Georgia, USA was moved to Valdosta (Lowndes county, Georgia, USA)";
  skos:scopeNote "Note: places that were physically moved from one location to another, often due to the threat or occurrence of natural disaster." ;
  dct:description """place - moved from - place; Note: places that were physically moved from one location to another, often due to the threat or occurrence of natural disaster..
Example: Troupville, Georgia, USA was moved to Valdosta (Lowndes county, Georgia, USA)""" .


gvp:tgn3402_moved_to a owl:ObjectProperty;
  rdfs:isDefinedBy <http://vocab.getty.edu/ontology>, tgn: ;
  rdfs:subPropertyOf skos:related;
  rdfs:domain skos:Concept; rdfs:range skos:Concept;
  # domain "place"; range "place";
  dc:identifier "3402";
  skos:prefLabel "tgn3402_moved_to";
  dc:title "moved to - place";
  skos:example "Valdosta (Lowndes county, Georgia, USA) moved from Troupville (Georgia, USA)" ;
  dct:description """place - moved to - place.
Example: Valdosta (Lowndes county, Georgia, USA) moved from Troupville (Georgia, USA)""" .
gvp:tgn3401_moved_from owl:inverseOf gvp:tgn3402_moved_to.


gvp:tgn3411_successor_of a owl:ObjectProperty;
  rdfs:isDefinedBy <http://vocab.getty.edu/ontology>, tgn: ;
  rdfs:subPropertyOf skos:related;
  rdfs:domain skos:Concept; rdfs:range skos:Concept;
  # domain "nation"; range "nation";
  dc:identifier "3411";
  skos:prefLabel "tgn3411_successor_of";
  dc:title "successor of - nation";
  skos:example "Iran (nation) is the successor of Persia" ;
  dct:description """nation - successor of - nation.
Example: Iran (nation) is the successor of Persia""" .


gvp:tgn3412_predecessor_of a owl:ObjectProperty;
  rdfs:isDefinedBy <http://vocab.getty.edu/ontology>, tgn: ;
  rdfs:subPropertyOf skos:related;
  rdfs:domain skos:Concept; rdfs:range skos:Concept;
  # domain "nation"; range "nation";
  dc:identifier "3412";
  skos:prefLabel "tgn3412_predecessor_of";
  dc:title "predecessor of - nation";
  skos:example "Persia is the predecessor of Iran (nation)" ;
  dct:description """nation - predecessor of - nation.
Example: Persia is the predecessor of Iran (nation)""" .
gvp:tgn3411_successor_of owl:inverseOf gvp:tgn3412_predecessor_of.


gvp:tgn3510_historical_connection a owl:ObjectProperty;
  rdfs:isDefinedBy <http://vocab.getty.edu/ontology>, tgn: ;
  rdfs:subPropertyOf skos:related;
  rdfs:domain skos:Concept; rdfs:range skos:Concept;
  # domain "any"; range "any";
  dc:identifier "3510";
  skos:prefLabel "tgn3510_historical_connection";
  dc:title "historical connection - any";
  skos:example "Guyenne, France (historical region) has a historical connection to Gascogne (France) (historical region)" ;
  dct:description """any - historical connection - any.
Example: Guyenne, France (historical region) has a historical connection to Gascogne (France) (historical region)""" .
gvp:tgn3510_historical_connection a owl:SymmetricProperty.


gvp:tgn3611_administrative_dependent_of a owl:ObjectProperty;
  rdfs:isDefinedBy <http://vocab.getty.edu/ontology>, tgn: ;
  rdfs:subPropertyOf skos:related;
  rdfs:domain skos:Concept; rdfs:range skos:Concept;
  # domain "place"; range "place";
  dc:identifier "3611";
  skos:prefLabel "tgn3611_administrative_dependent_of";
  dc:title "administrative dependent of - place";
  skos:example "Luni (La Spezia province, Liguria, Italy) is the admisistrative dependent of Ortonovo (Massa-Carrara province, Tuscany, Italy)";
  skos:scopeNote "New" ;
  dct:description """place - administrative dependent of - place; New.
Example: Luni (La Spezia province, Liguria, Italy) is the admisistrative dependent of Ortonovo (Massa-Carrara province, Tuscany, Italy)""" .


gvp:tgn3612_administrative_entity_for a owl:ObjectProperty;
  rdfs:isDefinedBy <http://vocab.getty.edu/ontology>, tgn: ;
  rdfs:subPropertyOf skos:related;
  rdfs:domain skos:Concept; rdfs:range skos:Concept;
  # domain "place"; range "place";
  dc:identifier "3612";
  skos:prefLabel "tgn3612_administrative_entity_for";
  dc:title "administrative entity for - place";
  skos:example "Ortonovo (Massa-Carra province, Tuscany, Italy) is the administrative entity for Luni (La Spezia province, Liguria, Italy)" ;
  dct:description """place - administrative entity for - place.
Example: Ortonovo (Massa-Carra province, Tuscany, Italy) is the administrative entity for Luni (La Spezia province, Liguria, Italy)""" .
gvp:tgn3611_administrative_dependent_of owl:inverseOf gvp:tgn3612_administrative_entity_for.


gvp:ulan1000_related_to a owl:ObjectProperty;
  rdfs:isDefinedBy <http://vocab.getty.edu/ontology>, ulan: ;
  rdfs:subPropertyOf skos:related;
  rdfs:domain skos:Concept; rdfs:range skos:Concept;
  # domain "any"; range "any";
  dc:identifier "1000";
  skos:prefLabel "ulan1000_related_to";
  dc:title "related to - any";
  skos:example "Frank Lloyd Wright is related to Francis Conroy Sullivan",
    "Herman Miller, Inc. is related to Irving Harper",
    "National Endowment for the Humanities is related to Connecticut Humanities Council" ;
  dct:description """any - related to - any.
Example: Frank Lloyd Wright is related to Francis Conroy Sullivan; Herman Miller, Inc. is related to Irving Harper; National Endowment for the Humanities is related to Connecticut Humanities Council""" .
gvp:ulan1000_related_to a owl:SymmetricProperty.


gvp:ulan1003_associated_with a owl:ObjectProperty;
  rdfs:isDefinedBy <http://vocab.getty.edu/ontology>, ulan: ;
  rdfs:subPropertyOf skos:related;
  rdfs:domain skos:Concept; rdfs:range skos:Concept;
  # domain "any"; range "any";
  dc:identifier "1003";
  skos:prefLabel "ulan1003_associated_with";
  dc:title "associated with - any";
  skos:example "Richard Meier is associated with Renny B.Saltzman",
    "United Nations is associated with World Bank" ;
  dct:description """any - associated with - any.
Example: Richard Meier is associated with Renny B.Saltzman; United Nations is associated with World Bank""" .
gvp:ulan1003_associated_with a owl:SymmetricProperty.


gvp:ulan1005_possibly_identified_with a owl:ObjectProperty;
  rdfs:isDefinedBy <http://vocab.getty.edu/ontology>, ulan: ;
  rdfs:subPropertyOf skos:related;
  rdfs:domain skos:Concept; rdfs:range skos:Concept;
  # domain "any"; range "any";
  dc:identifier "1005";
  skos:prefLabel "ulan1005_possibly_identified_with";
  dc:title "possibly identified with - any";
  skos:example "Master of the Saint John Altarpiece is possibly identified with Hughe Jacobsz",
    "Bauart is possibly identified with Gruppe BAUart" ;
  dct:description """any - possibly identified with - any.
Example: Master of the Saint John Altarpiece is possibly identified with Hughe Jacobsz; Bauart is possibly identified with Gruppe BAUart""" .
gvp:ulan1005_possibly_identified_with a owl:SymmetricProperty.


gvp:ulan1006_formerly_identified_with a owl:ObjectProperty;
  rdfs:isDefinedBy <http://vocab.getty.edu/ontology>, ulan: ;
  rdfs:subPropertyOf skos:related;
  rdfs:domain skos:Concept; rdfs:range skos:Concept;
  # domain "any"; range "any";
  dc:identifier "1006";
  skos:prefLabel "ulan1006_formerly_identified_with";
  dc:title "formerly identified with - any";
  skos:example "Tommaso is formerly identified with Tommaso di Stefano Lunetti",
    "GreenWorks is formerly identified with Mike Faha & Associates" ;
  dct:description """any - formerly identified with - any.
Example: Tommaso is formerly identified with Tommaso di Stefano Lunetti; GreenWorks is formerly identified with Mike Faha & Associates""" .
gvp:ulan1006_formerly_identified_with a owl:SymmetricProperty.


gvp:ulan1007_distinguished_from a owl:ObjectProperty;
  rdfs:isDefinedBy <http://vocab.getty.edu/ontology>, ulan: ;
  rdfs:subPropertyOf skos:related;
  rdfs:domain skos:Concept; rdfs:range skos:Concept;
  # domain "any"; range "any";
  dc:identifier "1007";
  skos:prefLabel "ulan1007_distinguished_from";
  dc:title "distinguished from - any";
  skos:example "Laura Theresa Alma-Tadema is distinguished from Lawrence Alma-Tadema",
    "The Noguchi Museum is distinguished form Isamu Noguchi Garden Museum Japan" ;
  dct:description """any - distinguished from - any.
Example: Laura Theresa Alma-Tadema is distinguished from Lawrence Alma-Tadema; The Noguchi Museum is distinguished form Isamu Noguchi Garden Museum Japan""" .
gvp:ulan1007_distinguished_from a owl:SymmetricProperty.


gvp:ulan1008_meaning_-usage_overlaps_with a owl:ObjectProperty;
  rdfs:isDefinedBy <http://vocab.getty.edu/ontology>, ulan: ;
  rdfs:subPropertyOf skos:related;
  rdfs:domain skos:Concept; rdfs:range skos:Concept;
  # domain "any"; range "any";
  dc:identifier "1008";
  skos:prefLabel "ulan1008_meaning_-usage_overlaps_with";
  dc:title "meaning /usage overlaps with - any";
  skos:example "The meaning or usage of unknown Zimbabwean overlaps with unknown Rodesian" ;
  dct:description """any - meaning /usage overlaps with - any.
Example: The meaning or usage of unknown Zimbabwean overlaps with unknown Rodesian""" .
gvp:ulan1008_meaning_-usage_overlaps_with a owl:SymmetricProperty.


gvp:ulan1101_teacher_of a owl:ObjectProperty;
  rdfs:isDefinedBy <http://vocab.getty.edu/ontology>, ulan: ;
  rdfs:subPropertyOf skos:related;
  rdfs:domain skos:Concept; rdfs:range skos:Concept;
  # domain "person"; range "person";
  dc:identifier "1101";
  skos:prefLabel "ulan1101_teacher_of";
  dc:title "teacher of - person";
  skos:example "Rivalz, Antoine was the teacher of Pierre Subleyras" ;
  dct:description """person - teacher of - person.
Example: Rivalz, Antoine was the teacher of Pierre Subleyras""" .


gvp:ulan1102_student_of a owl:ObjectProperty;
  rdfs:isDefinedBy <http://vocab.getty.edu/ontology>, ulan: ;
  rdfs:subPropertyOf skos:related;
  rdfs:domain skos:Concept; rdfs:range skos:Concept;
  # domain "person"; range "person";
  dc:identifier "1102";
  skos:prefLabel "ulan1102_student_of";
  dc:title "student of - person";
  skos:example "Pierre Subleyras was the student of Rivalz, Antoine" ;
  dct:description """person - student of - person.
Example: Pierre Subleyras was the student of Rivalz, Antoine""" .
gvp:ulan1101_teacher_of owl:inverseOf gvp:ulan1102_student_of.


gvp:ulan1105_apprentice_of a owl:ObjectProperty;
  rdfs:isDefinedBy <http://vocab.getty.edu/ontology>, ulan: ;
  rdfs:subPropertyOf skos:related;
  rdfs:domain skos:Concept; rdfs:range skos:Concept;
  # domain "person"; range "person";
  dc:identifier "1105";
  skos:prefLabel "ulan1105_apprentice_of";
  dc:title "apprentice of - person";
  skos:example "Nicolas Hawksmoor was the apprentice of Christopher Wren" ;
  dct:description """person - apprentice of - person.
Example: Nicolas Hawksmoor was the apprentice of Christopher Wren""" .


gvp:ulan1106_apprentice_was a owl:ObjectProperty;
  rdfs:isDefinedBy <http://vocab.getty.edu/ontology>, ulan: ;
  rdfs:subPropertyOf skos:related;
  rdfs:domain skos:Concept; rdfs:range skos:Concept;
  # domain "person"; range "person";
  dc:identifier "1106";
  skos:prefLabel "ulan1106_apprentice_was";
  dc:title "apprentice was - person";
  skos:example "Nicolas Hawksmoor was the apprentice of Christopher Wren" ;
  dct:description """person - apprentice was - person.
Example: Nicolas Hawksmoor was the apprentice of Christopher Wren""" .
gvp:ulan1105_apprentice_of owl:inverseOf gvp:ulan1106_apprentice_was.


gvp:ulan1107_influenced a owl:ObjectProperty;
  rdfs:isDefinedBy <http://vocab.getty.edu/ontology>, ulan: ;
  rdfs:subPropertyOf skos:related;
  rdfs:domain skos:Concept; rdfs:range skos:Concept;
  # domain "person"; range "person";
  dc:identifier "1107";
  skos:prefLabel "ulan1107_influenced";
  dc:title "influenced - person";
  skos:example "Rembrandt van Rijn influenced Salomon Koninck" ;
  dct:description """person - influenced - person.
Example: Rembrandt van Rijn influenced Salomon Koninck""" .


gvp:ulan1108_influenced_by a owl:ObjectProperty;
  rdfs:isDefinedBy <http://vocab.getty.edu/ontology>, ulan: ;
  rdfs:subPropertyOf skos:related;
  rdfs:domain skos:Concept; rdfs:range skos:Concept;
  # domain "person"; range "person";
  dc:identifier "1108";
  skos:prefLabel "ulan1108_influenced_by";
  dc:title "influenced by - person";
  skos:example "Salomon Koninck was influenced by Rembrandt van Rijn" ;
  dct:description """person - influenced by - person.
Example: Salomon Koninck was influenced by Rembrandt van Rijn""" .
gvp:ulan1107_influenced owl:inverseOf gvp:ulan1108_influenced_by.


gvp:ulan1111_master_of a owl:ObjectProperty;
  rdfs:isDefinedBy <http://vocab.getty.edu/ontology>, ulan: ;
  rdfs:subPropertyOf skos:related;
  rdfs:domain skos:Concept; rdfs:range skos:Concept;
  # domain "person"; range "person";
  dc:identifier "1111";
  skos:prefLabel "ulan1111_master_of";
  dc:title "master of - person";
  skos:example "Peter Paul Rubens - master of Jan Thomas" ;
  dct:description """person - master of - person.
Example: Peter Paul Rubens - master of Jan Thomas""" .


gvp:ulan1112_master_was a owl:ObjectProperty;
  rdfs:isDefinedBy <http://vocab.getty.edu/ontology>, ulan: ;
  rdfs:subPropertyOf skos:related;
  rdfs:domain skos:Concept; rdfs:range skos:Concept;
  # domain "person"; range "person";
  dc:identifier "1112";
  skos:prefLabel "ulan1112_master_was";
  dc:title "master was - person";
  skos:example "Peter Paul Rubens - master of Jan Thomas" ;
  dct:description """person - master was - person.
Example: Peter Paul Rubens - master of Jan Thomas""" .
gvp:ulan1111_master_of owl:inverseOf gvp:ulan1112_master_was.


gvp:ulan1113_fellow_student_of a owl:ObjectProperty;
  rdfs:isDefinedBy <http://vocab.getty.edu/ontology>, ulan: ;
  rdfs:subPropertyOf skos:related;
  rdfs:domain skos:Concept; rdfs:range skos:Concept;
  # domain "person"; range "person";
  dc:identifier "1113";
  skos:prefLabel "ulan1113_fellow_student_of";
  dc:title "fellow student of - person";
  skos:example "Alexander Calder was a fellow student of John Sloan",
    "John Sloan was a fellow student of Thomas Hart Benton" ;
  dct:description """person - fellow student of - person.
Example: Alexander Calder was a fellow student of John Sloan; John Sloan was a fellow student of Thomas Hart Benton""" .
gvp:ulan1113_fellow_student_of a owl:SymmetricProperty.


gvp:ulan1201_patron_of a owl:ObjectProperty;
  rdfs:isDefinedBy <http://vocab.getty.edu/ontology>, ulan: ;
  rdfs:subPropertyOf skos:related;
  rdfs:domain skos:Concept; rdfs:range skos:Concept;
  # domain "person"; range "person/firm/family";
  dc:identifier "1201";
  skos:prefLabel "ulan1201_patron_of";
  dc:title "patron of - person/firm/family";
  skos:example "Cosimo I, Grand-Duke of Tuscany was the patron of Donatello" ;
  dct:description """person - patron of - person/firm/family.
Example: Cosimo I, Grand-Duke of Tuscany was the patron of Donatello""" .


gvp:ulan1202_patron_was a owl:ObjectProperty;
  rdfs:isDefinedBy <http://vocab.getty.edu/ontology>, ulan: ;
  rdfs:subPropertyOf skos:related;
  rdfs:domain skos:Concept; rdfs:range skos:Concept;
  # domain "person/firm/family"; range "person";
  dc:identifier "1202";
  skos:prefLabel "ulan1202_patron_was";
  dc:title "patron was - person";
  skos:example "The patron of Donatello was Cosimo I, Grand-Duke of Tuscany" ;
  dct:description """person/firm/family - patron was - person.
Example: The patron of Donatello was Cosimo I, Grand-Duke of Tuscany""" .
gvp:ulan1201_patron_of owl:inverseOf gvp:ulan1202_patron_was.


gvp:ulan1203_donor_of a owl:ObjectProperty;
  rdfs:isDefinedBy <http://vocab.getty.edu/ontology>, ulan: ;
  rdfs:subPropertyOf skos:related;
  rdfs:domain skos:Concept; rdfs:range skos:Concept;
  # domain "person/firm/family"; range "person/firm/family";
  dc:identifier "1203";
  skos:prefLabel "ulan1203_donor_of";
  dc:title "donor of - person/firm/family";
  skos:example "Andrew W. Mellon was a donor of National Gallery of Art" ;
  dct:description """person/firm/family - donor of - person/firm/family.
Example: Andrew W. Mellon was a donor of National Gallery of Art""" .


gvp:ulan1204_donor_was a owl:ObjectProperty;
  rdfs:isDefinedBy <http://vocab.getty.edu/ontology>, ulan: ;
  rdfs:subPropertyOf skos:related;
  rdfs:domain skos:Concept; rdfs:range skos:Concept;
  # domain "person/firm/family"; range "person/firm/family";
  dc:identifier "1204";
  skos:prefLabel "ulan1204_donor_was";
  dc:title "donor was - person/firm/family";
  skos:example "Donor to the National Gallery of Art was Andrew W. Mellon" ;
  dct:description """person/firm/family - donor was - person/firm/family.
Example: Donor to the National Gallery of Art was Andrew W. Mellon""" .
gvp:ulan1203_donor_of owl:inverseOf gvp:ulan1204_donor_was.


gvp:ulan1205_client_of a owl:ObjectProperty;
  rdfs:isDefinedBy <http://vocab.getty.edu/ontology>, ulan: ;
  rdfs:subPropertyOf skos:related;
  rdfs:domain skos:Concept; rdfs:range skos:Concept;
  # domain "person/firm/family"; range "person/firm/family";
  dc:identifier "1205";
  skos:prefLabel "ulan1205_client_of";
  dc:title "client of - person/firm/family";
  skos:example "The Chicago Herald was the client of Burnham and Root" ;
  dct:description """person/firm/family - client of - person/firm/family.
Example: The Chicago Herald was the client of Burnham and Root""" .


gvp:ulan1206_client_was a owl:ObjectProperty;
  rdfs:isDefinedBy <http://vocab.getty.edu/ontology>, ulan: ;
  rdfs:subPropertyOf skos:related;
  rdfs:domain skos:Concept; rdfs:range skos:Concept;
  # domain "person/firm/family"; range "person/firm/family";
  dc:identifier "1206";
  skos:prefLabel "ulan1206_client_was";
  dc:title "client was - person/firm/family";
  skos:example "Burnham and Root's client was the Chicago Herald" ;
  dct:description """person/firm/family - client was - person/firm/family.
Example: Burnham and Root's client was the Chicago Herald""" .
gvp:ulan1205_client_of owl:inverseOf gvp:ulan1206_client_was.


gvp:ulan1211_artist_to a owl:ObjectProperty;
  rdfs:isDefinedBy <http://vocab.getty.edu/ontology>, ulan: ;
  rdfs:subPropertyOf skos:related;
  rdfs:domain skos:Concept; rdfs:range skos:Concept;
  # domain "person"; range "person";
  dc:identifier "1211";
  skos:prefLabel "ulan1211_artist_to";
  dc:title "artist to - person";
  skos:example "Artist to Louis XIV, King of France was Charles-Pierre Coustou" ;
  dct:description """person - artist to - person.
Example: Artist to Louis XIV, King of France was Charles-Pierre Coustou""" .


gvp:ulan1212_artist_was a owl:ObjectProperty;
  rdfs:isDefinedBy <http://vocab.getty.edu/ontology>, ulan: ;
  rdfs:subPropertyOf skos:related;
  rdfs:domain skos:Concept; rdfs:range skos:Concept;
  # domain "person"; range "person";
  dc:identifier "1212";
  skos:prefLabel "ulan1212_artist_was";
  dc:title "artist was - person";
  skos:example "Charles-Pierre Coustou was artist to Louis XIV, King of France" ;
  dct:description """person - artist was - person.
Example: Charles-Pierre Coustou was artist to Louis XIV, King of France""" .
gvp:ulan1211_artist_to owl:inverseOf gvp:ulan1212_artist_was.


gvp:ulan1213_court_artist_to a owl:ObjectProperty;
  rdfs:isDefinedBy <http://vocab.getty.edu/ontology>, ulan: ;
  rdfs:subPropertyOf skos:related;
  rdfs:domain skos:Concept; rdfs:range skos:Concept;
  # domain "person"; range "person";
  dc:identifier "1213";
  skos:prefLabel "ulan1213_court_artist_to";
  dc:title "court artist to - person";
  skos:example "Court artist to Gonzaga Vincenzo I, Duke of Mantua was Peter Paul Rubens",
    "court artist to Charles IV, King of Spain was Francisco de Goya" ;
  dct:description """person - court artist to - person.
Example: Court artist to Gonzaga Vincenzo I, Duke of Mantua was Peter Paul Rubens; court artist to Charles IV, King of Spain was Francisco de Goya""" .


gvp:ulan1214_court_artist_was a owl:ObjectProperty;
  rdfs:isDefinedBy <http://vocab.getty.edu/ontology>, ulan: ;
  rdfs:subPropertyOf skos:related;
  rdfs:domain skos:Concept; rdfs:range skos:Concept;
  # domain "person"; range "person";
  dc:identifier "1214";
  skos:prefLabel "ulan1214_court_artist_was";
  dc:title "court artist was - person";
  skos:example "Peter Paul Rubens was court artist to Gonzaga Vincenzo I, Duke of Mantua",
    "Francisco de Goya was court artist to Charles IV, King of Spain" ;
  dct:description """person - court artist was - person.
Example: Peter Paul Rubens was court artist to Gonzaga Vincenzo I, Duke of Mantua; Francisco de Goya was court artist to Charles IV, King of Spain""" .
gvp:ulan1213_court_artist_to owl:inverseOf gvp:ulan1214_court_artist_was.


gvp:ulan1217_employee_of a owl:ObjectProperty;
  rdfs:isDefinedBy <http://vocab.getty.edu/ontology>, ulan: ;
  rdfs:subPropertyOf skos:related;
  rdfs:domain skos:Concept; rdfs:range skos:Concept;
  # domain "person/firm"; range "person";
  dc:identifier "1217";
  skos:prefLabel "ulan1217_employee_of";
  dc:title "employee of - person";
  skos:example "Employee of Christopher Wren was Jean Tijou" ;
  dct:description """person/firm - employee of - person.
Example: Employee of Christopher Wren was Jean Tijou""" .


gvp:ulan1218_employee_was a owl:ObjectProperty;
  rdfs:isDefinedBy <http://vocab.getty.edu/ontology>, ulan: ;
  rdfs:subPropertyOf skos:related;
  rdfs:domain skos:Concept; rdfs:range skos:Concept;
  # domain "person"; range "person/firm";
  dc:identifier "1218";
  skos:prefLabel "ulan1218_employee_was";
  dc:title "employee was - person/firm";
  skos:example "Jean Tijou was an employee of Christopher Wren" ;
  dct:description """person - employee was - person/firm.
Example: Jean Tijou was an employee of Christopher Wren""" .
gvp:ulan1217_employee_of owl:inverseOf gvp:ulan1218_employee_was.


gvp:ulan1221_appointed_by a owl:ObjectProperty;
  rdfs:isDefinedBy <http://vocab.getty.edu/ontology>, ulan: ;
  rdfs:subPropertyOf skos:related;
  rdfs:domain skos:Concept; rdfs:range skos:Concept;
  # domain "person"; range "person";
  dc:identifier "1221";
  skos:prefLabel "ulan1221_appointed_by";
  dc:title "appointed by - person";
  skos:example "Pope Urban VIII appointed Virginio Cesarini" ;
  dct:description """person - appointed by - person.
Example: Pope Urban VIII appointed Virginio Cesarini""" .


gvp:ulan1222_appointee_of a owl:ObjectProperty;
  rdfs:isDefinedBy <http://vocab.getty.edu/ontology>, ulan: ;
  rdfs:subPropertyOf skos:related;
  rdfs:domain skos:Concept; rdfs:range skos:Concept;
  # domain "person"; range "person";
  dc:identifier "1222";
  skos:prefLabel "ulan1222_appointee_of";
  dc:title "appointee of - person";
  skos:example "Virginio Cesarini was appointee by Pope Urban VIII" ;
  dct:description """person - appointee of - person.
Example: Virginio Cesarini was appointee by Pope Urban VIII""" .
gvp:ulan1221_appointed_by owl:inverseOf gvp:ulan1222_appointee_of.


gvp:ulan1223_crowned_by a owl:ObjectProperty;
  rdfs:isDefinedBy <http://vocab.getty.edu/ontology>, ulan: ;
  rdfs:subPropertyOf skos:related;
  rdfs:domain skos:Concept; rdfs:range skos:Concept;
  # domain "person"; range "person";
  dc:identifier "1223";
  skos:prefLabel "ulan1223_crowned_by";
  dc:title "crowned by - person";
  skos:example "Pope Leo III crowned Emperor Charlemagne" ;
  dct:description """person - crowned by - person.
Example: Pope Leo III crowned Emperor Charlemagne""" .


gvp:ulan1224_crowned a owl:ObjectProperty;
  rdfs:isDefinedBy <http://vocab.getty.edu/ontology>, ulan: ;
  rdfs:subPropertyOf skos:related;
  rdfs:domain skos:Concept; rdfs:range skos:Concept;
  # domain "person"; range "person";
  dc:identifier "1224";
  skos:prefLabel "ulan1224_crowned";
  dc:title "crowned - person";
  skos:example "Emperor Charlemagne was crowned by Pope Leo III" ;
  dct:description """person - crowned - person.
Example: Emperor Charlemagne was crowned by Pope Leo III""" .
gvp:ulan1223_crowned_by owl:inverseOf gvp:ulan1224_crowned.


gvp:ulan1301_colleague_of a owl:ObjectProperty;
  rdfs:isDefinedBy <http://vocab.getty.edu/ontology>, ulan: ;
  rdfs:subPropertyOf skos:related;
  rdfs:domain skos:Concept; rdfs:range skos:Concept;
  # domain "person"; range "person";
  dc:identifier "1301";
  skos:prefLabel "ulan1301_colleague_of";
  dc:title "colleague of - person";
  skos:example "Titian was a colleague of Maria Giovanni Verdizotti" ;
  dct:description """person - colleague of - person.
Example: Titian was a colleague of Maria Giovanni Verdizotti""" .
gvp:ulan1301_colleague_of a owl:SymmetricProperty.


gvp:ulan1302_associate_of a owl:ObjectProperty;
  rdfs:isDefinedBy <http://vocab.getty.edu/ontology>, ulan: ;
  rdfs:subPropertyOf skos:related;
  rdfs:domain skos:Concept; rdfs:range skos:Concept;
  # domain "person"; range "person";
  dc:identifier "1302";
  skos:prefLabel "ulan1302_associate_of";
  dc:title "associate of - person";
  skos:example "Frank Lloyd Wright was an associate of Giannini and Hilgart" ;
  dct:description """person - associate of - person.
Example: Frank Lloyd Wright was an associate of Giannini and Hilgart""" .
gvp:ulan1302_associate_of a owl:SymmetricProperty.


gvp:ulan1303_collaborated_with a owl:ObjectProperty;
  rdfs:isDefinedBy <http://vocab.getty.edu/ontology>, ulan: ;
  rdfs:subPropertyOf skos:related;
  rdfs:domain skos:Concept; rdfs:range skos:Concept;
  # domain "person"; range "person";
  dc:identifier "1303";
  skos:prefLabel "ulan1303_collaborated_with";
  dc:title "collaborated with - person";
  skos:example "Pablo Picasso collaborated with Georges Braque" ;
  dct:description """person - collaborated with - person.
Example: Pablo Picasso collaborated with Georges Braque""" .
gvp:ulan1303_collaborated_with a owl:SymmetricProperty.


gvp:ulan1305_worked_with a owl:ObjectProperty;
  rdfs:isDefinedBy <http://vocab.getty.edu/ontology>, ulan: ;
  rdfs:subPropertyOf skos:related;
  rdfs:domain skos:Concept; rdfs:range skos:Concept;
  # domain "person"; range "person";
  dc:identifier "1305";
  skos:prefLabel "ulan1305_worked_with";
  dc:title "worked with - person";
  skos:example "William Cleare worked with Christopher Wren",
    "Frank Lloyd Wright work with Aaron G. Green" ;
  dct:description """person - worked with - person.
Example: William Cleare worked with Christopher Wren; Frank Lloyd Wright work with Aaron G. Green""" .
gvp:ulan1305_worked_with a owl:SymmetricProperty.


gvp:ulan1306_performs_with a owl:ObjectProperty;
  rdfs:isDefinedBy <http://vocab.getty.edu/ontology>, ulan: ;
  rdfs:subPropertyOf skos:related;
  rdfs:domain skos:Concept; rdfs:range skos:Concept;
  # domain "person"; range "person";
  dc:identifier "1306";
  skos:prefLabel "ulan1306_performs_with";
  dc:title "performs with - person";
  skos:example "Harry Kipper performs with Harry Kipper (as part of 'The Kipper Kids')" ;
  dct:description """person - performs with - person.
Example: Harry Kipper performs with Harry Kipper (as part of 'The Kipper Kids')""" .
gvp:ulan1306_performs_with a owl:SymmetricProperty.


gvp:ulan1307_assistant_of a owl:ObjectProperty;
  rdfs:isDefinedBy <http://vocab.getty.edu/ontology>, ulan: ;
  rdfs:subPropertyOf skos:related;
  rdfs:domain skos:Concept; rdfs:range skos:Concept;
  # domain "person"; range "person";
  dc:identifier "1307";
  skos:prefLabel "ulan1307_assistant_of";
  dc:title "assistant of - person";
  skos:example "Bernard Castelli was assistant of Pablo Picasso" ;
  dct:description """person - assistant of - person.
Example: Bernard Castelli was assistant of Pablo Picasso""" .


gvp:ulan1308_assisted_by a owl:ObjectProperty;
  rdfs:isDefinedBy <http://vocab.getty.edu/ontology>, ulan: ;
  rdfs:subPropertyOf skos:related;
  rdfs:domain skos:Concept; rdfs:range skos:Concept;
  # domain "person"; range "person";
  dc:identifier "1308";
  skos:prefLabel "ulan1308_assisted_by";
  dc:title "assisted by - person";
  skos:example "Pablo Picasso was assisted by Bernard Castelli" ;
  dct:description """person - assisted by - person.
Example: Pablo Picasso was assisted by Bernard Castelli""" .
gvp:ulan1307_assistant_of owl:inverseOf gvp:ulan1308_assisted_by.


gvp:ulan1309_advisor_of a owl:ObjectProperty;
  rdfs:isDefinedBy <http://vocab.getty.edu/ontology>, ulan: ;
  rdfs:subPropertyOf skos:related;
  rdfs:domain skos:Concept; rdfs:range skos:Concept;
  # domain "person"; range "person";
  dc:identifier "1309";
  skos:prefLabel "ulan1309_advisor_of";
  dc:title "advisor of - person";
  skos:example "Thomas Cromwell, Earl of Essex was the advisor of Henry VIII, King of England" ;
  dct:description """person - advisor of - person.
Example: Thomas Cromwell, Earl of Essex was the advisor of Henry VIII, King of England""" .


gvp:ulan1310_advised_by a owl:ObjectProperty;
  rdfs:isDefinedBy <http://vocab.getty.edu/ontology>, ulan: ;
  rdfs:subPropertyOf skos:related;
  rdfs:domain skos:Concept; rdfs:range skos:Concept;
  # domain "person"; range "person";
  dc:identifier "1310";
  skos:prefLabel "ulan1310_advised_by";
  dc:title "advised by - person";
  skos:example "Henry VIII, King of England was advised by Thomas Cromwell, Earl of Essex" ;
  dct:description """person - advised by - person.
Example: Henry VIII, King of England was advised by Thomas Cromwell, Earl of Essex""" .
gvp:ulan1309_advisor_of owl:inverseOf gvp:ulan1310_advised_by.


gvp:ulan1311_partner_of a owl:ObjectProperty;
  rdfs:isDefinedBy <http://vocab.getty.edu/ontology>, ulan: ;
  rdfs:subPropertyOf skos:related;
  rdfs:domain skos:Concept; rdfs:range skos:Concept;
  # domain "person"; range "person";
  dc:identifier "1311";
  skos:prefLabel "ulan1311_partner_of";
  dc:title "partner of - person";
  skos:example "Frank Gehry and James Glymph are partners" ;
  dct:description """person - partner of - person.
Example: Frank Gehry and James Glymph are partners""" .
gvp:ulan1311_partner_of a owl:SymmetricProperty.


gvp:ulan1313_partner_in a owl:ObjectProperty;
  rdfs:isDefinedBy <http://vocab.getty.edu/ontology>, ulan: ;
  rdfs:subPropertyOf skos:related;
  rdfs:domain skos:Concept; rdfs:range skos:Concept;
  # domain "person"; range "firm";
  dc:identifier "1313";
  skos:prefLabel "ulan1313_partner_in";
  dc:title "partner in - firm";
  skos:example "Parners of Adler and Sullivan included Louis H. Sullivan and Dankmar Adler" ;
  dct:description """person - partner in - firm.
Example: Parners of Adler and Sullivan included Louis H. Sullivan and Dankmar Adler""" .


gvp:ulan1314_partner_was a owl:ObjectProperty;
  rdfs:isDefinedBy <http://vocab.getty.edu/ontology>, ulan: ;
  rdfs:subPropertyOf skos:related;
  rdfs:domain skos:Concept; rdfs:range skos:Concept;
  # domain "firm"; range "person";
  dc:identifier "1314";
  skos:prefLabel "ulan1314_partner_was";
  dc:title "partner was - person";
  skos:example "Louis H. Sullivan and Dankmar Adler were partners in Adler and Sullivan" ;
  dct:description """firm - partner was - person.
Example: Louis H. Sullivan and Dankmar Adler were partners in Adler and Sullivan""" .
gvp:ulan1313_partner_in owl:inverseOf gvp:ulan1314_partner_was.


gvp:ulan1315_principal_in a owl:ObjectProperty;
  rdfs:isDefinedBy <http://vocab.getty.edu/ontology>, ulan: ;
  rdfs:subPropertyOf skos:related;
  rdfs:domain skos:Concept; rdfs:range skos:Concept;
  # domain "person"; range "firm";
  dc:identifier "1315";
  skos:prefLabel "ulan1315_principal_in";
  dc:title "principal in - firm";
  skos:example "Principal in Fontana Workshop was Orazio Fontana" ;
  dct:description """person - principal in - firm.
Example: Principal in Fontana Workshop was Orazio Fontana""" .


gvp:ulan1316_principal_was a owl:ObjectProperty;
  rdfs:isDefinedBy <http://vocab.getty.edu/ontology>, ulan: ;
  rdfs:subPropertyOf skos:related;
  rdfs:domain skos:Concept; rdfs:range skos:Concept;
  # domain "firm"; range "person";
  dc:identifier "1316";
  skos:prefLabel "ulan1316_principal_was";
  dc:title "principal was - person";
  skos:example "Orazio Fontana was principal in Fontana Workshop" ;
  dct:description """firm - principal was - person.
Example: Orazio Fontana was principal in Fontana Workshop""" .
gvp:ulan1315_principal_in owl:inverseOf gvp:ulan1316_principal_was.


gvp:ulan1317_member_of a owl:ObjectProperty;
  rdfs:isDefinedBy <http://vocab.getty.edu/ontology>, ulan: ;
  rdfs:subPropertyOf skos:related;
  rdfs:domain skos:Concept; rdfs:range skos:Concept;
  # domain "firm/group"; range "person/firm/group";
  dc:identifier "1317";
  skos:prefLabel "ulan1317_member_of";
  dc:title "member of - person/firm/group";
  skos:example "A member of the Foundation of Documents of Architecture is the National Gallery of Art" ;
  dct:description """firm/group - member of - person/firm/group.
Example: A member of the Foundation of Documents of Architecture is the National Gallery of Art""" .


gvp:ulan1318_member_was a owl:ObjectProperty;
  rdfs:isDefinedBy <http://vocab.getty.edu/ontology>, ulan: ;
  rdfs:subPropertyOf skos:related;
  rdfs:domain skos:Concept; rdfs:range skos:Concept;
  # domain "person/firm/group"; range "firm/group";
  dc:identifier "1318";
  skos:prefLabel "ulan1318_member_was";
  dc:title "member was - firm/group";
  skos:example "The National Gallery of Art was/is a member of the Foundation of Documentation of Architecture" ;
  dct:description """person/firm/group - member was - firm/group.
Example: The National Gallery of Art was/is a member of the Foundation of Documentation of Architecture""" .
gvp:ulan1317_member_of owl:inverseOf gvp:ulan1318_member_was.


gvp:ulan1321_school_of a owl:ObjectProperty;
  rdfs:isDefinedBy <http://vocab.getty.edu/ontology>, ulan: ;
  rdfs:subPropertyOf skos:related;
  rdfs:domain skos:Concept; rdfs:range skos:Concept;
  # domain "person"; range "firm/group";
  dc:identifier "1321";
  skos:prefLabel "ulan1321_school_of";
  dc:title "school of - firm/group";
  skos:example "The school of Pierre Saalburg was the Architectural Association. School of Architecture" ;
  dct:description """person - school of - firm/group.
Example: The school of Pierre Saalburg was the Architectural Association. School of Architecture""" .


gvp:ulan1322_school_was a owl:ObjectProperty;
  rdfs:isDefinedBy <http://vocab.getty.edu/ontology>, ulan: ;
  rdfs:subPropertyOf skos:related;
  rdfs:domain skos:Concept; rdfs:range skos:Concept;
  # domain "firm/group"; range "person";
  dc:identifier "1322";
  skos:prefLabel "ulan1322_school_was";
  dc:title "school was - person";
  skos:example "Pierre Saalburg attended Architectural Association. School of Architecture" ;
  dct:description """firm/group - school was - person.
Example: Pierre Saalburg attended Architectural Association. School of Architecture""" .
gvp:ulan1321_school_of owl:inverseOf gvp:ulan1322_school_was.


gvp:ulan1331_worked_with a owl:ObjectProperty;
  rdfs:isDefinedBy <http://vocab.getty.edu/ontology>, ulan: ;
  rdfs:subPropertyOf skos:related;
  rdfs:domain skos:Concept; rdfs:range skos:Concept;
  # domain "any"; range "person";
  dc:identifier "1331";
  skos:prefLabel "ulan1331_worked_with";
  dc:title "worked with - person";
  skos:example "Scarsellino and Domenichino worked with the Carracci family" ;
  dct:description """any - worked with - person.
Example: Scarsellino and Domenichino worked with the Carracci family""" .


gvp:ulan1332_worker_was a owl:ObjectProperty;
  rdfs:isDefinedBy <http://vocab.getty.edu/ontology>, ulan: ;
  rdfs:subPropertyOf skos:related;
  rdfs:domain skos:Concept; rdfs:range skos:Concept;
  # domain "person"; range "any";
  dc:identifier "1332";
  skos:prefLabel "ulan1332_worker_was";
  dc:title "worker was - any";
  skos:example "Workers for the Carracci family included Scarsellino and Domenichino" ;
  dct:description """person - worker was - any.
Example: Workers for the Carracci family included Scarsellino and Domenichino""" .
gvp:ulan1331_worked_with owl:inverseOf gvp:ulan1332_worker_was.


gvp:ulan1411_successor_of a owl:ObjectProperty;
  rdfs:isDefinedBy <http://vocab.getty.edu/ontology>, ulan: ;
  rdfs:subPropertyOf skos:related;
  rdfs:domain skos:Concept; rdfs:range skos:Concept;
  # domain "firm/group"; range "firm/group";
  dc:identifier "1411";
  skos:prefLabel "ulan1411_successor_of";
  dc:title "successor of - firm/group";
  skos:example "Richard Meier & Partners Architects LLP is the successor of Richard Meier & Associates" ;
  dct:description """firm/group - successor of - firm/group.
Example: Richard Meier & Partners Architects LLP is the successor of Richard Meier & Associates""" .


gvp:ulan1412_predecessor_of a owl:ObjectProperty;
  rdfs:isDefinedBy <http://vocab.getty.edu/ontology>, ulan: ;
  rdfs:subPropertyOf skos:related;
  rdfs:domain skos:Concept; rdfs:range skos:Concept;
  # domain "firm/group"; range "firm/group";
  dc:identifier "1412";
  skos:prefLabel "ulan1412_predecessor_of";
  dc:title "predecessor of - firm/group";
  skos:example "Richard Meier & Associates is the predecessor of Richard Meier & Partners Architects LLP" ;
  dct:description """firm/group - predecessor of - firm/group.
Example: Richard Meier & Associates is the predecessor of Richard Meier & Partners Architects LLP""" .
gvp:ulan1411_successor_of owl:inverseOf gvp:ulan1412_predecessor_of.


gvp:ulan1413_administration_overlaps_with a owl:ObjectProperty;
  rdfs:isDefinedBy <http://vocab.getty.edu/ontology>, ulan: ;
  rdfs:subPropertyOf skos:related;
  rdfs:domain skos:Concept; rdfs:range skos:Concept;
  # domain "firm/group"; range "firm/group";
  dc:identifier "1413";
  skos:prefLabel "ulan1413_administration_overlaps_with";
  dc:title "administration overlaps with - firm/group";
  skos:example "The administration of the Numismatic Collection overlaps with Bode Museum" ;
  dct:description """firm/group - administration overlaps with - firm/group.
Example: The administration of the Numismatic Collection overlaps with Bode Museum""" .
gvp:ulan1413_administration_overlaps_with a owl:SymmetricProperty.


gvp:ulan1414_joint_venture_with a owl:ObjectProperty;
  rdfs:isDefinedBy <http://vocab.getty.edu/ontology>, ulan: ;
  rdfs:subPropertyOf skos:related;
  rdfs:domain skos:Concept; rdfs:range skos:Concept;
  # domain "firm/group"; range "firm/group";
  dc:identifier "1414";
  skos:prefLabel "ulan1414_joint_venture_with";
  dc:title "joint venture with - firm/group";
  skos:example "Schwetye Luchini Architects is in a joint venture with ACME Architects" ;
  dct:description """firm/group - joint venture with - firm/group.
Example: Schwetye Luchini Architects is in a joint venture with ACME Architects""" .
gvp:ulan1414_joint_venture_with a owl:SymmetricProperty.


gvp:ulan1421_founded_by a owl:ObjectProperty;
  rdfs:isDefinedBy <http://vocab.getty.edu/ontology>, ulan: ;
  rdfs:subPropertyOf skos:related;
  rdfs:domain skos:Concept; rdfs:range skos:Concept;
  # domain "firm/group"; range "firm/group";
  dc:identifier "1421";
  skos:prefLabel "ulan1421_founded_by";
  dc:title "founded by - firm/group";
  skos:example "National Gallery of Art was founded by United States Congress" ;
  dct:description """firm/group - founded by - firm/group.
Example: National Gallery of Art was founded by United States Congress""" .


gvp:ulan1422_founded a owl:ObjectProperty;
  rdfs:isDefinedBy <http://vocab.getty.edu/ontology>, ulan: ;
  rdfs:subPropertyOf skos:related;
  rdfs:domain skos:Concept; rdfs:range skos:Concept;
  # domain "firm/group"; range "firm/group";
  dc:identifier "1422";
  skos:prefLabel "ulan1422_founded";
  dc:title "founded - firm/group";
  skos:example "The United States Congress founded the National Gallery of Art" ;
  dct:description """firm/group - founded - firm/group.
Example: The United States Congress founded the National Gallery of Art""" .
gvp:ulan1421_founded_by owl:inverseOf gvp:ulan1422_founded.


gvp:ulan1500_related_to a owl:ObjectProperty;
  rdfs:isDefinedBy <http://vocab.getty.edu/ontology>, ulan: ;
  rdfs:subPropertyOf skos:related;
  rdfs:domain skos:Concept; rdfs:range skos:Concept;
  # domain "person"; range "person";
  dc:identifier "1500";
  skos:prefLabel "ulan1500_related_to";
  dc:title "related to - person";
  skos:example "Titian and Tizianello have a familial relationship with each other" ;
  dct:description """person - related to (familial relationship) - person.
Example: Titian and Tizianello have a familial relationship with each other""" .
gvp:ulan1500_related_to a owl:SymmetricProperty.


gvp:ulan1501_sibling_of a owl:ObjectProperty;
  rdfs:isDefinedBy <http://vocab.getty.edu/ontology>, ulan: ;
  rdfs:subPropertyOf skos:related;
  rdfs:domain skos:Concept; rdfs:range skos:Concept;
  # domain "person"; range "person";
  dc:identifier "1501";
  skos:prefLabel "ulan1501_sibling_of";
  dc:title "sibling of - person";
  skos:example "Philippe Rubens is the sibling of Peter Paul Rubens" ;
  dct:description """person - sibling of - person.
Example: Philippe Rubens is the sibling of Peter Paul Rubens""" .
gvp:ulan1501_sibling_of a owl:SymmetricProperty.


gvp:ulan1511_child_of a owl:ObjectProperty;
  rdfs:isDefinedBy <http://vocab.getty.edu/ontology>, ulan: ;
  rdfs:subPropertyOf skos:related;
  rdfs:domain skos:Concept; rdfs:range skos:Concept;
  # domain "person"; range "person";
  dc:identifier "1511";
  skos:prefLabel "ulan1511_child_of";
  dc:title "child of - person";
  skos:example "Rembrandt van Rijn is the child of Neeltgen Willemsdr van Zuydtbroeck" ;
  dct:description """person - child of - person.
Example: Rembrandt van Rijn is the child of Neeltgen Willemsdr van Zuydtbroeck""" .


gvp:ulan1512_parent_of a owl:ObjectProperty;
  rdfs:isDefinedBy <http://vocab.getty.edu/ontology>, ulan: ;
  rdfs:subPropertyOf skos:related;
  rdfs:domain skos:Concept; rdfs:range skos:Concept;
  # domain "person"; range "person";
  dc:identifier "1512";
  skos:prefLabel "ulan1512_parent_of";
  dc:title "parent of - person";
  skos:example "Rembrandt van Rijn is the parent of Rumbertus van Rijn" ;
  dct:description """person - parent of - person.
Example: Rembrandt van Rijn is the parent of Rumbertus van Rijn""" .
gvp:ulan1511_child_of owl:inverseOf gvp:ulan1512_parent_of.


gvp:ulan1513_grandchild_of a owl:ObjectProperty;
  rdfs:isDefinedBy <http://vocab.getty.edu/ontology>, ulan: ;
  rdfs:subPropertyOf skos:related;
  rdfs:domain skos:Concept; rdfs:range skos:Concept;
  # domain "person"; range "person";
  dc:identifier "1513";
  skos:prefLabel "ulan1513_grandchild_of";
  dc:title "grandchild of - person";
  skos:example "Eric Lloyd Wright is the grandchild of Frank Lloyd Wright" ;
  dct:description """person - grandchild of - person.
Example: Eric Lloyd Wright is the grandchild of Frank Lloyd Wright""" .


gvp:ulan1514_gandparent_of a owl:ObjectProperty;
  rdfs:isDefinedBy <http://vocab.getty.edu/ontology>, ulan: ;
  rdfs:subPropertyOf skos:related;
  rdfs:domain skos:Concept; rdfs:range skos:Concept;
  # domain "person"; range "person";
  dc:identifier "1514";
  skos:prefLabel "ulan1514_gandparent_of";
  dc:title "gandparent of - person";
  skos:example "Frank Lloyd Wright is the grandparent of Eric Lloyd Wright" ;
  dct:description """person - gandparent of - person.
Example: Frank Lloyd Wright is the grandparent of Eric Lloyd Wright""" .
gvp:ulan1513_grandchild_of owl:inverseOf gvp:ulan1514_gandparent_of.


gvp:ulan1515_great-grandparent_of a owl:ObjectProperty;
  rdfs:isDefinedBy <http://vocab.getty.edu/ontology>, ulan: ;
  rdfs:subPropertyOf skos:related;
  rdfs:domain skos:Concept; rdfs:range skos:Concept;
  # domain "person"; range "person";
  dc:identifier "1515";
  skos:prefLabel "ulan1515_great-grandparent_of";
  dc:title "great-grandparent of - person";
  skos:example "Albrecht Adam is the great-grandparent of Richard Benno Adam" ;
  dct:description """person - great-grandparent of - person.
Example: Albrecht Adam is the great-grandparent of Richard Benno Adam""" .


gvp:ulan1516_great-grandchild_of a owl:ObjectProperty;
  rdfs:isDefinedBy <http://vocab.getty.edu/ontology>, ulan: ;
  rdfs:subPropertyOf skos:related;
  rdfs:domain skos:Concept; rdfs:range skos:Concept;
  # domain "person"; range "person";
  dc:identifier "1516";
  skos:prefLabel "ulan1516_great-grandchild_of";
  dc:title "great-grandchild of - person";
  skos:example "Richard Benno Adam is the great-grandchild of Albrecht Adam" ;
  dct:description """person - great-grandchild of - person.
Example: Richard Benno Adam is the great-grandchild of Albrecht Adam""" .
gvp:ulan1515_great-grandparent_of owl:inverseOf gvp:ulan1516_great-grandchild_of.


gvp:ulan1521_cousin_of a owl:ObjectProperty;
  rdfs:isDefinedBy <http://vocab.getty.edu/ontology>, ulan: ;
  rdfs:subPropertyOf skos:related;
  rdfs:domain skos:Concept; rdfs:range skos:Concept;
  # domain "person"; range "person";
  dc:identifier "1521";
  skos:prefLabel "ulan1521_cousin_of";
  dc:title "cousin of - person";
  skos:example "Richard Meier and Frank Gehry are cousins" ;
  dct:description """person - cousin of - person.
Example: Richard Meier and Frank Gehry are cousins""" .
gvp:ulan1521_cousin_of a owl:SymmetricProperty.


gvp:ulan1531_nephew-niece_of a owl:ObjectProperty;
  rdfs:isDefinedBy <http://vocab.getty.edu/ontology>, ulan: ;
  rdfs:subPropertyOf skos:related;
  rdfs:domain skos:Concept; rdfs:range skos:Concept;
  # domain "person"; range "person";
  dc:identifier "1531";
  skos:prefLabel "ulan1531_nephew-niece_of";
  dc:title "nephew/niece of - person";
  skos:example "Jan Brueghel, the elder is the nephew/neice of  Pieter Coecke van Aeist, the younger" ;
  dct:description """person - nephew/niece of - person.
Example: Jan Brueghel, the elder is the nephew/neice of  Pieter Coecke van Aeist, the younger""" .


gvp:ulan1532_uncle-aunt_of a owl:ObjectProperty;
  rdfs:isDefinedBy <http://vocab.getty.edu/ontology>, ulan: ;
  rdfs:subPropertyOf skos:related;
  rdfs:domain skos:Concept; rdfs:range skos:Concept;
  # domain "person"; range "person";
  dc:identifier "1532";
  skos:prefLabel "ulan1532_uncle-aunt_of";
  dc:title "uncle/aunt of - person";
  skos:example "Edouard Manet is the uncle/aunt of Julie Manet" ;
  dct:description """person - uncle/aunt of - person.
Example: Edouard Manet is the uncle/aunt of Julie Manet""" .
gvp:ulan1531_nephew-niece_of owl:inverseOf gvp:ulan1532_uncle-aunt_of.


gvp:ulan1541_spouse_of a owl:ObjectProperty;
  rdfs:isDefinedBy <http://vocab.getty.edu/ontology>, ulan: ;
  rdfs:subPropertyOf skos:related;
  rdfs:domain skos:Concept; rdfs:range skos:Concept;
  # domain "person"; range "person";
  dc:identifier "1541";
  skos:prefLabel "ulan1541_spouse_of";
  dc:title "spouse of - person";
  skos:example "Alfred Stieglitz and Georgia O'Keeffe were married to each other" ;
  dct:description """person - spouse of - person.
Example: Alfred Stieglitz and Georgia O'Keeffe were married to each other""" .
gvp:ulan1541_spouse_of a owl:SymmetricProperty.


gvp:ulan1542_consort_of a owl:ObjectProperty;
  rdfs:isDefinedBy <http://vocab.getty.edu/ontology>, ulan: ;
  rdfs:subPropertyOf skos:related;
  rdfs:domain skos:Concept; rdfs:range skos:Concept;
  # domain "person"; range "person";
  dc:identifier "1542";
  skos:prefLabel "ulan1542_consort_of";
  dc:title "consort of - person";
  skos:example "Empress Livia was the consort of Augustus, Emperor of Rome" ;
  dct:description """person - consort of - person.
Example: Empress Livia was the consort of Augustus, Emperor of Rome""" .


gvp:ulan1543_consort_was a owl:ObjectProperty;
  rdfs:isDefinedBy <http://vocab.getty.edu/ontology>, ulan: ;
  rdfs:subPropertyOf skos:related;
  rdfs:domain skos:Concept; rdfs:range skos:Concept;
  # domain "person"; range "person";
  dc:identifier "1543";
  skos:prefLabel "ulan1543_consort_was";
  dc:title "consort was - person";
  skos:example "Augustus, Emperor of Rome's consort was Empress Livia" ;
  dct:description """person - consort was - person.
Example: Augustus, Emperor of Rome's consort was Empress Livia""" .
gvp:ulan1542_consort_of owl:inverseOf gvp:ulan1543_consort_was.


gvp:ulan1544_significant_other_of a owl:ObjectProperty;
  rdfs:isDefinedBy <http://vocab.getty.edu/ontology>, ulan: ;
  rdfs:subPropertyOf skos:related;
  rdfs:domain skos:Concept; rdfs:range skos:Concept;
  # domain "person"; range "person";
  dc:identifier "1544";
  skos:prefLabel "ulan1544_significant_other_of";
  dc:title "significant other of - person";
  skos:example "Jeanne Hebuterne was the significant other of Amedeo Modigliani" ;
  dct:description """person - significant other of - person.
Example: Jeanne Hebuterne was the significant other of Amedeo Modigliani""" .
gvp:ulan1544_significant_other_of a owl:SymmetricProperty.


gvp:ulan1547_romantic_partner_of a owl:ObjectProperty;
  rdfs:isDefinedBy <http://vocab.getty.edu/ontology>, ulan: ;
  rdfs:subPropertyOf skos:related;
  rdfs:domain skos:Concept; rdfs:range skos:Concept;
  # domain "person"; range "person";
  dc:identifier "1547";
  skos:prefLabel "ulan1547_romantic_partner_of";
  dc:title "romantic partner of - person";
  skos:example "Pablo Picasso and Gaby Lespinasse were romantic partners",
    "Vincent van Gogh and Clasina Hoornik were romantic partners" ;
  dct:description """person - romantic partner of - person.
Example: Pablo Picasso and Gaby Lespinasse were romantic partners; Vincent van Gogh and Clasina Hoornik were romantic partners""" .
gvp:ulan1547_romantic_partner_of a owl:SymmetricProperty.


gvp:ulan1548_domestic_partner_of a owl:ObjectProperty;
  rdfs:isDefinedBy <http://vocab.getty.edu/ontology>, ulan: ;
  rdfs:subPropertyOf skos:related;
  rdfs:domain skos:Concept; rdfs:range skos:Concept;
  # domain "person"; range "person";
  dc:identifier "1548";
  skos:prefLabel "ulan1548_domestic_partner_of";
  dc:title "domestic partner of - person" ;
  dct:description """person - domestic partner of - person""" .
gvp:ulan1548_domestic_partner_of a owl:SymmetricProperty.


gvp:ulan1550_relative_by_marriage a owl:ObjectProperty;
  rdfs:isDefinedBy <http://vocab.getty.edu/ontology>, ulan: ;
  rdfs:subPropertyOf skos:related;
  rdfs:domain skos:Concept; rdfs:range skos:Concept;
  # domain "person"; range "person";
  dc:identifier "1550";
  skos:prefLabel "ulan1550_relative_by_marriage";
  dc:title "relative by marriage - person";
  skos:example "Juana Galarza d Goicoechea and Francisco de Goya are related by marriage" ;
  dct:description """person - relative by marriage (in-law) - person.
Example: Juana Galarza d Goicoechea and Francisco de Goya are related by marriage""" .
gvp:ulan1550_relative_by_marriage a owl:SymmetricProperty.


gvp:ulan1551_sibling_by_marriage_of a owl:ObjectProperty;
  rdfs:isDefinedBy <http://vocab.getty.edu/ontology>, ulan: ;
  rdfs:subPropertyOf skos:related;
  rdfs:domain skos:Concept; rdfs:range skos:Concept;
  # domain "person"; range "person";
  dc:identifier "1551";
  skos:prefLabel "ulan1551_sibling_by_marriage_of";
  dc:title "sibling by marriage of - person";
  skos:example "Peter Paul Rubens and Susanne Fourment are siblings by marriage" ;
  dct:description """person - sibling by marriage (step sibling) - person.
Example: Peter Paul Rubens and Susanne Fourment are siblings by marriage""" .
gvp:ulan1551_sibling_by_marriage_of a owl:SymmetricProperty.


gvp:ulan1552_parent_by_marriage_of a owl:ObjectProperty;
  rdfs:isDefinedBy <http://vocab.getty.edu/ontology>, ulan: ;
  rdfs:subPropertyOf skos:related;
  rdfs:domain skos:Concept; rdfs:range skos:Concept;
  # domain "person"; range "person";
  dc:identifier "1552";
  skos:prefLabel "ulan1552_parent_by_marriage_of";
  dc:title "parent by marriage of - person";
  skos:example "Frans Hals is a parent by marriage of Pieter Gerritsz van Roestraten" ;
  dct:description """person - parent by marriage (step parent) - person.
Example: Frans Hals is a parent by marriage of Pieter Gerritsz van Roestraten""" .


gvp:ulan1553_child_by_marriage_of a owl:ObjectProperty;
  rdfs:isDefinedBy <http://vocab.getty.edu/ontology>, ulan: ;
  rdfs:subPropertyOf skos:related;
  rdfs:domain skos:Concept; rdfs:range skos:Concept;
  # domain "person"; range "person";
  dc:identifier "1553";
  skos:prefLabel "ulan1553_child_by_marriage_of";
  dc:title "child by marriage of - person";
  skos:example "Pieter Gerritsz van Roestraten is the child by marriage of Frans Hals" ;
  dct:description """person - child by marriage (step child) - person.
Example: Pieter Gerritsz van Roestraten is the child by marriage of Frans Hals""" .
gvp:ulan1552_parent_by_marriage_of owl:inverseOf gvp:ulan1553_child_by_marriage_of.


gvp:ulan1554_adoptive_parent_of a owl:ObjectProperty;
  rdfs:isDefinedBy <http://vocab.getty.edu/ontology>, ulan: ;
  rdfs:subPropertyOf skos:related;
  rdfs:domain skos:Concept; rdfs:range skos:Concept;
  # domain "person"; range "person";
  dc:identifier "1554";
  skos:prefLabel "ulan1554_adoptive_parent_of";
  dc:title "adoptive parent of - person";
  skos:example "Julius Caesar is the adoptive parent of Augustus, Emperor of Rome" ;
  dct:description """person - adoptive parent of - person.
Example: Julius Caesar is the adoptive parent of Augustus, Emperor of Rome""" .


gvp:ulan1555_adopted_child_of a owl:ObjectProperty;
  rdfs:isDefinedBy <http://vocab.getty.edu/ontology>, ulan: ;
  rdfs:subPropertyOf skos:related;
  rdfs:domain skos:Concept; rdfs:range skos:Concept;
  # domain "person"; range "person";
  dc:identifier "1555";
  skos:prefLabel "ulan1555_adopted_child_of";
  dc:title "adopted child of - person";
  skos:example "Augusts, Emperor of Rome is the adopted child of Julius Caesar" ;
  dct:description """person - adopted child of - person.
Example: Augusts, Emperor of Rome is the adopted child of Julius Caesar""" .
gvp:ulan1554_adoptive_parent_of owl:inverseOf gvp:ulan1555_adopted_child_of.


gvp:ulan1556_half-sibling_of a owl:ObjectProperty;
  rdfs:isDefinedBy <http://vocab.getty.edu/ontology>, ulan: ;
  rdfs:subPropertyOf skos:related;
  rdfs:domain skos:Concept; rdfs:range skos:Concept;
  # domain "person"; range "person";
  dc:identifier "1556";
  skos:prefLabel "ulan1556_half-sibling_of";
  dc:title "half-sibling of - person";
  skos:example "Juan Bautista Monegro and Luis de Carbajal are half siblings" ;
  dct:description """person - half-sibling of - person.
Example: Juan Bautista Monegro and Luis de Carbajal are half siblings""" .
gvp:ulan1556_half-sibling_of a owl:SymmetricProperty.


gvp:ulan1557_step-sibling_of a owl:ObjectProperty;
  rdfs:isDefinedBy <http://vocab.getty.edu/ontology>, ulan: ;
  rdfs:subPropertyOf skos:related;
  rdfs:domain skos:Concept; rdfs:range skos:Concept;
  # domain "person"; range "person";
  dc:identifier "1557";
  skos:prefLabel "ulan1557_step-sibling_of";
  dc:title "step-sibling of - person";
  skos:example "W. L. Wyllie and Lionel Percy Smythe are step-siblings" ;
  dct:description """person - step-sibling of - person.
Example: W. L. Wyllie and Lionel Percy Smythe are step-siblings""" .
gvp:ulan1557_step-sibling_of a owl:SymmetricProperty.


gvp:ulan1561_step-child_of a owl:ObjectProperty;
  rdfs:isDefinedBy <http://vocab.getty.edu/ontology>, ulan: ;
  rdfs:subPropertyOf skos:related;
  rdfs:domain skos:Concept; rdfs:range skos:Concept;
  # domain "person"; range "person";
  dc:identifier "1561";
  skos:prefLabel "ulan1561_step-child_of";
  dc:title "step-child of - person";
  skos:example "Hortense, Quene consort of Louis Bonaparte is the step-child of Napoleon I, Emperor of the French" ;
  dct:description """person - step-child of - person.
Example: Hortense, Quene consort of Louis Bonaparte is the step-child of Napoleon I, Emperor of the French""" .


gvp:ulan1562_step-parent_of a owl:ObjectProperty;
  rdfs:isDefinedBy <http://vocab.getty.edu/ontology>, ulan: ;
  rdfs:subPropertyOf skos:related;
  rdfs:domain skos:Concept; rdfs:range skos:Concept;
  # domain "person"; range "person";
  dc:identifier "1562";
  skos:prefLabel "ulan1562_step-parent_of";
  dc:title "step-parent of - person";
  skos:example "Napoleon I, Emperor of the French is the step-parent of Hortense, Quene consort of Louis Bonaparte" ;
  dct:description """person - step-parent of - person.
Example: Napoleon I, Emperor of the French is the step-parent of Hortense, Quene consort of Louis Bonaparte""" .
gvp:ulan1561_step-child_of owl:inverseOf gvp:ulan1562_step-parent_of.


gvp:ulan1571_guardian_of a owl:ObjectProperty;
  rdfs:isDefinedBy <http://vocab.getty.edu/ontology>, ulan: ;
  rdfs:subPropertyOf skos:related;
  rdfs:domain skos:Concept; rdfs:range skos:Concept;
  # domain "person"; range "person";
  dc:identifier "1571";
  skos:prefLabel "ulan1571_guardian_of";
  dc:title "guardian of - person";
  skos:example "John Hoskins, the elder was the guardian of Samuel Cooper" ;
  dct:description """person - guardian of - person.
Example: John Hoskins, the elder was the guardian of Samuel Cooper""" .


gvp:ulan1573_ward_of a owl:ObjectProperty;
  rdfs:isDefinedBy <http://vocab.getty.edu/ontology>, ulan: ;
  rdfs:subPropertyOf skos:related;
  rdfs:domain skos:Concept; rdfs:range skos:Concept;
  # domain "person"; range "person";
  dc:identifier "1573";
  skos:prefLabel "ulan1573_ward_of";
  dc:title "ward of - person";
  skos:example "Samuel Cooper was a ward of John Hoskins, the elder" ;
  dct:description """person - ward of - person.
Example: Samuel Cooper was a ward of John Hoskins, the elder""" .
gvp:ulan1571_guardian_of owl:inverseOf gvp:ulan1573_ward_of.


gvp:ulan1574_godparent_of a owl:ObjectProperty;
  rdfs:isDefinedBy <http://vocab.getty.edu/ontology>, ulan: ;
  rdfs:subPropertyOf skos:related;
  rdfs:domain skos:Concept; rdfs:range skos:Concept;
  # domain "person"; range "person";
  dc:identifier "1574";
  skos:prefLabel "ulan1574_godparent_of";
  dc:title "godparent of - person";
  skos:example "Jean-Baptiste Goy is godparent of Jean I Nocret" ;
  dct:description """person - godparent of - person.
Example: Jean-Baptiste Goy is godparent of Jean I Nocret""" .


gvp:ulan1575_godchild_of a owl:ObjectProperty;
  rdfs:isDefinedBy <http://vocab.getty.edu/ontology>, ulan: ;
  rdfs:subPropertyOf skos:related;
  rdfs:domain skos:Concept; rdfs:range skos:Concept;
  # domain "person"; range "person";
  dc:identifier "1575";
  skos:prefLabel "ulan1575_godchild_of";
  dc:title "godchild of - person";
  skos:example "Jean I Nocret is the godchild of Jean-Baptiste Goy" ;
  dct:description """person - godchild of - person.
Example: Jean I Nocret is the godchild of Jean-Baptiste Goy""" .
gvp:ulan1574_godparent_of owl:inverseOf gvp:ulan1575_godchild_of.


gvp:ulan1581_descendant_of a owl:ObjectProperty;
  rdfs:isDefinedBy <http://vocab.getty.edu/ontology>, ulan: ;
  rdfs:subPropertyOf skos:related;
  rdfs:domain skos:Concept; rdfs:range skos:Concept;
  # domain "person"; range "person";
  dc:identifier "1581";
  skos:prefLabel "ulan1581_descendant_of";
  dc:title "descendant of - person";
  skos:example "Paolo Caliari is the descendant of Paolo Veronese" ;
  dct:description """person - descendant of - person.
Example: Paolo Caliari is the descendant of Paolo Veronese""" .


gvp:ulan1582_ancestor_of a owl:ObjectProperty;
  rdfs:isDefinedBy <http://vocab.getty.edu/ontology>, ulan: ;
  rdfs:subPropertyOf skos:related;
  rdfs:domain skos:Concept; rdfs:range skos:Concept;
  # domain "person"; range "person";
  dc:identifier "1582";
  skos:prefLabel "ulan1582_ancestor_of";
  dc:title "ancestor of - person";
  skos:example "Paolo Veronese is the ancestor of Paolo Caliari" ;
  dct:description """person - ancestor of - person.
Example: Paolo Veronese is the ancestor of Paolo Caliari""" .
gvp:ulan1581_descendant_of owl:inverseOf gvp:ulan1582_ancestor_of.


gvp:ulan1590_possibly_related_to a owl:ObjectProperty;
  rdfs:isDefinedBy <http://vocab.getty.edu/ontology>, ulan: ;
  rdfs:subPropertyOf skos:related;
  rdfs:domain skos:Concept; rdfs:range skos:Concept;
  # domain "person"; range "person";
  dc:identifier "1590";
  skos:prefLabel "ulan1590_possibly_related_to";
  dc:title "possibly related to - person";
  skos:example "A familial relationship between Ramon Destorrents, the younger and Ramon Destorrents, the elder is possible" ;
  dct:description """person - possibly related to (familial relationship) - person.
Example: A familial relationship between Ramon Destorrents, the younger and Ramon Destorrents, the elder is possible""" .
gvp:ulan1590_possibly_related_to a owl:SymmetricProperty.


gvp:ulan2550_friend_of a owl:ObjectProperty;
  rdfs:isDefinedBy <http://vocab.getty.edu/ontology>, ulan: ;
  rdfs:subPropertyOf skos:related;
  rdfs:domain skos:Concept; rdfs:range skos:Concept;
  # domain "person"; range "person";
  dc:identifier "2550";
  skos:prefLabel "ulan2550_friend_of";
  dc:title "friend of - person";
  skos:example "Alfred Stieglitz and Frank Simon Herrmann were friends" ;
  dct:description """person - friend of (personal relationship) - person.
Example: Alfred Stieglitz and Frank Simon Herrmann were friends""" .
gvp:ulan2550_friend_of a owl:SymmetricProperty.


gvp:ulan2572_founder_of a owl:ObjectProperty;
  rdfs:isDefinedBy <http://vocab.getty.edu/ontology>, ulan: ;
  rdfs:subPropertyOf skos:related;
  rdfs:domain skos:Concept; rdfs:range skos:Concept;
  # domain "person"; range "institution";
  dc:identifier "2572";
  skos:prefLabel "ulan2572_founder_of";
  dc:title "founder of - institution";
  skos:example "Louis Comfort Tiffany was the founder of Tiffany Glass & Decorating Company" ;
  dct:description """person - founder of - institution.
Example: Louis Comfort Tiffany was the founder of Tiffany Glass & Decorating Company""" .


gvp:ulan2573_founded_by a owl:ObjectProperty;
  rdfs:isDefinedBy <http://vocab.getty.edu/ontology>, ulan: ;
  rdfs:subPropertyOf skos:related;
  rdfs:domain skos:Concept; rdfs:range skos:Concept;
  # domain "institution"; range "person";
  dc:identifier "2573";
  skos:prefLabel "ulan2573_founded_by";
  dc:title "founded by - person";
  skos:example "Tiffany Glass & Decorating Company was founded by Louis Comfort Tiffany" ;
  dct:description """institution - founded by - person.
Example: Tiffany Glass & Decorating Company was founded by Louis Comfort Tiffany""" .
gvp:ulan2572_founder_of owl:inverseOf gvp:ulan2573_founded_by.


gvp:ulan2574_director_of a owl:ObjectProperty;
  rdfs:isDefinedBy <http://vocab.getty.edu/ontology>, ulan: ;
  rdfs:subPropertyOf skos:related;
  rdfs:domain skos:Concept; rdfs:range skos:Concept;
  # domain "person"; range "institution";
  dc:identifier "2574";
  skos:prefLabel "ulan2574_director_of";
  dc:title "director of - institution";
  skos:example "Jean Jans I directed Gobelins Tapestry Manufactory" ;
  dct:description """person - director of - institution.
Example: Jean Jans I directed Gobelins Tapestry Manufactory""" .


gvp:ulan2575_directed_by a owl:ObjectProperty;
  rdfs:isDefinedBy <http://vocab.getty.edu/ontology>, ulan: ;
  rdfs:subPropertyOf skos:related;
  rdfs:domain skos:Concept; rdfs:range skos:Concept;
  # domain "institution"; range "person";
  dc:identifier "2575";
  skos:prefLabel "ulan2575_directed_by";
  dc:title "directed by - person";
  skos:example "Gobelins Tapestry Manufactory was directed by Jean Jans I" ;
  dct:description """institution - directed by - person.
Example: Gobelins Tapestry Manufactory was directed by Jean Jans I""" .
gvp:ulan2574_director_of owl:inverseOf gvp:ulan2575_directed_by.


gvp:ulan2576_patron_of a owl:ObjectProperty;
  rdfs:isDefinedBy <http://vocab.getty.edu/ontology>, ulan: ;
  rdfs:subPropertyOf skos:related;
  rdfs:domain skos:Concept; rdfs:range skos:Concept;
  # domain "person"; range "person";
  dc:identifier "2576";
  skos:prefLabel "ulan2576_patron_of";
  dc:title "patron of - person";
  skos:example "The patron of William Chambers was James Caulfiel, Earl of Charlemont" ;
  dct:description """person - patron of - person.
Example: The patron of William Chambers was James Caulfiel, Earl of Charlemont""" .


gvp:ulan2577_patron_was a owl:ObjectProperty;
  rdfs:isDefinedBy <http://vocab.getty.edu/ontology>, ulan: ;
  rdfs:subPropertyOf skos:related;
  rdfs:domain skos:Concept; rdfs:range skos:Concept;
  # domain "person"; range "person";
  dc:identifier "2577";
  skos:prefLabel "ulan2577_patron_was";
  dc:title "patron was - person";
  skos:example "James Caulfiel, Earl of Charlemont was the patron of William Chambers" ;
  dct:description """person - patron was - person.
Example: James Caulfiel, Earl of Charlemont was the patron of William Chambers""" .
gvp:ulan2576_patron_of owl:inverseOf gvp:ulan2577_patron_was.


gvp:ulan2578_trustee_of a owl:ObjectProperty;
  rdfs:isDefinedBy <http://vocab.getty.edu/ontology>, ulan: ;
  rdfs:subPropertyOf skos:related;
  rdfs:domain skos:Concept; rdfs:range skos:Concept;
  # domain "person"; range "institution";
  dc:identifier "2578";
  skos:prefLabel "ulan2578_trustee_of";
  dc:title "trustee of - institution";
  skos:example "George Douglas Haig was a trustee of the National Galleries of Scotland" ;
  dct:description """person - trustee of - institution.
Example: George Douglas Haig was a trustee of the National Galleries of Scotland""" .


gvp:ulan2579_trustee_was a owl:ObjectProperty;
  rdfs:isDefinedBy <http://vocab.getty.edu/ontology>, ulan: ;
  rdfs:subPropertyOf skos:related;
  rdfs:domain skos:Concept; rdfs:range skos:Concept;
  # domain "institution"; range "person";
  dc:identifier "2579";
  skos:prefLabel "ulan2579_trustee_was";
  dc:title "trustee was - person";
  skos:example "National Galleries of Scotland trustee was George Douglas Haig" ;
  dct:description """institution - trustee was - person.
Example: National Galleries of Scotland trustee was George Douglas Haig""" .
gvp:ulan2578_trustee_of owl:inverseOf gvp:ulan2579_trustee_was.


gvp:ulan2581_administrator_of a owl:ObjectProperty;
  rdfs:isDefinedBy <http://vocab.getty.edu/ontology>, ulan: ;
  rdfs:subPropertyOf skos:related;
  rdfs:domain skos:Concept; rdfs:range skos:Concept;
  # domain "person"; range "institution";
  dc:identifier "2581";
  skos:prefLabel "ulan2581_administrator_of";
  dc:title "administrator of - institution";
  skos:example "Georges Mathieu was the administrator of Societe nationale des chemins de fer Francais. Agence des gares" ;
  dct:description """person - administrator of - institution.
Example: Georges Mathieu was the administrator of Societe nationale des chemins de fer Francais. Agence des gares""" .


gvp:ulan2582_administered_by a owl:ObjectProperty;
  rdfs:isDefinedBy <http://vocab.getty.edu/ontology>, ulan: ;
  rdfs:subPropertyOf skos:related;
  rdfs:domain skos:Concept; rdfs:range skos:Concept;
  # domain "institution"; range "person";
  dc:identifier "2582";
  skos:prefLabel "ulan2582_administered_by";
  dc:title "administered by - person";
  skos:example "Societe nationale des chemins de fer Francais. Agence des gares was administered by Georges Mathieu" ;
  dct:description """institution - administered by - person.
Example: Societe nationale des chemins de fer Francais. Agence des gares was administered by Georges Mathieu""" .
gvp:ulan2581_administrator_of owl:inverseOf gvp:ulan2582_administered_by.


gvp:ulan2583_chairman_of a owl:ObjectProperty;
  rdfs:isDefinedBy <http://vocab.getty.edu/ontology>, ulan: ;
  rdfs:subPropertyOf skos:related;
  rdfs:domain skos:Concept; rdfs:range skos:Concept;
  # domain "person"; range "institution";
  dc:identifier "2583";
  skos:prefLabel "ulan2583_chairman_of";
  dc:title "chairman of - institution" ;
  dct:description """person - chairman of - institution""" .


gvp:ulan2584_chaired_by a owl:ObjectProperty;
  rdfs:isDefinedBy <http://vocab.getty.edu/ontology>, ulan: ;
  rdfs:subPropertyOf skos:related;
  rdfs:domain skos:Concept; rdfs:range skos:Concept;
  # domain "institution"; range "person";
  dc:identifier "2584";
  skos:prefLabel "ulan2584_chaired_by";
  dc:title "chaired by - person" ;
  dct:description """institution - chaired by - person""" .
gvp:ulan2583_chairman_of owl:inverseOf gvp:ulan2584_chaired_by.


gvp:ulan2650_publisher_was a owl:ObjectProperty;
  rdfs:isDefinedBy <http://vocab.getty.edu/ontology>, ulan: ;
  rdfs:subPropertyOf skos:related;
  rdfs:domain skos:Concept; rdfs:range skos:Concept;
  # domain "person"; range "firm";
  dc:identifier "2650";
  skos:prefLabel "ulan2650_publisher_was";
  dc:title "publisher was - firm";
  skos:example "The publisher for Pierre Joseph Rossier was Negretti and Zambra" ;
  dct:description """person - publisher was - firm.
Example: The publisher for Pierre Joseph Rossier was Negretti and Zambra""" .


gvp:ulan2651_publisher_of a owl:ObjectProperty;
  rdfs:isDefinedBy <http://vocab.getty.edu/ontology>, ulan: ;
  rdfs:subPropertyOf skos:related;
  rdfs:domain skos:Concept; rdfs:range skos:Concept;
  # domain "firm"; range "person";
  dc:identifier "2651";
  skos:prefLabel "ulan2651_publisher_of";
  dc:title "publisher of - person";
  skos:example "Negretti and Zambra was the publisher of Pierre Joseph Rossier" ;
  dct:description """firm - publisher of - person.
Example: Negretti and Zambra was the publisher of Pierre Joseph Rossier""" .
gvp:ulan2650_publisher_was owl:inverseOf gvp:ulan2651_publisher_of.


gvp:ulan2674_professor_at a owl:ObjectProperty;
  rdfs:isDefinedBy <http://vocab.getty.edu/ontology>, ulan: ;
  rdfs:subPropertyOf skos:related;
  rdfs:domain skos:Concept; rdfs:range skos:Concept;
  # domain "person"; range "institution";
  dc:identifier "2674";
  skos:prefLabel "ulan2674_professor_at";
  dc:title "professor at - institution";
  skos:example "Paul Klee was a professor at Bauhaus" ;
  dct:description """person - professor at - institution.
Example: Paul Klee was a professor at Bauhaus""" .


gvp:ulan2675_professor_was a owl:ObjectProperty;
  rdfs:isDefinedBy <http://vocab.getty.edu/ontology>, ulan: ;
  rdfs:subPropertyOf skos:related;
  rdfs:domain skos:Concept; rdfs:range skos:Concept;
  # domain "institution"; range "person";
  dc:identifier "2675";
  skos:prefLabel "ulan2675_professor_was";
  dc:title "professor was - person";
  skos:example "A professor at Bauhaus was Paul Klee" ;
  dct:description """institution - professor was - person.
Example: A professor at Bauhaus was Paul Klee""" .
gvp:ulan2674_professor_at owl:inverseOf gvp:ulan2675_professor_was.


gvp:ulan2676_teacher_at a owl:ObjectProperty;
  rdfs:isDefinedBy <http://vocab.getty.edu/ontology>, ulan: ;
  rdfs:subPropertyOf skos:related;
  rdfs:domain skos:Concept; rdfs:range skos:Concept;
  # domain "person"; range "institution";
  dc:identifier "2676";
  skos:prefLabel "ulan2676_teacher_at";
  dc:title "teacher at - institution";
  skos:example "Willem De Kooning was a teacher at Black Mountain College" ;
  dct:description """person - teacher at - institution.
Example: Willem De Kooning was a teacher at Black Mountain College""" .


gvp:ulan2677_teacher_was a owl:ObjectProperty;
  rdfs:isDefinedBy <http://vocab.getty.edu/ontology>, ulan: ;
  rdfs:subPropertyOf skos:related;
  rdfs:domain skos:Concept; rdfs:range skos:Concept;
  # domain "institution"; range "person";
  dc:identifier "2677";
  skos:prefLabel "ulan2677_teacher_was";
  dc:title "teacher was - person";
  skos:example "A teacher at Black Mountain College was Willem De Kooning" ;
  dct:description """institution - teacher was - person.
Example: A teacher at Black Mountain College was Willem De Kooning""" .
gvp:ulan2676_teacher_at owl:inverseOf gvp:ulan2677_teacher_was.


gvp:ulan2692_president_of a owl:ObjectProperty;
  rdfs:isDefinedBy <http://vocab.getty.edu/ontology>, ulan: ;
  rdfs:subPropertyOf skos:related;
  rdfs:domain skos:Concept; rdfs:range skos:Concept;
  # domain "person"; range "institution";
  dc:identifier "2692";
  skos:prefLabel "ulan2692_president_of";
  dc:title "president of - institution";
  skos:example "David K. E. Bruce was president of National Gallery of Art" ;
  dct:description """person - president of - institution.
Example: David K. E. Bruce was president of National Gallery of Art""" .


gvp:ulan2693_president_was a owl:ObjectProperty;
  rdfs:isDefinedBy <http://vocab.getty.edu/ontology>, ulan: ;
  rdfs:subPropertyOf skos:related;
  rdfs:domain skos:Concept; rdfs:range skos:Concept;
  # domain "institution"; range "person";
  dc:identifier "2693";
  skos:prefLabel "ulan2693_president_was";
  dc:title "president was - person";
  skos:example "A president of National Gallery of Art was David K. E. Bruce" ;
  dct:description """institution - president was - person.
Example: A president of National Gallery of Art was David K. E. Bruce""" .
gvp:ulan2692_president_of owl:inverseOf gvp:ulan2693_president_was.


gvp:ulan2696_leader_of a owl:ObjectProperty;
  rdfs:isDefinedBy <http://vocab.getty.edu/ontology>, ulan: ;
  rdfs:subPropertyOf skos:related;
  rdfs:domain skos:Concept; rdfs:range skos:Concept;
  # domain "person"; range "institution";
  dc:identifier "2696";
  skos:prefLabel "ulan2696_leader_of";
  dc:title "leader of - institution";
  skos:example "Rush Harrison Kress was the leader of Samuel H. Kress Foundation" ;
  dct:description """person - leader of - institution.
Example: Rush Harrison Kress was the leader of Samuel H. Kress Foundation""" .


gvp:ulan2697_leader_was a owl:ObjectProperty;
  rdfs:isDefinedBy <http://vocab.getty.edu/ontology>, ulan: ;
  rdfs:subPropertyOf skos:related;
  rdfs:domain skos:Concept; rdfs:range skos:Concept;
  # domain "institution"; range "person";
  dc:identifier "2697";
  skos:prefLabel "ulan2697_leader_was";
  dc:title "leader was - person";
  skos:example "The leader of Samuel H. Kress Foundation was Rush Harrison Kress" ;
  dct:description """institution - leader was - person.
Example: The leader of Samuel H. Kress Foundation was Rush Harrison Kress""" .
gvp:ulan2696_leader_of owl:inverseOf gvp:ulan2697_leader_was.


gvp:ulan2778_owner_of a owl:ObjectProperty;
  rdfs:isDefinedBy <http://vocab.getty.edu/ontology>, ulan: ;
  rdfs:subPropertyOf skos:related;
  rdfs:domain skos:Concept; rdfs:range skos:Concept;
  # domain "firm"; range "person";
  dc:identifier "2778";
  skos:prefLabel "ulan2778_owner_of";
  dc:title "owner of - person";
  skos:example "Walter Scott Lenox was the owner of Lenox China Co." ;
  dct:description """firm - owner of - person.
Example: Walter Scott Lenox was the owner of Lenox China Co.""" .


gvp:ulan2779_owned_by a owl:ObjectProperty;
  rdfs:isDefinedBy <http://vocab.getty.edu/ontology>, ulan: ;
  rdfs:subPropertyOf skos:related;
  rdfs:domain skos:Concept; rdfs:range skos:Concept;
  # domain "person"; range "firm";
  dc:identifier "2779";
  skos:prefLabel "ulan2779_owned_by";
  dc:title "owned by - firm";
  skos:example "Walter Scott Lenox was owned by Lenox China Co." ;
  dct:description """person - owned by - firm.
Example: Walter Scott Lenox was owned by Lenox China Co.""" .
gvp:ulan2778_owner_of owl:inverseOf gvp:ulan2779_owned_by.


gvp:ulan2781_dedicatee_of a owl:ObjectProperty;
  rdfs:isDefinedBy <http://vocab.getty.edu/ontology>, ulan: ;
  rdfs:subPropertyOf skos:related;
  rdfs:domain skos:Concept; rdfs:range skos:Concept;
  # domain "person"; range "institution";
  dc:identifier "2781";
  skos:prefLabel "ulan2781_dedicatee_of";
  dc:title "dedicatee of - institution";
  skos:example "Auguste Rodin is the dedicatee of The Rodin Museum in Philadelphia" ;
  dct:description """person - dedicatee of - institution.
Example: Auguste Rodin is the dedicatee of The Rodin Museum in Philadelphia""" .


gvp:ulan2782_dedicated_to a owl:ObjectProperty;
  rdfs:isDefinedBy <http://vocab.getty.edu/ontology>, ulan: ;
  rdfs:subPropertyOf skos:related;
  rdfs:domain skos:Concept; rdfs:range skos:Concept;
  # domain "institution"; range "person";
  dc:identifier "2782";
  skos:prefLabel "ulan2782_dedicated_to";
  dc:title "dedicated to - person";
  skos:example "The Rodin Museum in Philadelphia is didicated to Auguste Rodin" ;
  dct:description """institution - dedicated to - person.
Example: The Rodin Museum in Philadelphia is didicated to Auguste Rodin""" .
gvp:ulan2781_dedicatee_of owl:inverseOf gvp:ulan2782_dedicated_to.


gvp:ulan2794_representative_of a owl:ObjectProperty;
  rdfs:isDefinedBy <http://vocab.getty.edu/ontology>, ulan: ;
  rdfs:subPropertyOf skos:related;
  rdfs:domain skos:Concept; rdfs:range skos:Concept;
  # domain "person"; range "institution";
  dc:identifier "2794";
  skos:prefLabel "ulan2794_representative_of";
  dc:title "representative of - institution";
  skos:example "The Noguch Museum - representative was Isamu Noguchi" ;
  dct:description """person - representative of - institution.
Example: The Noguch Museum - representative was Isamu Noguchi""" .


gvp:ulan2795_representative_was a owl:ObjectProperty;
  rdfs:isDefinedBy <http://vocab.getty.edu/ontology>, ulan: ;
  rdfs:subPropertyOf skos:related;
  rdfs:domain skos:Concept; rdfs:range skos:Concept;
  # domain "institution"; range "person";
  dc:identifier "2795";
  skos:prefLabel "ulan2795_representative_was";
  dc:title "representative was - person";
  skos:example "The Noguch Museum - representative was Isamu Noguchi" ;
  dct:description """institution - representative was - person.
Example: The Noguch Museum - representative was Isamu Noguchi""" .
gvp:ulan2794_representative_of owl:inverseOf gvp:ulan2795_representative_was.


gvp:ulan2828_student_at a owl:ObjectProperty;
  rdfs:isDefinedBy <http://vocab.getty.edu/ontology>, ulan: ;
  rdfs:subPropertyOf skos:related;
  rdfs:domain skos:Concept; rdfs:range skos:Concept;
  # domain "person"; range "institution";
  dc:identifier "2828";
  skos:prefLabel "ulan2828_student_at";
  dc:title "student at - institution";
  skos:example "Zdanek Rossman was a student at Bauhaus" ;
  dct:description """person - student at - institution.
Example: Zdanek Rossman was a student at Bauhaus""" .


gvp:ulan2829_student_was a owl:ObjectProperty;
  rdfs:isDefinedBy <http://vocab.getty.edu/ontology>, ulan: ;
  rdfs:subPropertyOf skos:related;
  rdfs:domain skos:Concept; rdfs:range skos:Concept;
  # domain "institution"; range "person";
  dc:identifier "2829";
  skos:prefLabel "ulan2829_student_was";
  dc:title "student was - person";
  skos:example "Bauhaus student was Zdanek Rossman" ;
  dct:description """institution - student was - person.
Example: Bauhaus student was Zdanek Rossman""" .
gvp:ulan2828_student_at owl:inverseOf gvp:ulan2829_student_was.


gvp:ulan2840_performer_with a owl:ObjectProperty;
  rdfs:isDefinedBy <http://vocab.getty.edu/ontology>, ulan: ;
  rdfs:subPropertyOf skos:related;
  rdfs:domain skos:Concept; rdfs:range skos:Concept;
  # domain "person"; range "group";
  dc:identifier "2840";
  skos:prefLabel "ulan2840_performer_with";
  dc:title "performer with - group" ;
  dct:description """person - performer with - group""" .


gvp:ulan2841_performer_was a owl:ObjectProperty;
  rdfs:isDefinedBy <http://vocab.getty.edu/ontology>, ulan: ;
  rdfs:subPropertyOf skos:related;
  rdfs:domain skos:Concept; rdfs:range skos:Concept;
  # domain "group"; range "person";
  dc:identifier "2841";
  skos:prefLabel "ulan2841_performer_was";
  dc:title "performer was - person" ;
  dct:description """group - performer was - person""" .
gvp:ulan2840_performer_with owl:inverseOf gvp:ulan2841_performer_was.
