@prefix dc:    <http://purl.org/dc/elements/1.1/> .
@prefix dcterms: <http://purl.org/dc/terms/> .
@prefix iso-thes: <http://purl.org/iso25964/skos-thes#> .
@prefix owl:   <http://www.w3.org/2002/07/owl#> .
@prefix rdf:   <http://www.w3.org/1999/02/22-rdf-syntax-ns#> .
@prefix rdfs:  <http://www.w3.org/2000/01/rdf-schema#> .
@prefix skos:  <http://www.w3.org/2004/02/skos/core#> .
@prefix voaf:  <http://purl.org/vocommons/voaf#> .
@prefix vs:    <http://www.w3.org/2003/06/sw-vocab-status/ns#> .
@prefix xl:    <http://www.w3.org/2008/05/skos-xl#> .
@prefix xsd:   <http://www.w3.org/2001/XMLSchema#> .

<http://purl.org/iso25964/skos-thes>
        a                    owl:Ontology ;
        rdfs:comment         "These notes apply to the published mapping between the ISO 25964 data model and the SKOS schema (http://www.niso.org/schemas/iso25964/correspondencesSKOS/).\nRemarks can be exchanged using: 25964info@list.niso.org \nSubscription info and archive is on: http://www.niso.org/lists/25964info/ \nGeneral information about ISO 25964: http://www.niso.org/schemas/iso25964/\n\nThe annotation http://www.w3.org/2003/06/sw-vocab-status/ns#term_status indicates \"proposed\" properties that are not part of the mapping documentation."@en ;
        rdfs:seeAlso         <http://www.niso.org/schemas/iso25964/correspondencesSKOS/> ;
        dc:date              "2013-12-09"^^xsd:date ;
        dcterms:contributor  "Marcia Lei Zeng" , "Jutta Lindenthal" , "Leonard Will" , "Douglas S. Tudhope" , "Vladimir Alexiev" , "Stella Dextre Clarke" ;
        dcterms:created      "2013-10-04"^^xsd:date ;
        dcterms:creator      "Antoine Isaac" , "Johan De Smedt" ;
        dcterms:modified     "2013-12-09"^^xsd:date ;
        voaf:toDoList        "Todo: \nNot modelled but requiring further extension:\n\n- CustomTermAttribute : \n  Best practice would be to define custom RDF data-type properties taking plain literal values. The property name depends on the customAttributeType.\n\n- CustomConceptAttribute :\n  Best practice would be to define custom RDF data-type properties taking plain literal values. The property name depends on the customAttributeType.\n\n- refersTo (reference from within a note to a concept or label/term:\n   May be an embedded and tagged link in the note value (e.g., as done for EuroVoc http://eurovoc.europa.eu/).\n\n- CustomNote :\n  Depending noteType a new custom property should be defined as a sub-property of skos:note (consider applicability of: skos:changeNote and skos:example)\n \n - BTG/NTG - BTP/NTP - BTI/NTI :\n   Currently these are only defined as direct (one-step) sub-properties of skos:broader / skos:narrower.\n\nSome constraints currently expressed only in natural language (in rdfs:comment) may be formally expressed as OWL(2) axioms.\n\nWe have postponed the implementation of the iso-thes properties mentioned in the VersionHistory section of the mapping documentation." ;
        owl:imports          <http://www.w3.org/2004/02/skos/core> , <http://www.w3.org/2008/05/skos-xl> .

iso-thes:CompoundEquivalence
        a                 owl:Class ;
        rdfs:comment      "ISO CompoundEquivalence \n\niso-thes:plusUseTerm (and its inverse iso-thes:plusUFTerm) may be derived from iso-thes:CompoundEquivalence.\n\nFor a iso-thes:CompoundEquivalence instance each derived iso thes:plusUseTerm has as:\n- subject: the iso thes:plusUF value\n- object: the iso thes:plusUse value\n\nAn ISO 25964 compliant thesaurus only has one compound equivalence relation for each split non preferred term.\n\nIn special cases where the iso-thes:SplitNonPreferredTerm has more than one decomposition, the inverse inference may not be possible.   (While this situation should not arise within a single thesaurus that complies with ISO 25964, it could occur if terms and relationships have been drawn from more than one thesaurus. For this reason the property skos:inScheme (http://www.w3.org/2004/02/skos/core#inScheme) should be used with each instance of the class Compound Equivalence, to relate it to its Thesaurus.)"@en ;
        rdfs:isDefinedBy  <http://purl.org/iso25964/skos-thes> ;
        rdfs:label        "Compound Equivalence"@en ;
        rdfs:subClassOf   [ a                         owl:Restriction ;
                            owl:onClass               iso-thes:SplitNonPreferredTerm ;
                            owl:onProperty            iso-thes:plusUF ;
                            owl:qualifiedCardinality  "1"^^xsd:nonNegativeInteger
                          ] ;
        rdfs:subClassOf   [ a                            owl:Restriction ;
                            owl:minQualifiedCardinality  "2"^^xsd:nonNegativeInteger ;
                            owl:onClass                  iso-thes:PreferredTerm ;
                            owl:onProperty               iso-thes:plusUse
                          ] ;
        dcterms:modified  "2013-12-09"^^xsd:date ;
        vs:term_status    "released" .

iso-thes:ConceptGroup
        a                 owl:Class ;
        rdfs:comment      "ISO ConceptGroup\n\nConcept groups have several applications.\n\nOne such application is illustrated by the EUROVOC and the UNESCO thesaurus.  Both of these use a super structure of domain and of micro-thesaurus.  Both of these structuring elements can be modeled using ConceptGroup."@en ;
        rdfs:isDefinedBy  <http://purl.org/iso25964/skos-thes> ;
        rdfs:label        "Concept Group"@en ;
        rdfs:subClassOf   skos:Collection ;
        dcterms:modified  "2013-12-09"^^xsd:date ;
        owl:disjointWith  iso-thes:ThesaurusArray ;
        vs:term_status    "released" ;
        skos:definition   "Definition: A concept group is a group of concepts making up a subset of the thesaurus. Member concepts may be drawn from many different facets or hierarchies of the thesaurus. While almost any criterion may be used to select the members, this construct is commonly used to define a micro-thesaurus that will be used by a particular user group or domain.\n\nThe skos:inScheme (http://www.w3.org/2004/02/skos/core#inScheme) property should be used to indicate the thesaurus to which an instance of skos:Collection applies (see ISO 25964: isPartOf).\n\nUse rdfs:label or xl:prefLabel for the ConceptGroup label (1 per language).\nOptional label attributes typically are mapped to dc: (or dct:) properties:\n- dct:created\n- dct:modified\nThese can be attached to the xl:Label instance that is the value of the xl:prefLabel.\n\nDepending on the value of the ISO conceptGroupType a sub-class of iso thes:ConceptGroup should be defined.\ne.g.: EUROVOC and UNESCO use\n- Domain\n- MicroThesaurus (an iso-thes:hasSubGroup of a Domain)"@en .

iso-thes:PreferredTerm
        a                 owl:Class ;
        rdfs:comment      "ISO PreferredTerm:\n\nInstances of iso-thes:PreferredTerm are objects of skos-xl:prefLabel statements.\n\nMaking the class explicit allows RDF/OWL consistency checks for CompoundEquivalence."@en ;
        rdfs:isDefinedBy  <http://purl.org/iso25964/skos-thes> ;
        rdfs:label        "Preferred Term"@en ;
        rdfs:subClassOf   xl:Label ;
        dcterms:modified  "2013-12-09"^^xsd:date ;
        vs:term_status    "released" .

iso-thes:SimpleNonPreferredTerm
        a                 owl:Class ;
        rdfs:comment      "ISO SimpleNonPreferredTerm\n\nInstances of iso:SimpleNonPreferredTerm are the object of either of skos xl:altLabel or skos xl:hiddenLabel statements.\n\n\nIdentifying cases of Equivalence:\n\nIn SKOS/-XL, Equivalence may be derived between the skos/skos xl:prefLabel statements on one hand and the skos/skos xl:altLabel or the skos/skos xl:hiddenLabel statements on the other hand where:\n- the subject of all these statements is the same instance of skos:Concept,\n- the language of all the bound labels is the same,\n- the prefLabel has the role USE, and\n- the altLabel and hiddenLabel have the role UF."@en ;
        rdfs:isDefinedBy  <http://purl.org/iso25964/skos-thes> ;
        rdfs:label        "Simple Non Preferred Term"@en ;
        rdfs:subClassOf   xl:Label ;
        dcterms:modified  "2013-12-09"^^xsd:date ;
        vs:term_status    "released" .

iso-thes:SplitNonPreferredTerm
        a                 owl:Class ;
        rdfs:comment      "iso SplitNonPreferredTerm\n\nThis class provides for an 'imagined' concept that may exist in a userâ€™s mind but is not present in the thesaurus (Concept Scheme); it can, however, be represented by a combination of two or more preferred terms (skos-xl:prefLabel) in the thesaurus. (In contrast, concepts present in the thesaurus are provided for by the ThesaurusConcept class.)\nThis label is provided by the object property iso thes:plusUF\n- domain: iso-thes:CompoundEquivalence\n- range: iso-thes:SplitNonPreferredTerm."@en ;
        rdfs:isDefinedBy  <http://purl.org/iso25964/skos-thes> ;
        rdfs:label        "Split Non Preferred Term"@en ;
        rdfs:subClassOf   xl:Label ;
        dcterms:modified  "2013-12-09"^^xsd:date ;
        vs:term_status    "released" .

iso-thes:ThesaurusArray
        a                 owl:Class ;
        rdfs:isDefinedBy  <http://purl.org/iso25964/skos-thes> ;
        rdfs:label        "Thesaurus Array"@en ;
        rdfs:subClassOf   skos:Collection ;
        dcterms:modified  "2013-12-09"^^xsd:date ;
        vs:term_status    "released" ;
        skos:definition   "Definition: ISO ThesaurusArray\nAn array is a group of sibling concepts\n\nInstances of ThesaurusArray can be mapped to instances of skos:OrderedCollection (a subclass of skos:Collection) if and only if the array needs to be an ordered array (in the ISO-25964 model the value of its Boolean attribute \"ordered\" is true).\nIt is advised to use the skos:inScheme (http://www.w3.org/2004/02/skos/core#inScheme) property on such a skos:Collection to relate it to its Thesaurus (see ISO 25964: isPartOf).\n\nConcepts in a thesaurus array are sibling concepts in the thesaurus.\n\nIf present, the node label of a thesaurus array is mapped to rdfs:label or xl:prefLabel.\nOptional node label attributes typically are mapped to dc: (or dct:) properties:\n- dct:created\n- dct:modified\nThese can be attached (if needed) to the xl:Label instance that is the value of xl:prefLabel."@en .

iso-thes:broaderGeneric
        a                   owl:ObjectProperty ;
        rdfs:domain         skos:Concept ;
        rdfs:isDefinedBy    <http://purl.org/iso25964/skos-thes> ;
        rdfs:label          "broader term (generic)"@en ;
        rdfs:range          skos:Concept ;
        rdfs:subPropertyOf  skos:broader ;
        dcterms:modified    "2013-11-11"^^xsd:date ;
        vs:term_status      "proposed" ;
        skos:definition     "Definition: ISO 25964-1: BTG\nThe immediate (direct or one-step) class - generalized class relationship."@en .

iso-thes:broaderInstantial
        a                   owl:ObjectProperty ;
        rdfs:domain         skos:Concept ;
        rdfs:isDefinedBy    <http://purl.org/iso25964/skos-thes> ;
        rdfs:label          "broader term (instantial)"@en ;
        rdfs:range          skos:Concept ;
        rdfs:subPropertyOf  skos:broader ;
        dcterms:modified    "2013-12-09"^^xsd:date ;
        vs:term_status      "proposed" ;
        skos:changeNote     "The URI has been renamed: #broaderInstantive is replaced by #broaderInstantial according to the observed usage of these words in English. (2013-12-09)"@en ;
        skos:definition     "Definition: ISO 25964-1: BTI\nThe immediate (direct or one-step) instance - class relationship."@en .

iso-thes:broaderPartitive
        a                   owl:ObjectProperty ;
        rdfs:domain         skos:Concept ;
        rdfs:isDefinedBy    <http://purl.org/iso25964/skos-thes> ;
        rdfs:label          "broader term (partitive)"@en ;
        rdfs:range          skos:Concept ;
        rdfs:subPropertyOf  skos:broader ;
        dcterms:modified    "2013-11-18"^^xsd:date ;
        vs:term_status      "proposed" ;
        skos:definition     "Definition: ISO 25964-1: BTP\nWhen the ISO 25964 standard is followed, the BTP/NTP relationship should qualify for a transitive closure."@en ;
        skos:example        "A \"bicycle wheel\" for instance belongs uniquely to a \"bicycle\" while a \"wheel\" does not.\nA BTP/NTP relationship should not be established between \"bicycles\" and \"wheels\" because a wheel could be part of a motor car, a wheelbarrow or one of many other artefacts."@en .

iso-thes:microThesaurusOf
        a                   owl:ObjectProperty ;
        rdfs:domain         iso-thes:ConceptGroup ;
        rdfs:isDefinedBy    <http://purl.org/iso25964/skos-thes> ;
        rdfs:label          "micro-thesaurus of"@en ;
        rdfs:range          skos:ConceptScheme ;
        rdfs:subPropertyOf  skos:inScheme ;
        dcterms:modified    "2013-10-04"^^xsd:date ;
        vs:term_status      "released" ;
        skos:definition     "Definition: Concept groups published as sub-thesauri (e.g., having micro-thesaurus as ISO conceptGroupType)"@en .

iso-thes:narrowerGeneric
        a                   owl:ObjectProperty ;
        rdfs:domain         skos:Concept ;
        rdfs:isDefinedBy    <http://purl.org/iso25964/skos-thes> ;
        rdfs:label          "narrower term (generic)"@en ;
        rdfs:range          skos:Concept ;
        rdfs:subPropertyOf  skos:narrower ;
        dcterms:modified    "2013-11-11"^^xsd:date ;
        owl:inverseOf       iso-thes:broaderGeneric ;
        vs:term_status      "proposed" ;
        skos:definition     "Definition: ISO 25964-1: NTG\nThe immediate (direct or one-step) class - specialized class relationship."@en .

iso-thes:narrowerInstantial
        a                   owl:ObjectProperty ;
        rdfs:domain         skos:Concept ;
        rdfs:isDefinedBy    <http://purl.org/iso25964/skos-thes> ;
        rdfs:label          "narrower term (instantial)"@en ;
        rdfs:range          skos:Concept ;
        rdfs:subPropertyOf  skos:narrower ;
        dcterms:modified    "2013-12-09"^^xsd:date ;
        owl:inverseOf       iso-thes:broaderInstantial ;
        vs:term_status      "proposed" ;
        skos:changeNote     "The URI has been renamed: #narrowerInstantive is replaced by #narrowerInstantial according to the observed usage of these words in English. (2013-12-09)"@en ;
        skos:definition     "Definition: ISO 25964-1: NTI\nThe immediate (direct or one-step) class - instance relationship."@en .

iso-thes:narrowerPartitive
        a                   owl:ObjectProperty ;
        rdfs:domain         skos:Concept ;
        rdfs:isDefinedBy    <http://purl.org/iso25964/skos-thes> ;
        rdfs:label          "narrower term (partitive)"@en ;
        rdfs:range          skos:Concept ;
        rdfs:subPropertyOf  skos:narrower ;
        dcterms:modified    "2013-11-18"^^xsd:date ;
        owl:inverseOf       iso-thes:broaderPartitive ;
        vs:term_status      "proposed" ;
        skos:definition     "Definition: ISO 25964-1: NTP\nWhen the ISO 25964 standard is followed, the BTP/NTP relationship should qualify for a transitive closure."@en ;
        skos:example        "A \"bicycle wheel\" for instance belongs uniquely to a \"bicycle\" while a \"wheel\" does not.\nA BTP/NTP relationship should not be established between \"bicycles\" and \"wheels\" because a wheel could be part of a motor car, a wheelbarrow or one of many other artefacts."@en .

iso-thes:plusUF  a        owl:ObjectProperty ;
        rdfs:domain       iso-thes:CompoundEquivalence ;
        rdfs:isDefinedBy  <http://purl.org/iso25964/skos-thes> ;
        rdfs:label        "split non preferred term"@en ;
        rdfs:range        iso-thes:SplitNonPreferredTerm ;
        dcterms:modified  "2013-10-04"^^xsd:date ;
        vs:term_status    "released" ;
        skos:definition   "Definition: ISO 25964-1: UF+\nThe non preferred term labeling a complex concept.\nThe complex concept will be identified by splitting the non preferred term into 2 or more (component) preferred terms."@en .

iso-thes:plusUFTerm  a      owl:ObjectProperty ;
        rdfs:domain         iso-thes:PreferredTerm ;
        rdfs:isDefinedBy    <http://purl.org/iso25964/skos-thes> ;
        rdfs:label          "UF+"@en ;
        rdfs:range          iso-thes:SplitNonPreferredTerm ;
        rdfs:subPropertyOf  xl:labelRelation ;
        dcterms:modified    "2013-12-09"^^xsd:date ;
        owl:inverseOf       iso-thes:plusUseTerm ;
        vs:term_status      "released" ;
        skos:definition     "Definition: ISO 25964-1: UF+\nThe non-preferred term expressing a compound concept that should be represented by a combination of preferred terms"@en .

iso-thes:plusUse  a       owl:ObjectProperty ;
        rdfs:domain       iso-thes:CompoundEquivalence ;
        rdfs:isDefinedBy  <http://purl.org/iso25964/skos-thes> ;
        rdfs:label        "component preferred term"@en ;
        rdfs:range        iso-thes:PreferredTerm ;
        dcterms:modified  "2013-10-04"^^xsd:date ;
        vs:term_status    "released" ;
        skos:scopeNote    "ISO 25964-1: USE+\nOne of two or more (component) preferred terms used together to represent the (complex) concept labeled by a (split) non preferred term."@en .

iso-thes:plusUseTerm  a     owl:ObjectProperty ;
        rdfs:domain         iso-thes:SplitNonPreferredTerm ;
        rdfs:isDefinedBy    <http://purl.org/iso25964/skos-thes> ;
        rdfs:label          "USE+"@en ;
        rdfs:range          iso-thes:PreferredTerm ;
        rdfs:subPropertyOf  xl:labelRelation ;
        dcterms:modified    "2013-10-04"^^xsd:date ;
        vs:term_status      "released" ;
        skos:definition     "Definition: ISO 25964-1: USE+\nThe two or more (component) preferred terms following should be used together to represent the concept indicated by the (split) non preferred term."@en ;
        skos:scopeNote      "iso-thes:plusUseTerm (and its inverse iso-thes:plusUFTerm) may be derived from iso-thes:CompoundEquivalence.\n\nFor an iso-thes:CompoundEquivalence instance each derived iso-thes:plusUseTerm has as:\n- subject: the iso-thes:plusUF value\n- object: the iso-thes:plusUse value\n\nIn special cases where the iso-thes:SplitNonPreferredTerm has more than one decomposition, the inverse inference may not be possible."@en .

iso-thes:status  a        owl:DatatypeProperty ;
        rdfs:comment      "ISO status\n- on ThesaurusConcept\n- on ThesaurusTerm"@en ;
        rdfs:domain       [ a            owl:Class ;
                            owl:unionOf  ( skos:Concept xl:Label )
                          ] ;
        rdfs:isDefinedBy  <http://purl.org/iso25964/skos-thes> ;
        rdfs:label        "status"@en ;
        rdfs:range        xsd:string ;
        dcterms:modified  "2013-10-04"^^xsd:date ;
        vs:term_status    "released" .

iso-thes:subGroup  a      owl:ObjectProperty , owl:TransitiveProperty ;
        rdfs:domain       iso-thes:ConceptGroup ;
        rdfs:isDefinedBy  <http://purl.org/iso25964/skos-thes> ;
        rdfs:label        "sub group"@en ;
        rdfs:range        iso-thes:ConceptGroup ;
        dcterms:modified  "2013-10-04"^^xsd:date ;
        owl:inverseOf     iso-thes:superGroup ;
        vs:term_status    "released" ;
        skos:definition   "Definition: All members of the (object) subGroup are members of the (subject) group."@en .

iso-thes:subordinateArray
        a                 owl:ObjectProperty ;
        rdfs:domain       skos:Concept ;
        rdfs:isDefinedBy  <http://purl.org/iso25964/skos-thes> ;
        rdfs:label        "subordinate array"@en ;
        rdfs:range        iso-thes:ThesaurusArray ;
        dcterms:modified  "2013-12-09"^^xsd:date ;
        vs:term_status    "released" ;
        skos:definition   "Definition: Explicitly links a (superordinate) concept to one or more subordinate arrays. Each array may either be composed of narrower concepts of the superordinate concept (in which case there may be an associated node label with a characteristic of division) or by concepts that need not be narrower concepts of the superordinate concept (in which case a node label may provide a facet name).\n\nIn other words, though each array only contains sibling concepts, no hierarchical relation may be automatically derived between a concept and the concepts in any of its subordinate arrays. The hierarchical relationship between these concepts has to be asserted explicitly."@en .

iso-thes:superGroup  a    owl:TransitiveProperty , owl:ObjectProperty ;
        rdfs:domain       iso-thes:ConceptGroup ;
        rdfs:isDefinedBy  <http://purl.org/iso25964/skos-thes> ;
        rdfs:label        "super group"@en ;
        rdfs:range        iso-thes:ConceptGroup ;
        dcterms:modified  "2013-11-11"^^xsd:date ;
        vs:term_status    "released" ;
        skos:definition   "Definition: All members of the (subject) group are members of the (object) superGroup."@en .

iso-thes:superOrdinate
        a                 owl:ObjectProperty ;
        rdfs:domain       iso-thes:ThesaurusArray ;
        rdfs:isDefinedBy  <http://purl.org/iso25964/skos-thes> ;
        rdfs:label        "super ordinate"@en ;
        rdfs:range        skos:Concept ;
        dcterms:modified  "2013-11-09"^^xsd:date ;
        owl:inverseOf     iso-thes:subordinateArray ;
        vs:term_status    "released" ;
        skos:definition   "Definition: ISO 25964: hasSuperOrdinateConcept\nThe (subject) array organizes a set of sibling concepts under the (object) concept."@en .


[ a                 owl:AllDisjointClasses ;
  dcterms:modified  "2013-10-04"^^xsd:date ;
  owl:members       ( iso-thes:PreferredTerm iso-thes:SimpleNonPreferredTerm iso-thes:SplitNonPreferredTerm )
] .

skos:Concept  rdfs:comment  "super class of ISO ThesaurusConcept\n\nThe mandatory attribute identifier may be mapped to the Dublin Core property dc:identifier.\nAttributes or associations not detailed below typically are mapped to dc: (or dct:) properties:\n- dct:created\n- dct:modified"@en .

skos:ConceptScheme  rdfs:comment  "super class of ISO Thesaurus\n\nThe mandatory attribute identifier may be mapped to the Dublin Core property dc:identifier. A typical representation of a thesaurus should document a (scoped) relationship between an identifier of this thesaurus and the URI of the RDF Concept Scheme URI.\n\nThe mandatory attribute lang can be mapped to either of the Dublin Core properties dc:language or dct:language. The value space is defined by RFC 4646. For multilingual thesaurus, one lang attribute is needed per supported language.\n\nTypically these can be mapped to the corresponding Dublin Core dc: (or dct:) properties:\n- dc:contributor\n- dc:coverage\n- dc:creator\n- dct:created\n- dct:modified\n- dc:date\n- skos:definition\n- dc:format\n- dc:publisher\n- dc:relation, dct:relation or a specialization\n- dc:rights\n- dc:source\n- dc:subject\n- dc:title\n- dc:type\n\nThe association \"hasVersion\" is discussed in the Version_History section of the mapping documentation (http://www.niso.org/schemas/iso25964/correspondencesSKOS/)."@en .

skos:altLabel  rdfs:comment  "Simple or basic super property of ISO hasNonPreferredLabel\n\nApplies if the value of \"hasNonPreferredLabel\" is of class SimpleNonPreferredTerm with the Boolean attribute \"hidden\" either absent or with value false."@en .

skos:broader  skos:definition  "Comment: As an extension to SKOS, sub-properties of skos:broader and skos:narrower may be needed to model the different hierarchical relationships identified by the ISO 25964 attribute \"role\"."@en .

skos:broaderTransitive
        rdfs:comment  "Can be used to derive ISO hasTopConcept (which is different from skos:hasTopConcept).\n\nThe ISO hasTopConcept can be derived in SKOS from skos:broaderTransitive where the object of skos:broaderTransitive is a concept having the property skos:topConceptOf (i.e., a ThesaurusConcept having topConcept = true)."@en .

skos:definition  skos:definition  "Caution: In ISO 25964, \"hasDefinition\" applies to a term rather than to a concept."@en .

skos:editorialNote  skos:definition  "Caution: In ISO 25964, \"hasEditorialNote\" applies to a term rather than to a concept."@en .

skos:hasTopConcept  skos:definition  "Definition: Captures ISO TopLevelRelationship"@en .

skos:hiddenLabel  rdfs:comment  "Simple or basic super property of ISO hasNonPreferredLabel\n\nApplies if the value of \"hasNonPreferredLabel\" is of class SimpleNonPreferredTerm with the Boolean attribute \"hidden\" having value true."@en .

skos:historyNote  skos:definition  "Definition: In ISO 25964, \"hasHistoryNote\" can apply to a term or to a concept."@en .

skos:inScheme  rdfs:comment  "Super property of ISO isPartOf\n\nApplies to any ISO 25964 \"isPartOf\" relation that targets the Thesaurus. Subjects of the skos:inScheme statements can be ISO 25964â€™s ThesaurusConcept, ConceptGroup, and ThesaurusArray.\n\nOnly applies to ISO 25964 \"contains\" statements having a Thesaurus [ConceptScheme] as subject."@en .

skos:member  rdfs:comment  "ISO\n- hasMemberArray\n- hasMemberConcept\n- hasAsMember\nNote: SKOS S39 (any concept in a List of a skos:memberList is also a value of skos:member).\n\nBy definition, used to represent members of a thesaurus Array or of a thesaurus Group.\n\nAn Array may have as members thesaurus Concepts or other thesaurus Arrays.\n\nThesaurus Group members are thesaurus Concepts."@en .

skos:memberList  rdfs:comment  "ISO\n- hasMemberArray<ordered=true>\n- hasMemberConcept<ordered=true>"@en .

skos:narrower  skos:definition  "Comment: As an extension to SKOS, sub-properties of skos:broader and skos:narrower may be needed to model the different hierarchical relationships identified by the ISO 25964 attribute \"role\"."@en .

skos:narrowerTransitive
        rdfs:comment  "Can be used to derive ISO isTopConceptOf (which is different from skos:isTopConceptOf).\n\nThe ISO isTopConceptOf can be derived in SKOS from skos:narrowerTransitive where the skos:narrowerTransitive has as subject a concept that is object of a skos:hasTopConcept statement (i.e., a ThesaurusConcept having topConcept = true)."@en .

skos:notation  rdfs:comment  "Best practice in SKOS is to (RDF) type the notation value object. This allows multiple notation value types for the same concept or term to be distinguished. \n\nNote: In ISO 25964-1, such typing is implicit in the thesaurus or it is part of the \"notation\" value."@en .

skos:note  rdfs:comment  "ISO refersTo is not mapped.\n\nWork is ongoing in the RDF group to type the content explicitly as HTML or XML in RDF1.1 (http://dvcs.w3.org/hg/rdf/raw-file/default/rdf-concepts/index.html#section-html). This would allow embedding relevant hyperlinks in notes.\n\nMay be an embedded and tagged link in the note value (e.g., as done for EuroVoc).\n\n\nIn ISO 25964, some types of Note are associated with concepts, others with terms. In SKOS, all documentation notes are associated with concepts.\n\nIn basic SKOS, notes are represented using simple annotation properties, which type captures the note type. However the SKOS annotation properties can also be used with structured representation of notes as fully-fledged resources. See http://www.w3.org/TR/skos-primer/#secdocumentation and http://www.w3.org/TR/skos-primer/#secadvanceddocumentation for examples of both approaches.\n\nWithin a thesaurus the application of notes to concept and term is more restrictive than in SKOS.\n\nA note may have some structure or formatting. In general, this can be modelled using rdf:value (to represent lexicalValue)\n\nThe language should be held in rdf:value. If this is an XMLLiteral, the language shall also be made available using dc:language (or dct:language).\n\nNote: Work is ongoing in the RDF group to type the content explicitly as HTML or XML In RDF1.1 (http://dvcs.w3.org/hg/rdf/raw-file/default/rdf-concepts/index.html#section-html). This would allow embedding relevant hyperlinks in notes.\n\nAdditional attributes can be added to the note structure:\n- dct:created\n- dct:modified"@en .

skos:prefLabel  rdfs:comment  "Simple super property of ISO hasPreferredLabel\n\nBasic SKOS allows labels (as simple literals) to be attached directly to Concepts using skos:prefLabel; this is the preferred simple scenario where label relations are not explicit."@en .

skos:related  skos:definition  "Comment: As an extension to SKOS, sub-properties of skos:related may be needed to model the different associative relationships identified by the ISO 25964 attribute \"role\"."@en .

skos:scopeNote  skos:definition  "Caution: In ISO 25964, \"hasScopeNote\" applies to a concept rather than to a term."@en .

skos:topConceptOf  skos:definition  "Definition: Super property of ISO isPartOf of a ThesaurusConcept having its attribute topConcept = true.\n\nCaptures ISO TopLevelRelationship"@en .

vs:term_status  a         owl:AnnotationProperty ;
        rdfs:isDefinedBy  <http://www.w3.org/2003/06/sw-vocab-status/ns> ;
        rdfs:label        "model axiom or term status"@en ;
        rdfs:range        <http://ec.europa.eu/esco/model#statusDataType> ;
        dcterms:issued    "2013-12-05"^^xsd:date ;
        dcterms:modified  "2013-12-05"^^xsd:date ;
        vs:term_status    "proposed" .

xl:Label  rdfs:comment  "Super class of ISO ThesaurusTerm and of ISO NodeLabel.\n\nA ThesaurusTerm has mandatory attributes lexicalValue and identifier. lexicalValue can be mapped to skos xl:literalForm. The value of identifier can be used as the URI of the skos xl:Label or as the object of a dc:identifier statement on that skos-xl:Label.\nA NodeLabel has mandatory attributes lexicalValue.\n\nThe optional ISO25964 lang attribute of ThesaurusTerm and of NodeLabel must be mapped to RDF language tag for RDF plain literals.\n\nAttributes or associations not detailed below typically are mapped to dc: (or dct:) properties:\n- dct:created\n- dct:modified\n- dc:source"@en .

xl:altLabel  rdfs:comment  "Complex super property of ISO hasNonPreferredLabel\n\nApplies if the value of \"hasNonPreferredLabel\" is of class SimpleNonPreferredTerm with the Boolean attribute \"hidden\" either absent or with value false."@en .

xl:hiddenLabel  rdfs:comment  "Complex super property of ISO hasNonPreferredLabel\n\nApplies if the value of \"hasNonPreferredLabel\" is of class SimpleNonPreferredTerm with the Boolean attribute \"hidden\" having value true."@en .

xl:prefLabel  rdfs:comment  "Complex super property of ISO hasPreferredLabel\n\nWhen a label is represented as skos xl:Label, a skos:prefLabel statement is derived from the skos-xl:prefLabel one. (Likewise for altLabel and hiddenLabel.)"@en .

<http://ec.europa.eu/esco/model#statusDataType>
        a                    rdfs:Datatype ;
        rdfs:comment         "list of status values used for managing ESCO ontology changes."@en ;
        rdfs:isDefinedBy     <http://ec.europa.eu/esco/model> ;
        rdfs:label           "term status type" ;
        dcterms:modified     "2013-12-05" ;
        owl:equivalentClass  [ a            rdfs:Datatype ;
                               owl:unionOf  ( [ a                     rdfs:Datatype ;
                                                owl:onDatatype        xsd:string ;
                                                owl:withRestrictions  ( [ xsd:pattern  "approved" ]
                                                                      )
                                              ]
                                              [ a                     rdfs:Datatype ;
                                                owl:onDatatype        xsd:string ;
                                                owl:withRestrictions  ( [ xsd:pattern  "prepared" ]
                                                                      )
                                              ]
                                              [ a                     rdfs:Datatype ;
                                                owl:onDatatype        xsd:string ;
                                                owl:withRestrictions  ( [ xsd:pattern  "proposed" ]
                                                                      )
                                              ]
                                              [ a                     rdfs:Datatype ;
                                                owl:onDatatype        xsd:string ;
                                                owl:withRestrictions  ( [ xsd:pattern  "rejected" ]
                                                                      )
                                              ]
                                              [ a                     rdfs:Datatype ;
                                                owl:onDatatype        xsd:string ;
                                                owl:withRestrictions  ( [ xsd:pattern  "released" ]
                                                                      )
                                              ]
                                            )
                             ] ;
        vs:term_status       "proposed" .
